<?xml version="1.0" encoding="UTF-8"?>
<!DOCTYPE rdf:RDF [
	<!ENTITY auto-mo "https://spec.edmcouncil.org/auto/ontology/MO/MiddleOntology/">
	<!ENTITY auto-vc "https://spec.edmcouncil.org/auto/ontology/VC/VehicleCore/">
	<!ENTITY dc "http://purl.org/dc/elements/1.1/">
	<!ENTITY dct "http://purl.org/dc/terms/">
	<!ENTITY dctype "http://purl.org/dc/dcmitype/">
	<!ENTITY fibo-fnd-utl-av "https://spec.edmcouncil.org/fibo/ontology/FND/Utilities/AnnotationVocabulary/">
	<!ENTITY foaf "http://xmlns.com/foaf/0.1/">
	<!ENTITY ns "http://creativecommons.org/ns#">
	<!ENTITY owl "http://www.w3.org/2002/07/owl#">
	<!ENTITY rdf "http://www.w3.org/1999/02/22-rdf-syntax-ns#">
	<!ENTITY rdfa "http://www.w3.org/ns/rdfa#">
	<!ENTITY rdfs "http://www.w3.org/2000/01/rdf-schema#">
	<!ENTITY skos "http://www.w3.org/2004/02/skos/core#">
	<!ENTITY sm "http://www.omg.org/techprocess/ab/SpecificationMetadata/">
	<!ENTITY vann "http://purl.org/vocab/vann/">
	<!ENTITY xsd "http://www.w3.org/2001/XMLSchema#">
]>
<rdf:RDF xml:base="https://spec.edmcouncil.org/auto/ontology/VC/VehicleCore/"
	xmlns="https://spec.edmcouncil.org/auto/ontology/VC/VehicleCore/"
	xmlns:auto-mo="https://spec.edmcouncil.org/auto/ontology/MO/MiddleOntology/"
	xmlns:auto-vc="https://spec.edmcouncil.org/auto/ontology/VC/VehicleCore/"
	xmlns:dc="http://purl.org/dc/elements/1.1/"
	xmlns:dct="http://purl.org/dc/terms/"
	xmlns:dctype="http://purl.org/dc/dcmitype/"
	xmlns:fibo-fnd-utl-av="https://spec.edmcouncil.org/fibo/ontology/FND/Utilities/AnnotationVocabulary/"
	xmlns:foaf="http://xmlns.com/foaf/0.1/"
	xmlns:ns="http://creativecommons.org/ns#"
	xmlns:owl="http://www.w3.org/2002/07/owl#"
	xmlns:rdf="http://www.w3.org/1999/02/22-rdf-syntax-ns#"
	xmlns:rdfa="http://www.w3.org/ns/rdfa#"
	xmlns:rdfs="http://www.w3.org/2000/01/rdf-schema#"
	xmlns:skos="http://www.w3.org/2004/02/skos/core#"
	xmlns:sm="http://www.omg.org/techprocess/ab/SpecificationMetadata/"
	xmlns:vann="http://purl.org/vocab/vann/"
	xmlns:xsd="http://www.w3.org/2001/XMLSchema#">
	
	<owl:Ontology rdf:about="https://spec.edmcouncil.org/auto/ontology/VC/VehicleCore/">
		<rdfs:label>Vehicle core ontology (VC)</rdfs:label>
		<dc:contributor>Robert Trypuz</dc:contributor>
		<dct:abstract xml:lang="en">The Vehicle Core (VC) module focuses on the core concepts related to vehicles&apos; types, structure and configuration.

It contains many classes and properties extracted from:
- the automotive extension of schema.org (https://schema.org/docs/automotive.html). 
- the Volkswagen Vehicles Ontology created by Martin Hepp with the contribution of Charles Sandeman-Craik, Tribal DDB; Chris Jenkins, Tribal DDB; Tim Redding, Tribal DDB; Yago Otero, Tribal DDB; William Greenly, Tribal DDB; Robin Dingle, Volkswagen UK (see https://lov.linkeddata.es/dataset/lov/vocabs/vvo) and available under the Creative Commons Attribution 3.0 Unported license (see http://creativecommons.org/licenses/by/3.0/). 
- the Car Options Ontology (COO) created by Martin Hepp, Hepp Research GmbH, with the contribution of Charles Sandeman-Craik, Tribal DDB; Chris Jenkins, Tribal DDB; Tim Redding, Tribal DDB; Yago Otero, Tribal DDB; William Greenly, Tribal DDB; Robin Dingle, Volkswagen UK (see https://lov.linkeddata.es/dataset/lov/vocabs/coo) and available under the Creative Commons Attribution 3.0 Unported license (see http://creativecommons.org/licenses/by/3.0/).
- the Vehicle Emissions Ontology (VEO) created by Bojan Najdenov, with the contribution of Milos Jovanovik (see https://lov.linkeddata.es/dataset/lov/vocabs/veo) and available under the Creative Commons Attribution 3.0 Unported license (see http://creativecommons.org/licenses/by/3.0/).
- the Car Ontology (CAR) created by Lihua Zhao and Yutaka Sasaki at the Computational Intelligence Laboratory, Toyota Technological Institute, Nagoya, Japan (see https://www.toyota-ti.ac.jp/Lab/Denshi/COIN/Ontology/TTICore-0.03/) and published by the Toyota Technological Institute Smart Vehicle Research Project. MAP, as created by the Computational Intelligence Laboratory, is available under the Creative Commons - Attribution-NonCommercial-ShareAlike
4.0 International (http://creativecommons.org/licenses/by-nc-sa/4.0/).
- the Used Cars Ontology (UCO) (created by Hepp Research GmbH and Makolab SA (see http://ontologies.makolab.com/uco/ns.html) and available under the Creative Commons Attribution 3.0 Unported license; see http://creativecommons.org/licenses/by/3.0/)
- the Vehicle Sales Ontology (VSO) (created by Martin Hepp (see https://lov.linkeddata.es/dataset/lov/vocabs/vso) and available under the Creative Commons Attribution 3.0 Unported license; see http://creativecommons.org/licenses/by/3.0/).</dct:abstract>
		<sm:contentLanguage rdf:datatype="&xsd;anyURI">http://www.w3.org/standards/techs/owl#w3c_all</sm:contentLanguage>
		<sm:copyright>Copyright (c) 2021 EDM Council, Inc.</sm:copyright>
		<sm:fileAbbreviation>auto-vc-vc</sm:fileAbbreviation>
		<sm:filename>VehicleCore.rdf</sm:filename>
		<owl:imports rdf:resource="https://spec.edmcouncil.org/auto/ontology/MO/MiddleOntology/"/>
		<owl:imports rdf:resource="https://spec.edmcouncil.org/fibo/ontology/FND/Utilities/AnnotationVocabulary/"/>
		<owl:versionIRI rdf:resource="https://spec.edmcouncil.org/auto/ontology/VC/VehicleCore/"/>
		<fibo-fnd-utl-av:hasMaturityLevel rdf:resource="&fibo-fnd-utl-av;Provisional"/>
	</owl:Ontology>
	
	<owl:AnnotationProperty rdf:about="&dc;contributor">
	</owl:AnnotationProperty>
	
	<owl:AnnotationProperty rdf:about="&dct;abstract">
	</owl:AnnotationProperty>
	
	<owl:AnnotationProperty rdf:about="&dct;isPartOf">
	</owl:AnnotationProperty>
	
	<owl:AnnotationProperty rdf:about="&dct;source">
	</owl:AnnotationProperty>
	
	<owl:AnnotationProperty rdf:about="&sm;contentLanguage">
	</owl:AnnotationProperty>
	
	<owl:AnnotationProperty rdf:about="&sm;copyright">
	</owl:AnnotationProperty>
	
	<owl:AnnotationProperty rdf:about="&sm;directSource">
	</owl:AnnotationProperty>
	
	<owl:AnnotationProperty rdf:about="&sm;fileAbbreviation">
	</owl:AnnotationProperty>
	
	<owl:AnnotationProperty rdf:about="&sm;filename">
	</owl:AnnotationProperty>
	
	<owl:AnnotationProperty rdf:about="&skos;definition">
	</owl:AnnotationProperty>
	
	<owl:Class rdf:about="&auto-mo;GenericallyDependentContinuant">
		<rdfs:label xml:lang="en">generically dependent continuant</rdfs:label>
	</owl:Class>
	
	<owl:Class rdf:about="&auto-mo;IndependentContinuant">
		<rdfs:label xml:lang="en">independent continuant</rdfs:label>
	</owl:Class>
	
	<owl:Class rdf:about="&auto-mo;Location">
		<rdfs:label xml:lang="en">location</rdfs:label>
	</owl:Class>
	
	<owl:Class rdf:about="&auto-mo;Model">
		<rdfs:label xml:lang="en">model</rdfs:label>
	</owl:Class>
	
	<owl:Class rdf:about="&auto-mo;NumericalValue">
		<rdfs:label xml:lang="en">numerical value</rdfs:label>
	</owl:Class>
	
	<owl:Class rdf:about="&auto-mo;Object">
		<rdfs:label xml:lang="en">object</rdfs:label>
	</owl:Class>
	
	<owl:Class rdf:about="&auto-mo;Organization">
		<rdfs:label xml:lang="en">organization</rdfs:label>
	</owl:Class>
	
	<owl:Class rdf:about="&auto-mo;Person">
		<rdfs:label xml:lang="en">person</rdfs:label>
		<rdfs:comment xml:lang="en">Within the context of this manual, a fetus is considered part of a pregnant woman rather than a separate individual. After death, a human body is not considered to be a person.</rdfs:comment>
		<skos:definition xml:lang="en">Any living human.</skos:definition>
		<fibo-fnd-utl-av:adaptedFrom>ANSI D.16-2017, section 2.1.1</fibo-fnd-utl-av:adaptedFrom>
	</owl:Class>
	
	<owl:Class rdf:about="&auto-mo;PostalAddress">
		<rdfs:label xml:lang="en">postal address</rdfs:label>
	</owl:Class>
	
	<owl:Class rdf:about="&auto-mo;Process">
		<rdfs:label xml:lang="en">process</rdfs:label>
	</owl:Class>
	
	<owl:Class rdf:about="&auto-mo;PropertyValue">
		<rdfs:subClassOf>
			<owl:Restriction>
				<owl:onProperty rdf:resource="&auto-vc;propertyID"/>
				<owl:minCardinality rdf:datatype="&xsd;nonNegativeInteger">0</owl:minCardinality>
			</owl:Restriction>
		</rdfs:subClassOf>
		<rdfs:subClassOf>
			<owl:Restriction>
				<owl:onProperty rdf:resource="&auto-vc;propertyName"/>
				<owl:minCardinality rdf:datatype="&xsd;nonNegativeInteger">0</owl:minCardinality>
			</owl:Restriction>
		</rdfs:subClassOf>
		<rdfs:subClassOf>
			<owl:Restriction>
				<owl:onProperty rdf:resource="&auto-vc;propertyValue"/>
				<owl:minCardinality rdf:datatype="&xsd;nonNegativeInteger">0</owl:minCardinality>
			</owl:Restriction>
		</rdfs:subClassOf>
		<rdfs:subClassOf>
			<owl:Restriction>
				<owl:onProperty rdf:resource="&auto-vc;unitText"/>
				<owl:minCardinality rdf:datatype="&xsd;nonNegativeInteger">0</owl:minCardinality>
			</owl:Restriction>
		</rdfs:subClassOf>
		<rdfs:subClassOf>
			<owl:Restriction>
				<owl:onProperty rdf:resource="&auto-vc;unitCode"/>
				<owl:minQualifiedCardinality rdf:datatype="&xsd;nonNegativeInteger">0</owl:minQualifiedCardinality>
				<owl:onDataRange rdf:resource="&xsd;string"/>
			</owl:Restriction>
		</rdfs:subClassOf>
		<rdfs:label xml:lang="en">property value</rdfs:label>
	</owl:Class>
	
	<owl:Class rdf:about="&auto-mo;QualitativeValue">
		<rdfs:label xml:lang="en">qualitative value</rdfs:label>
		<dct:isPartOf rdf:resource="http://auto.schema.org"/>
		<dct:source rdf:resource="http://www.w3.org/wiki/WebSchemas/SchemaDotOrgSources#Automotive_Ontology_Working_Group"/>
		<sm:directSource rdf:resource="https://schema.org/QualitativeValue"/>
		<skos:definition xml:lang="en">a predefined value for a product characteristic, e.g. the power cord plug type &apos;US&apos; or the garment sizes &apos;S&apos;, &apos;M&apos;, &apos;L&apos;, and &apos;XL&apos;</skos:definition>
	</owl:Class>
	
	<owl:Class rdf:about="&auto-mo;Quality">
		<rdfs:label xml:lang="en">quality</rdfs:label>
	</owl:Class>
	
	<owl:Class rdf:about="&auto-mo;QuantitativeValue">
		<rdfs:subClassOf>
			<owl:Class>
				<owl:intersectionOf rdf:parseType="Collection">
					<owl:Restriction>
						<owl:onProperty rdf:resource="&auto-vc;rotationalSpeedReference"/>
						<owl:onClass rdf:resource="&auto-mo;QuantitativeValue"/>
						<owl:minQualifiedCardinality rdf:datatype="&xsd;nonNegativeInteger">0</owl:minQualifiedCardinality>
					</owl:Restriction>
					<owl:Restriction>
						<owl:onProperty rdf:resource="&auto-vc;rotationalSpeedReference"/>
						<owl:onClass rdf:resource="&auto-mo;QuantitativeValue"/>
						<owl:maxQualifiedCardinality rdf:datatype="&xsd;nonNegativeInteger">1</owl:maxQualifiedCardinality>
					</owl:Restriction>
				</owl:intersectionOf>
			</owl:Class>
		</rdfs:subClassOf>
		<rdfs:subClassOf>
			<owl:Class>
				<owl:intersectionOf rdf:parseType="Collection">
					<owl:Restriction>
						<owl:onProperty rdf:resource="&auto-vc;refersToTrafficPattern"/>
						<owl:onClass rdf:resource="&auto-vc;TrafficPattern"/>
						<owl:minQualifiedCardinality rdf:datatype="&xsd;nonNegativeInteger">0</owl:minQualifiedCardinality>
					</owl:Restriction>
					<owl:Restriction>
						<owl:onProperty rdf:resource="&auto-vc;refersToTrafficPattern"/>
						<owl:onClass rdf:resource="&auto-vc;TrafficPattern"/>
						<owl:maxQualifiedCardinality rdf:datatype="&xsd;nonNegativeInteger">1</owl:maxQualifiedCardinality>
					</owl:Restriction>
				</owl:intersectionOf>
			</owl:Class>
		</rdfs:subClassOf>
		<rdfs:label xml:lang="en">quantitative value</rdfs:label>
		<dct:isPartOf rdf:resource="http://auto.schema.org"/>
		<dct:source rdf:resource="http://www.w3.org/wiki/WebSchemas/SchemaDotOrgSources#Automotive_Ontology_Working_Group"/>
		<sm:directSource rdf:resource="https://schema.org/QuantitativeValue"/>
		<skos:definition xml:lang="en">a point value or interval for product characteristics and other purposes</skos:definition>
	</owl:Class>
	
	<owl:Class rdf:about="&auto-mo;QuantitativeValueFloat">
		<rdfs:subClassOf>
			<owl:Class>
				<owl:intersectionOf rdf:parseType="Collection">
					<owl:Restriction>
						<owl:onProperty rdf:resource="&auto-vc;referenceDistance"/>
						<owl:onClass rdf:resource="&auto-mo;QuantitativeValue"/>
						<owl:minQualifiedCardinality rdf:datatype="&xsd;nonNegativeInteger">0</owl:minQualifiedCardinality>
					</owl:Restriction>
					<owl:Restriction>
						<owl:onProperty rdf:resource="&auto-vc;referenceDistance"/>
						<owl:onClass rdf:resource="&auto-mo;QuantitativeValue"/>
						<owl:maxQualifiedCardinality rdf:datatype="&xsd;nonNegativeInteger">1</owl:maxQualifiedCardinality>
					</owl:Restriction>
				</owl:intersectionOf>
			</owl:Class>
		</rdfs:subClassOf>
		<rdfs:subClassOf>
			<owl:Class>
				<owl:intersectionOf rdf:parseType="Collection">
					<owl:Restriction>
						<owl:onProperty rdf:resource="&auto-vc;referenceFuelQuantity"/>
						<owl:onClass rdf:resource="&auto-vc;FuelQuantity"/>
						<owl:minQualifiedCardinality rdf:datatype="&xsd;nonNegativeInteger">0</owl:minQualifiedCardinality>
					</owl:Restriction>
					<owl:Restriction>
						<owl:onProperty rdf:resource="&auto-vc;referenceFuelQuantity"/>
						<owl:onClass rdf:resource="&auto-vc;FuelQuantity"/>
						<owl:maxQualifiedCardinality rdf:datatype="&xsd;nonNegativeInteger">1</owl:maxQualifiedCardinality>
					</owl:Restriction>
				</owl:intersectionOf>
			</owl:Class>
		</rdfs:subClassOf>
		<rdfs:label xml:lang="en">quantitative value float</rdfs:label>
	</owl:Class>
	
	<owl:Class rdf:about="&auto-mo;QuantitativeValueInteger">
	</owl:Class>
	
	<owl:Class rdf:about="&auto-mo;Role">
		<rdfs:label xml:lang="en">role</rdfs:label>
	</owl:Class>
	
	<owl:Class rdf:about="&auto-mo;TextValue">
		<rdfs:label xml:lang="en">text value</rdfs:label>
	</owl:Class>
	
	<owl:Class rdf:about="&auto-mo;ValueSpace">
		<rdfs:label xml:lang="en">value space</rdfs:label>
	</owl:Class>
	
	<owl:DatatypeProperty rdf:about="&auto-mo;datatypeProductOrServiceProperty">
		<rdfs:label>datatype product or service property</rdfs:label>
	</owl:DatatypeProperty>
	
	<owl:DatatypeProperty rdf:about="&auto-mo;hasMaxValue">
		<rdfs:label>has max value</rdfs:label>
	</owl:DatatypeProperty>
	
	<owl:DatatypeProperty rdf:about="&auto-mo;hasMinValue">
		<rdfs:label>has min value</rdfs:label>
	</owl:DatatypeProperty>
	
	<owl:DatatypeProperty rdf:about="&auto-mo;hasUnitOfMeasurement">
		<rdfs:label>has unit of measurement</rdfs:label>
		<rdfs:domain rdf:resource="&auto-mo;QuantitativeValue"/>
	</owl:DatatypeProperty>
	
	<owl:ObjectProperty rdf:about="&auto-mo;valueReference">
		<rdfs:label>value reference</rdfs:label>
	</owl:ObjectProperty>
	
	<owl:NamedIndividual rdf:about="&auto-vc;0to100KMH">
		<rdf:type rdf:resource="&auto-vc;SpeedInterval"/>
		<rdfs:label xml:lang="en">0 to 100KMH</rdfs:label>
		<rdfs:isDefinedBy rdf:resource="http://purl.org/vso/ns"/>
		<skos:definition xml:lang="en">The speed interval from 0 to 100 km/h</skos:definition>
		<auto-mo:hasMaxValue rdf:datatype="&xsd;float">100.0</auto-mo:hasMaxValue>
		<auto-mo:hasMinValue rdf:datatype="&xsd;float">0.0</auto-mo:hasMinValue>
		<auto-mo:hasUnitOfMeasurement>KMH</auto-mo:hasUnitOfMeasurement>
	</owl:NamedIndividual>
	
	<owl:NamedIndividual rdf:about="&auto-vc;0to60MPH">
		<rdf:type rdf:resource="&auto-vc;SpeedInterval"/>
		<rdfs:label xml:lang="en">0 to 60MPH</rdfs:label>
		<rdfs:isDefinedBy rdf:resource="http://purl.org/vso/ns"/>
		<skos:definition xml:lang="en">The speed interval from 0 to 60 mph</skos:definition>
		<auto-mo:hasMaxValue rdf:datatype="&xsd;float">60.0</auto-mo:hasMaxValue>
		<auto-mo:hasMinValue rdf:datatype="&xsd;float">0.0</auto-mo:hasMinValue>
		<auto-mo:hasUnitOfMeasurement>HM</auto-mo:hasUnitOfMeasurement>
	</owl:NamedIndividual>
	
	<owl:NamedIndividual rdf:about="&auto-vc;1GLI">
		<rdf:type rdf:resource="&auto-vc;FuelQuantity"/>
		<rdfs:label xml:lang="en">1GLI</rdfs:label>
		<rdfs:isDefinedBy rdf:resource="http://purl.org/vso/ns"/>
		<skos:definition xml:lang="en">The fuel quantity of 1 British (imperial) gallon</skos:definition>
		<auto-mo:hasUnitOfMeasurement>GLI</auto-mo:hasUnitOfMeasurement>
	</owl:NamedIndividual>
	
	<owl:NamedIndividual rdf:about="&auto-vc;1GLL">
		<rdf:type rdf:resource="&auto-vc;FuelQuantity"/>
		<rdfs:label xml:lang="en">1GLL</rdfs:label>
		<rdfs:isDefinedBy rdf:resource="http://purl.org/vso/ns"/>
		<skos:definition xml:lang="en">The fuel quantity of 1 US gallon</skos:definition>
		<auto-mo:hasUnitOfMeasurement>GLL</auto-mo:hasUnitOfMeasurement>
	</owl:NamedIndividual>
	
	<owl:NamedIndividual rdf:about="&auto-vc;1LTR">
		<rdf:type rdf:resource="&auto-vc;FuelQuantity"/>
		<rdfs:label xml:lang="en">1LTR</rdfs:label>
		<rdfs:isDefinedBy rdf:resource="http://purl.org/vso/ns"/>
		<skos:definition xml:lang="en">The fuel quantity of 1 liter</skos:definition>
		<auto-mo:hasUnitOfMeasurement>LTR</auto-mo:hasUnitOfMeasurement>
	</owl:NamedIndividual>
	
	<owl:Class rdf:about="&auto-vc;AgriculturalCommodityTrailer">
		<rdfs:subClassOf rdf:resource="&auto-vc;FullTrailer"/>
		<rdfs:label xml:lang="en">agricultural commodity trailer</rdfs:label>
		<skos:definition xml:lang="en">trailer that is designed to transport bulk agricultural commodities in off-road harvesting sites and to a processing plant or storage location, as evidenced by skeletal construction that accommodates harvest containers, a maximum length of 28 feet, and an arrangement of air control lines and reservoirs that minimizes damage in field operations</skos:definition>
	</owl:Class>
	
	<owl:Class rdf:about="&auto-vc;Aircraft">
		<rdfs:subClassOf rdf:resource="&auto-vc;Vehicle"/>
		<rdfs:label xml:lang="en">aircraft</rdfs:label>
		<skos:definition xml:lang="en">A transport vehicle designed primarily for, or in use for, moving persons or property through the air from one place to another.</skos:definition>
		<fibo-fnd-utl-av:adaptedFrom>ANSI D.16-2017, section 2.1.5</fibo-fnd-utl-av:adaptedFrom>
	</owl:Class>
	
	<owl:NamedIndividual rdf:about="&auto-vc;AllWheelDriveConfiguration">
		<rdf:type rdf:resource="&auto-vc;DriveWheelConfigurationValue"/>
		<rdfs:label xml:lang="en">all-wheel drive</rdfs:label>
		<skos:definition xml:lang="en">All-wheel Drive is a transmission layout where the engine drives all four wheels.</skos:definition>
	</owl:NamedIndividual>
	
	<owl:Class rdf:about="&auto-vc;AudioAndNavigation">
		<rdfs:subClassOf rdf:resource="&auto-vc;ChoiceOrComponent"/>
		<rdfs:label xml:lang="en">audio and navigation choice or component</rdfs:label>
		<rdfs:isDefinedBy rdf:resource="http://purl.org/vvo/ns#"/>
		<skos:definition xml:lang="en">The class of audio and navigation choices or components (CD/DVD/SatNav, a &quot;MonoSelectGroup&quot; in automotive terminology), VW ID: 1</skos:definition>
	</owl:Class>
	
	<owl:NamedIndividual rdf:about="&auto-vc;AuthorizedDealer">
		<rdf:type rdf:resource="&auto-vc;BusinessEntityType"/>
		<rdfs:label xml:lang="en">authorized dealer</rdfs:label>
		<rdfs:isDefinedBy rdf:resource="http://purl.org/uco/ns#"/>
		<skos:definition xml:lang="en">An authorized dealer of the manufacturer of the respective vehicle</skos:definition>
	</owl:NamedIndividual>
	
	<owl:Class rdf:about="&auto-vc;Autocycle">
		<rdfs:subClassOf rdf:resource="&auto-vc;Motorcycle"/>
		<rdfs:label xml:lang="en">autocycle</rdfs:label>
		<skos:definition xml:lang="en">A large motorcycle with one rear wheel and two front wheels, with either a saddle and handlebars or seat (s) and a steering wheel, that can be fully enclosed, partially enclosed, or unenclosed.</skos:definition>
		<fibo-fnd-utl-av:adaptedFrom>ANSI D.16-2017, section 2.2.9.7</fibo-fnd-utl-av:adaptedFrom>
	</owl:Class>
	
	<owl:Class rdf:about="&auto-vc;BaseModel">
		<rdfs:subClassOf rdf:resource="&auto-mo;Model"/>
		<rdfs:subClassOf>
			<owl:Restriction>
				<owl:onProperty rdf:resource="&auto-vc;hasTrim"/>
				<owl:onClass rdf:resource="&auto-vc;Trim"/>
				<owl:minQualifiedCardinality rdf:datatype="&xsd;nonNegativeInteger">0</owl:minQualifiedCardinality>
			</owl:Restriction>
		</rdfs:subClassOf>
		<rdfs:label xml:lang="en">base model</rdfs:label>
		<rdfs:isDefinedBy rdf:resource="http://purl.org/coo/ns#"/>
		<owl:disjointWith rdf:resource="&auto-vc;ChoiceOrComponent"/>
		<owl:disjointWith rdf:resource="&auto-vc;CompleteCarModel"/>
		<owl:disjointWith rdf:resource="&auto-vc;ConfigurationInfo"/>
		<owl:disjointWith rdf:resource="&auto-vc;Derivative"/>
		<owl:disjointWith rdf:resource="&auto-vc;PropertySpecification"/>
		<owl:disjointWith rdf:resource="&auto-vc;SpecItemCollection"/>
		<owl:disjointWith rdf:resource="&auto-vc;Trim"/>
		<skos:definition xml:lang="en">A Base Model is an abstract entity specifying the basic features of a group of vehicles.

Examples: VW Golf, VW Polo, VW Passat</skos:definition>
	</owl:Class>
	
	<owl:Class rdf:about="&auto-vc;Bicycle">
		<rdfs:subClassOf rdf:resource="&auto-vc;Pedalcycle"/>
		<rdfs:label xml:lang="en">bicycle</rdfs:label>
		<rdfs:label xml:lang="pl">rower</rdfs:label>
		<rdfs:comment>QName: auto-vc-vc:Bicycle</rdfs:comment>
		<rdfs:comment xml:lang="pl">pojazd o szerokości nieprzekraczającej 0,9 m poruszany siłą mięśni osoby jadącej tym pojazdem; rower może być wyposażony w uruchamiany naciskiem na pedały pomocniczy napęd elektryczny zasilany prądem o napięciu nie wyższym niż 48 V o znamionowej mocy ciągłej nie większej niż 250 W, którego moc wyjściowa zmniejsza się stopniowo i spada do zera po przekroczeniu prędkości 25 km/h</rdfs:comment>
		<rdfs:isDefinedBy rdf:resource="http://purl.org/vso/ns"/>
		<rdfs:isDefinedBy rdf:resource="https://spec.edmcouncil.org/auto/ontology/VC/VehicleCore/"/>
		<rdfs:seeAlso rdf:resource="http://dbpedia.org/resource/Bicycle"/>
		<rdfs:seeAlso rdf:resource="http://en.wikipedia.org/wiki/Bicycle"/>
		<skos:definition xml:lang="en">a pedal-driven, human-powered, single-track vehicle, having two wheels attached to a frame, one behind the other. Some bicycles have a small combustion or electric engine that assists with the pedaling.</skos:definition>
		<fibo-fnd-utl-av:synonym xml:lang="en">bike</fibo-fnd-utl-av:synonym>
	</owl:Class>
	
	<owl:Class rdf:about="&auto-vc;Boat">
		<rdfs:subClassOf rdf:resource="&auto-vc;Watercraft"/>
		<rdfs:label xml:lang="en">boat</rdfs:label>
		<rdfs:isDefinedBy rdf:resource="http://purl.org/vso/ns"/>
		<rdfs:seeAlso rdf:resource="http://dbpedia.org/resource/Boat"/>
		<rdfs:seeAlso rdf:resource="http://en.wikipedia.org/wiki/Boat"/>
		<skos:definition xml:lang="en">a watercraft of modest size designed to float or plane, to provide passage across water</skos:definition>
	</owl:Class>
	
	<owl:Class rdf:about="&auto-vc;BoatTrailer">
		<rdfs:subClassOf rdf:resource="&auto-vc;FullTrailer"/>
		<rdfs:label xml:lang="en">boat trailer</rdfs:label>
		<skos:definition xml:lang="en">trailer designed with cradle-type mountings to transport a boat and configured to permit the launching of the boat from the rear of the trailer</skos:definition>
	</owl:Class>
	
	<owl:NamedIndividual rdf:about="&auto-vc;BodyStyle4X4">
		<rdf:type rdf:resource="&auto-vc;BodyStyleValue"/>
		<rdfs:label xml:lang="en">4 X 4</rdfs:label>
		<dct:source>vso:BodyStyleValue</dct:source>
		<rdfs:isDefinedBy rdf:resource="http://purl.org/vvo/ns#"/>
		<skos:definition xml:lang="en">Four-by-Four Vehicle, VW ID: 6</skos:definition>
		<auto-vc:hasID>6</auto-vc:hasID>
	</owl:NamedIndividual>
	
	<owl:NamedIndividual rdf:about="&auto-vc;BodyStyleCabriolet">
		<rdf:type rdf:resource="&auto-vc;BodyStyleValue"/>
		<rdfs:label xml:lang="en">cabriolet</rdfs:label>
		<dct:source>vso:BodyStyleValue</dct:source>
		<rdfs:isDefinedBy rdf:resource="http://purl.org/vvo/ns#"/>
		<skos:definition xml:lang="en">Cabriolet, VW ID: 4</skos:definition>
		<auto-vc:hasID>4</auto-vc:hasID>
	</owl:NamedIndividual>
	
	<owl:NamedIndividual rdf:about="&auto-vc;BodyStyleCoupe">
		<rdf:type rdf:resource="&auto-vc;BodyStyleValue"/>
		<rdfs:label xml:lang="en">coupe</rdfs:label>
		<dct:source>vso:BodyStyleValue</dct:source>
		<rdfs:isDefinedBy rdf:resource="http://purl.org/vvo/ns#"/>
		<skos:definition xml:lang="en">Coupe, VW ID: 7</skos:definition>
		<auto-vc:hasID>7</auto-vc:hasID>
	</owl:NamedIndividual>
	
	<owl:NamedIndividual rdf:about="&auto-vc;BodyStyleEstate">
		<rdf:type rdf:resource="&auto-vc;BodyStyleValue"/>
		<rdfs:label xml:lang="en">estate</rdfs:label>
		<dct:source>vso:BodyStyleValue</dct:source>
		<rdfs:isDefinedBy rdf:resource="http://purl.org/vvo/ns#"/>
		<skos:definition xml:lang="en">Estate, VW ID: 3</skos:definition>
		<auto-vc:hasID>3</auto-vc:hasID>
	</owl:NamedIndividual>
	
	<owl:NamedIndividual rdf:about="&auto-vc;BodyStyleHatchback">
		<rdf:type rdf:resource="&auto-vc;BodyStyleValue"/>
		<rdfs:label xml:lang="en">hatchback</rdfs:label>
		<dct:source>vso:BodyStyleValue</dct:source>
		<rdfs:isDefinedBy rdf:resource="http://purl.org/vvo/ns#"/>
		<skos:definition xml:lang="en">Hatchback, VW ID: 1</skos:definition>
		<auto-vc:hasID>1</auto-vc:hasID>
	</owl:NamedIndividual>
	
	<owl:NamedIndividual rdf:about="&auto-vc;BodyStyleMPV">
		<rdf:type rdf:resource="&auto-vc;BodyStyleValue"/>
		<rdfs:label xml:lang="en">MPV</rdfs:label>
		<dct:source>vso:BodyStyleValue</dct:source>
		<rdfs:isDefinedBy rdf:resource="http://purl.org/vvo/ns#"/>
		<skos:definition xml:lang="en">Multi-purpose Vehicle, VW ID: 5</skos:definition>
		<auto-vc:hasID>5</auto-vc:hasID>
	</owl:NamedIndividual>
	
	<owl:NamedIndividual rdf:about="&auto-vc;BodyStyleSaloon">
		<rdf:type rdf:resource="&auto-vc;BodyStyleValue"/>
		<rdfs:label xml:lang="en">saloon</rdfs:label>
		<dct:source>vso:BodyStyleValue</dct:source>
		<rdfs:isDefinedBy rdf:resource="http://purl.org/vvo/ns#"/>
		<skos:definition xml:lang="en">Saloon, VW ID: 2</skos:definition>
		<auto-vc:hasID>2</auto-vc:hasID>
	</owl:NamedIndividual>
	
	<owl:NamedIndividual rdf:about="&auto-vc;BodyStyleUnspecified">
		<rdf:type rdf:resource="&auto-vc;BodyStyleValue"/>
		<rdfs:label xml:lang="en">unspecified</rdfs:label>
		<dct:source>vso:BodyStyleValue</dct:source>
		<rdfs:isDefinedBy rdf:resource="http://purl.org/vvo/ns#"/>
		<skos:definition xml:lang="en">Unspecified, VW ID: 0</skos:definition>
		<auto-vc:hasID>0</auto-vc:hasID>
	</owl:NamedIndividual>
	
	<owl:Class rdf:about="&auto-vc;BodyStyleValue">
		<rdfs:subClassOf rdf:resource="&auto-mo;QualitativeValue"/>
		<rdfs:label xml:lang="en">body style value</rdfs:label>
		<rdfs:comment xml:lang="en">You can safely use any reasonable DBPedia URI, e.g. 
  http://dbpedia.org/resource/Convertible
  http://dbpedia.org/resource/Hatchback
  http://dbpedia.org/resource/Station_wagon
  http://dbpedia.org/resource/Sport_utility_vehicle
  http://dbpedia.org/resource/Roadster</rdfs:comment>
		<rdfs:isDefinedBy rdf:resource="http://purl.org/vso/ns"/>
		<skos:definition xml:lang="en">a value indicating the body style of a vehicle</skos:definition>
	</owl:Class>
	
	<owl:Class rdf:about="&auto-vc;Bus">
		<rdfs:subClassOf rdf:resource="&auto-vc;LargeSpecialVehicle"/>
		<rdfs:subClassOf>
			<owl:Restriction>
				<owl:onProperty rdf:resource="&auto-vc;acrissCode"/>
				<owl:minQualifiedCardinality rdf:datatype="&xsd;nonNegativeInteger">0</owl:minQualifiedCardinality>
				<owl:onDataRange rdf:resource="&xsd;string"/>
			</owl:Restriction>
		</rdfs:subClassOf>
		<rdfs:label xml:lang="pl">autobus</rdfs:label>
		<rdfs:label xml:lang="en">bus</rdfs:label>
		<rdfs:comment xml:lang="en">A bus (also omnibus or autobus) is a road vehicle designed to carry passengers. Buses have a capacity as high as 300 passengers and are widely used for public transportation. 
Coaches are luxury busses, usually in service for long distance travel.</rdfs:comment>
		<rdfs:comment>QName: auto-vc-vc:BusOrCoach</rdfs:comment>
		<rdfs:comment xml:lang="pl">pojazd samochodowy przeznaczony konstrukcyjnie do przewozu więcej niż 9 osób łącznie z kierowcą</rdfs:comment>
		<dct:isPartOf rdf:resource="http://auto.schema.org"/>
		<dct:source rdf:resource="http://www.w3.org/wiki/WebSchemas/SchemaDotOrgSources#Automotive_Ontology_Working_Group"/>
		<sm:directSource rdf:resource="https://schema.org/BusOrCoach"/>
		<rdfs:isDefinedBy rdf:resource="http://purl.org/vso/ns"/>
		<rdfs:isDefinedBy rdf:resource="https://spec.edmcouncil.org/auto/ontology/VC/VehicleCore/"/>
		<rdfs:seeAlso rdf:resource="http://dbpedia.org/page/Coach_%28vehicle%29"/>
		<rdfs:seeAlso rdf:resource="http://dbpedia.org/resource/Bus"/>
		<rdfs:seeAlso rdf:resource="http://en.wikipedia.org/wiki/Bus"/>
		<rdfs:seeAlso rdf:resource="http://en.wikipedia.org/wiki/Coach_%28vehicle%29"/>
		<skos:definition xml:lang="en">A motor vehicle with seating for transporting nine or more persons, including the driver.</skos:definition>
		<skos:definition xml:lang="en">a road vehicle designed to carry passengers. Coaches are luxury busses, usually in service for long distance travel</skos:definition>
		<fibo-fnd-utl-av:adaptedFrom>ANSI D.16-2017, section 2.2.10</fibo-fnd-utl-av:adaptedFrom>
		<fibo-fnd-utl-av:synonym xml:lang="en">autobus</fibo-fnd-utl-av:synonym>
		<fibo-fnd-utl-av:synonym xml:lang="en">coach</fibo-fnd-utl-av:synonym>
		<fibo-fnd-utl-av:synonym xml:lang="en">omnibus</fibo-fnd-utl-av:synonym>
	</owl:Class>
	
	<owl:NamedIndividual rdf:about="&auto-vc;Business">
		<rdf:type rdf:resource="&auto-vc;CarUsageType"/>
		<rdfs:label xml:lang="en">business</rdfs:label>
		<rdfs:isDefinedBy rdf:resource="http://purl.org/uco/ns#"/>
		<skos:definition xml:lang="en">The usage of a vehicle for general business purposes, i.e. excluding usages like as a taxi, rental car, or driving instructions.</skos:definition>
	</owl:NamedIndividual>
	
	<owl:Class rdf:about="&auto-vc;BusinessEntity">
		<rdfs:subClassOf rdf:resource="&auto-mo;IndependentContinuant"/>
		<rdfs:label xml:lang="en">business entity</rdfs:label>
		<owl:equivalentClass>
			<owl:Class>
				<owl:unionOf rdf:parseType="Collection">
					<rdf:Description rdf:about="&auto-mo;Organization">
					</rdf:Description>
					<rdf:Description rdf:about="&auto-mo;Person">
					</rdf:Description>
				</owl:unionOf>
			</owl:Class>
		</owl:equivalentClass>
		<skos:definition xml:lang="en">entity that is formed and administered as per commercial law in order to engage in business activities</skos:definition>
	</owl:Class>
	
	<owl:Class rdf:about="&auto-vc;BusinessEntityType">
		<rdfs:subClassOf rdf:resource="&auto-mo;QualitativeValue"/>
		<rdfs:label xml:lang="en">business entity type</rdfs:label>
		<skos:definition xml:lang="en">type of a business entity</skos:definition>
	</owl:Class>
	
	<owl:Class rdf:about="&auto-vc;Canoe">
		<rdfs:subClassOf rdf:resource="&auto-vc;Boat"/>
		<rdfs:label xml:lang="en">canoe</rdfs:label>
		<rdfs:isDefinedBy rdf:resource="http://purl.org/vso/ns"/>
		<rdfs:seeAlso rdf:resource="http://dbpedia.org/resource/Canoe"/>
		<rdfs:seeAlso rdf:resource="http://en.wikipedia.org/wiki/Canoe"/>
		<skos:definition xml:lang="en">a small narrow boat, typically human-powered, though it may also be powered by sails or small electric or gas motors</skos:definition>
	</owl:Class>
	
	<owl:Class rdf:about="&auto-vc;Car">
		<rdfs:subClassOf rdf:resource="&auto-vc;MotorizedRoadVehicle"/>
		<rdfs:subClassOf>
			<owl:Restriction>
				<owl:onProperty rdf:resource="&auto-vc;acrissCode"/>
				<owl:minQualifiedCardinality rdf:datatype="&xsd;nonNegativeInteger">0</owl:minQualifiedCardinality>
				<owl:onDataRange rdf:resource="&xsd;string"/>
			</owl:Restriction>
		</rdfs:subClassOf>
		<rdfs:subClassOf>
			<owl:Restriction>
				<owl:onProperty rdf:resource="&auto-vc;bodyStyle"/>
				<owl:onClass rdf:resource="&auto-vc;BodyStyleValue"/>
				<owl:qualifiedCardinality rdf:datatype="&xsd;nonNegativeInteger">1</owl:qualifiedCardinality>
			</owl:Restriction>
		</rdfs:subClassOf>
		<rdfs:label xml:lang="en">automobile</rdfs:label>
		<rdfs:label xml:lang="en">car</rdfs:label>
		<rdfs:label xml:lang="pl">samochód</rdfs:label>
		<rdfs:comment>Automobiles may be classified by size or weight, or both. Size classification is based on wheelbase. Weight classification is based on curb weight, the weight of an automobile with standard equipment and a full complement of fuel and other fluids, but with no load of persons or property. Before classification, wheelbase should be rounded to the nearest inch and curb weight should be rounded to the nearest 100 pounds.</rdfs:comment>
		<rdfs:comment>QName: auto-vc-vc:Car</rdfs:comment>
		<dct:isPartOf rdf:resource="http://auto.schema.org"/>
		<dct:source rdf:resource="http://www.w3.org/wiki/WebSchemas/SchemaDotOrgSources#Automotive_Ontology_Working_Group"/>
		<sm:directSource rdf:resource="https://schema.org/Car"/>
		<rdfs:isDefinedBy rdf:resource="http://purl.org/vso/ns"/>
		<rdfs:isDefinedBy rdf:resource="https://spec.edmcouncil.org/auto/ontology/VC/VehicleCore/"/>
		<rdfs:seeAlso rdf:resource="http://dbpedia.org/resource/Automobile"/>
		<rdfs:seeAlso rdf:resource="http://en.wikipedia.org/wiki/Automobile"/>
		<skos:definition xml:lang="en">A motor vehicle other than a motorcycle, utility vehicle or low speed vehicle consisting of a transport device typically designed for carrying eight or fewer persons.</skos:definition>
		<skos:definition xml:lang="en">a wheeled motor vehicle used for transporting passengers, which also carries its own engine or motor</skos:definition>
		<skos:definition xml:lang="en">a wheeled, self-powered motor vehicle used for transportation</skos:definition>
		<fibo-fnd-utl-av:adaptedFrom>ANSI D.16-2017, section 2.2.12</fibo-fnd-utl-av:adaptedFrom>
	</owl:Class>
	
	<owl:NamedIndividual rdf:about="&auto-vc;CarSharing">
		<rdf:type rdf:resource="&auto-vc;CarUsageType"/>
		<rdfs:label xml:lang="en">car sharing</rdfs:label>
		<rdfs:isDefinedBy rdf:resource="http://purl.org/uco/ns#"/>
		<skos:definition xml:lang="en">The usage of a vehicle for car sharing networks</skos:definition>
	</owl:NamedIndividual>
	
	<owl:Class rdf:about="&auto-vc;CarUsageType">
		<rdfs:subClassOf rdf:resource="&auto-mo;QualitativeValue"/>
		<rdfs:label xml:lang="en">car usage</rdfs:label>
		<dct:isPartOf rdf:resource="http://auto.schema.org"/>
		<dct:source rdf:resource="http://www.w3.org/wiki/WebSchemas/SchemaDotOrgSources#Automotive_Ontology_Working_Group"/>
		<sm:directSource rdf:resource="https://schema.org/CarUsageType"/>
		<skos:definition xml:lang="en">a special usage of a car, e.g. commercial rental, driving school, or as a taxi</skos:definition>
	</owl:Class>
	
	<owl:Class rdf:about="&auto-vc;CargoVan">
		<rdfs:subClassOf rdf:resource="&auto-vc;Van"/>
		<rdfs:label xml:lang="en">cargo van</rdfs:label>
		<skos:definition xml:lang="en">Any van where the area behind the driver or cab is designed for transporting cargo or operated for general commercial use.</skos:definition>
		<fibo-fnd-utl-av:adaptedFrom>ANSI D.16-2017, section 2.2.14.2</fibo-fnd-utl-av:adaptedFrom>
	</owl:Class>
	
	<owl:NamedIndividual rdf:about="&auto-vc;Carport">
		<rdf:type rdf:resource="&auto-vc;ParkingType"/>
		<rdfs:label xml:lang="en">carport</rdfs:label>
		<rdfs:isDefinedBy rdf:resource="http://purl.org/uco/ns#"/>
		<skos:definition xml:lang="en">The parking of a vehicle under a protective roof, e.g. in a carport</skos:definition>
	</owl:NamedIndividual>
	
	<owl:Class rdf:about="&auto-vc;CharterBus">
		<rdfs:subClassOf rdf:resource="&auto-vc;Bus"/>
		<rdfs:label xml:lang="en">charter bus</rdfs:label>
		<skos:definition xml:lang="en">A bus providing contract service for a group tour or outing, usually on a round-trip basis.</skos:definition>
		<fibo-fnd-utl-av:adaptedFrom>ANSI D.16-2017, section 2.2.10.5</fibo-fnd-utl-av:adaptedFrom>
	</owl:Class>
	
	<owl:Class rdf:about="&auto-vc;Check">
		<rdfs:subClassOf rdf:resource="&auto-mo;Process"/>
		<rdfs:subClassOf>
			<owl:Restriction>
				<owl:onProperty rdf:resource="&auto-vc;carriedOutBy"/>
				<owl:onClass>
					<owl:Class>
						<owl:unionOf rdf:parseType="Collection">
							<rdf:Description rdf:about="&auto-mo;Organization">
							</rdf:Description>
							<rdf:Description rdf:about="&auto-mo;Person">
							</rdf:Description>
							<rdf:Description rdf:about="&auto-vc;BusinessEntityType">
							</rdf:Description>
						</owl:unionOf>
					</owl:Class>
				</owl:onClass>
				<owl:minQualifiedCardinality rdf:datatype="&xsd;nonNegativeInteger">0</owl:minQualifiedCardinality>
			</owl:Restriction>
		</rdfs:subClassOf>
		<rdfs:label xml:lang="en">check</rdfs:label>
		<rdfs:isDefinedBy rdf:resource="http://purl.org/uco/ns#"/>
		<skos:definition xml:lang="en">a mandatory or optional technical inspection, e.g. the MOT, a vendor-specific certification of used cars, etc.</skos:definition>
	</owl:Class>
	
	<owl:Class rdf:about="&auto-vc;ChoiceOrComponent">
		<rdfs:subClassOf rdf:resource="&auto-mo;GenericallyDependentContinuant"/>
		<rdfs:subClassOf rdf:resource="&auto-mo;Model"/>
		<rdfs:subClassOf>
			<owl:Class>
				<owl:intersectionOf rdf:parseType="Collection">
					<owl:Restriction>
						<owl:onProperty rdf:resource="&auto-vc;priceModifier"/>
						<owl:onClass rdf:resource="&auto-vc;RelativePriceSpecification"/>
						<owl:minQualifiedCardinality rdf:datatype="&xsd;nonNegativeInteger">0</owl:minQualifiedCardinality>
					</owl:Restriction>
					<owl:Restriction>
						<owl:onProperty rdf:resource="&auto-vc;priceModifier"/>
						<owl:onClass rdf:resource="&auto-vc;RelativePriceSpecification"/>
						<owl:maxQualifiedCardinality rdf:datatype="&xsd;nonNegativeInteger">1</owl:maxQualifiedCardinality>
					</owl:Restriction>
				</owl:intersectionOf>
			</owl:Class>
		</rdfs:subClassOf>
		<rdfs:subClassOf>
			<owl:Class>
				<owl:intersectionOf rdf:parseType="Collection">
					<owl:Restriction>
						<owl:onProperty rdf:resource="&auto-vc;displayPos"/>
						<owl:minQualifiedCardinality rdf:datatype="&xsd;nonNegativeInteger">0</owl:minQualifiedCardinality>
						<owl:onDataRange rdf:resource="&xsd;int"/>
					</owl:Restriction>
					<owl:Restriction>
						<owl:onProperty rdf:resource="&auto-vc;displayPos"/>
						<owl:maxQualifiedCardinality rdf:datatype="&xsd;nonNegativeInteger">1</owl:maxQualifiedCardinality>
						<owl:onDataRange rdf:resource="&xsd;int"/>
					</owl:Restriction>
				</owl:intersectionOf>
			</owl:Class>
		</rdfs:subClassOf>
		<rdfs:subClassOf>
			<owl:Class>
				<owl:intersectionOf rdf:parseType="Collection">
					<owl:Restriction>
						<owl:onProperty rdf:resource="&auto-vc;productCode"/>
						<owl:minQualifiedCardinality rdf:datatype="&xsd;nonNegativeInteger">0</owl:minQualifiedCardinality>
						<owl:onDataRange rdf:resource="&xsd;string"/>
					</owl:Restriction>
					<owl:Restriction>
						<owl:onProperty rdf:resource="&auto-vc;productCode"/>
						<owl:maxQualifiedCardinality rdf:datatype="&xsd;nonNegativeInteger">1</owl:maxQualifiedCardinality>
						<owl:onDataRange rdf:resource="&xsd;string"/>
					</owl:Restriction>
				</owl:intersectionOf>
			</owl:Class>
		</rdfs:subClassOf>
		<rdfs:subClassOf>
			<owl:Restriction>
				<owl:onProperty rdf:resource="&auto-vc;compatibleWith"/>
				<owl:onClass rdf:resource="&auto-vc;ChoiceOrComponent"/>
				<owl:minQualifiedCardinality rdf:datatype="&xsd;nonNegativeInteger">0</owl:minQualifiedCardinality>
			</owl:Restriction>
		</rdfs:subClassOf>
		<rdfs:subClassOf>
			<owl:Restriction>
				<owl:onProperty rdf:resource="&auto-vc;dependsOn"/>
				<owl:onClass rdf:resource="&auto-vc;ChoiceOrComponent"/>
				<owl:minQualifiedCardinality rdf:datatype="&xsd;nonNegativeInteger">0</owl:minQualifiedCardinality>
			</owl:Restriction>
		</rdfs:subClassOf>
		<rdfs:subClassOf>
			<owl:Restriction>
				<owl:onProperty rdf:resource="&auto-vc;includes"/>
				<owl:onClass rdf:resource="&auto-vc;ChoiceOrComponent"/>
				<owl:minQualifiedCardinality rdf:datatype="&xsd;nonNegativeInteger">0</owl:minQualifiedCardinality>
			</owl:Restriction>
		</rdfs:subClassOf>
		<rdfs:subClassOf>
			<owl:Restriction>
				<owl:onProperty rdf:resource="&auto-vc;incompatibleWith"/>
				<owl:onClass rdf:resource="&auto-vc;ChoiceOrComponent"/>
				<owl:minQualifiedCardinality rdf:datatype="&xsd;nonNegativeInteger">0</owl:minQualifiedCardinality>
			</owl:Restriction>
		</rdfs:subClassOf>
		<rdfs:subClassOf>
			<owl:Restriction>
				<owl:onProperty rdf:resource="&auto-vc;featureOverride"/>
				<owl:onClass rdf:resource="&auto-vc;PropertySpecification"/>
				<owl:minQualifiedCardinality rdf:datatype="&xsd;nonNegativeInteger">0</owl:minQualifiedCardinality>
			</owl:Restriction>
		</rdfs:subClassOf>
		<rdfs:label xml:lang="en">choice or component</rdfs:label>
		<rdfs:isDefinedBy rdf:resource="http://purl.org/coo/ns#"/>
		<owl:disjointWith rdf:resource="&auto-vc;CompleteCarModel"/>
		<owl:disjointWith rdf:resource="&auto-vc;ConfigurationInfo"/>
		<owl:disjointWith rdf:resource="&auto-vc;Derivative"/>
		<owl:disjointWith rdf:resource="&auto-vc;PropertySpecification"/>
		<owl:disjointWith rdf:resource="&auto-vc;SpecItemCollection"/>
		<owl:disjointWith rdf:resource="&auto-vc;Trim"/>
		<skos:definition xml:lang="en">A Choice or Component is a component (e.g. engine), add-on, feature (color &quot;ocean blue&quot;), or service that can be chosen to be part of a final vehicle configuration.
  
Example: Engine 1.6 l TDI, color ocean blue, trailer hitch</skos:definition>
	</owl:Class>
	
	<owl:NamedIndividual rdf:about="&auto-vc;Combined">
		<rdf:type rdf:resource="&auto-vc;TrafficPattern"/>
		<rdfs:label xml:lang="en">combined</rdfs:label>
		<dct:source>vvo:TrafficPattern</dct:source>
		<rdfs:isDefinedBy rdf:resource="http://purl.org/vvo/ns#"/>
		<skos:definition xml:lang="en">Combined usage as a traffic pattern</skos:definition>
	</owl:NamedIndividual>
	
	<owl:Class rdf:about="&auto-vc;CommercialMotorVehicle">
		<rdfs:subClassOf rdf:resource="&auto-vc;TransportVehicle"/>
		<rdfs:label xml:lang="en">commercial motor vehicle</rdfs:label>
		<skos:definition xml:lang="en">Any motor vehicle used for the transportation of goods, property or people in interstate (See 2.9.2) or intrastate (2.9.3) commerce.</skos:definition>
		<fibo-fnd-utl-av:adaptedFrom>ANSI D.16-2017, section 2.2.7.3</fibo-fnd-utl-av:adaptedFrom>
	</owl:Class>
	
	<owl:Class rdf:about="&auto-vc;CompleteCarModel">
		<rdfs:subClassOf rdf:resource="&auto-mo;Model"/>
		<rdfs:subClassOf>
			<owl:Restriction>
				<owl:onProperty rdf:resource="&auto-vc;hasSpecItemChoice"/>
				<owl:onClass rdf:resource="&auto-vc;ChoiceOrComponent"/>
				<owl:minQualifiedCardinality rdf:datatype="&xsd;nonNegativeInteger">0</owl:minQualifiedCardinality>
			</owl:Restriction>
		</rdfs:subClassOf>
		<rdfs:label xml:lang="en">complete car model</rdfs:label>
		<rdfs:isDefinedBy rdf:resource="http://purl.org/coo/ns#"/>
		<owl:disjointWith rdf:resource="&auto-vc;ConfigurationInfo"/>
		<owl:disjointWith rdf:resource="&auto-vc;Derivative"/>
		<owl:disjointWith rdf:resource="&auto-vc;PropertySpecification"/>
		<owl:disjointWith rdf:resource="&auto-vc;SpecItemCollection"/>
		<owl:disjointWith rdf:resource="&auto-vc;Trim"/>
		<skos:definition xml:lang="en">A Complete Car Model is an abstract entity specifying all features and configuration choices needed for actually producing a vehicle. In other words, it is the gr:ProductOrServiceModel (&quot;datasheet&quot;) for a completely configured vehicle.
While a Complete Car Model can be defined indepently of a Base Model, Trim, or Derivative, it is usually based on a Derivative plus choices for all mandatory configurational options (coo:SpecItemCollection) of that Derivative.
A Complete Car Model should be linked to its Derivative via gr:isVariantOf, if available.

Example: VW Golf S 1.6 TDI 3door Manual in ocean blue with air-conditioning, CD player, trailer hitch, power steering, and power windows

Note: A coo:CompleteCarModel is NOT an actual car, but a complete feature description of one or multiple actual cars.</skos:definition>
	</owl:Class>
	
	<owl:Class rdf:about="&auto-vc;ConfigurationInfo">
		<rdfs:subClassOf rdf:resource="&auto-mo;GenericallyDependentContinuant"/>
		<rdfs:subClassOf>
			<owl:Restriction>
				<owl:onProperty rdf:resource="&auto-vc;featureOverride"/>
				<owl:onClass rdf:resource="&auto-vc;PropertySpecification"/>
				<owl:minQualifiedCardinality rdf:datatype="&xsd;nonNegativeInteger">0</owl:minQualifiedCardinality>
			</owl:Restriction>
		</rdfs:subClassOf>
		<rdfs:subClassOf>
			<owl:Restriction>
				<owl:onProperty rdf:resource="&auto-vc;valid"/>
				<owl:onDataRange rdf:resource="&xsd;boolean"/>
				<owl:qualifiedCardinality rdf:datatype="&xsd;nonNegativeInteger">1</owl:qualifiedCardinality>
			</owl:Restriction>
		</rdfs:subClassOf>
		<rdfs:subClassOf>
			<owl:Restriction>
				<owl:onProperty rdf:resource="&auto-vc;includesChoices"/>
				<owl:someValuesFrom rdf:resource="&auto-vc;ChoiceOrComponent"/>
			</owl:Restriction>
		</rdfs:subClassOf>
		<rdfs:label xml:lang="en">configuration info</rdfs:label>
		<rdfs:isDefinedBy rdf:resource="http://purl.org/coo/ns#"/>
		<owl:disjointWith rdf:resource="&auto-vc;Derivative"/>
		<owl:disjointWith rdf:resource="&auto-vc;PropertySpecification"/>
		<owl:disjointWith rdf:resource="&auto-vc;SpecItemCollection"/>
		<owl:disjointWith rdf:resource="&auto-vc;Trim"/>
		<skos:definition xml:lang="en">A Configuration Info is an abstract entity that gives information on whether a set of Choices Or Components results in a valid configuration. 
Using coo:compatible, it is possible to indicate either compatibility (true) and incompatibility (false) so that modeling remains efficient, no matter whether most combinations are valid or whether most configurations are invalid.
If no such statement is found, the validity of a configuration is unknown.

Note: The two properties coo:includes and coo:dependsOn, attached to coo:ChoiceOrComponent, may contain additional information on the validity of configuration.</skos:definition>
	</owl:Class>
	
	<owl:Class rdf:about="&auto-vc;ContainerChassisTrailer">
		<rdfs:subClassOf rdf:resource="&auto-vc;Semitrailer"/>
		<rdfs:label xml:lang="en">container chassis trailer</rdfs:label>
		<skos:definition xml:lang="en">semitrailer of skeleton construction limited to a bottom frame, one or more axles, specially built and fitted with locking devices for the transport of intermodal cargo containers so that when the chassis and container are assembled, the units serve the same function as an over the road trailer</skos:definition>
	</owl:Class>
	
	<owl:Class rdf:about="&auto-vc;CoveredFarmVehicle">
		<rdfs:subClassOf rdf:resource="&auto-vc;SpecialVehicle"/>
		<rdfs:label xml:lang="en">covered farm vehicle</rdfs:label>
		<skos:definition xml:lang="en">straight truck or articulated vehicle that is registered in a State with a license plate or other designation issued by the State of registration that allows law enforcement officials to identify it as a farm vehicle and used to transport agricultural commodities, livestock, machinery or supplies to or from a farm or ranch</skos:definition>
	</owl:Class>
	
	<owl:Class rdf:about="&auto-vc;CribTypeLogTrailer">
		<rdfs:subClassOf rdf:resource="&auto-vc;FullTrailer"/>
		<rdfs:label xml:lang="en">crib-type log trailer</rdfs:label>
		<skos:definition xml:lang="en">trailer equipped with stakes, bunks, a front-end structure, and a rear structure to restrain logs</skos:definition>
	</owl:Class>
	
	<owl:Class rdf:about="&auto-vc;DamageOrAccident">
		<rdfs:subClassOf rdf:resource="&auto-mo;Process"/>
		<rdfs:subClassOf>
			<owl:Restriction>
				<owl:onProperty rdf:resource="&auto-vc;carriedOutBy"/>
				<owl:onClass>
					<owl:Class>
						<owl:unionOf rdf:parseType="Collection">
							<rdf:Description rdf:about="&auto-vc;BusinessEntity">
							</rdf:Description>
							<rdf:Description rdf:about="&auto-vc;BusinessEntityType">
							</rdf:Description>
						</owl:unionOf>
					</owl:Class>
				</owl:onClass>
				<owl:minQualifiedCardinality rdf:datatype="&xsd;nonNegativeInteger">0</owl:minQualifiedCardinality>
			</owl:Restriction>
		</rdfs:subClassOf>
		<rdfs:subClassOf>
			<owl:Restriction>
				<owl:onProperty rdf:resource="&auto-vc;airbagDeployment"/>
				<owl:minQualifiedCardinality rdf:datatype="&xsd;nonNegativeInteger">0</owl:minQualifiedCardinality>
				<owl:onDataRange rdf:resource="&xsd;boolean"/>
			</owl:Restriction>
		</rdfs:subClassOf>
		<rdfs:subClassOf>
			<owl:Restriction>
				<owl:onProperty rdf:resource="&auto-vc;notAtFaultAccident"/>
				<owl:minQualifiedCardinality rdf:datatype="&xsd;nonNegativeInteger">0</owl:minQualifiedCardinality>
				<owl:onDataRange rdf:resource="&xsd;boolean"/>
			</owl:Restriction>
		</rdfs:subClassOf>
		<rdfs:subClassOf>
			<owl:Restriction>
				<owl:onProperty rdf:resource="&auto-vc;originalPartsOnly"/>
				<owl:minQualifiedCardinality rdf:datatype="&xsd;nonNegativeInteger">0</owl:minQualifiedCardinality>
				<owl:onDataRange rdf:resource="&xsd;boolean"/>
			</owl:Restriction>
		</rdfs:subClassOf>
		<rdfs:subClassOf>
			<owl:Restriction>
				<owl:onProperty rdf:resource="&auto-vc;repaired"/>
				<owl:minQualifiedCardinality rdf:datatype="&xsd;nonNegativeInteger">0</owl:minQualifiedCardinality>
				<owl:onDataRange rdf:resource="&xsd;boolean"/>
			</owl:Restriction>
		</rdfs:subClassOf>
		<rdfs:subClassOf>
			<owl:Restriction>
				<owl:onProperty rdf:resource="&auto-vc;structuralDamage"/>
				<owl:minQualifiedCardinality rdf:datatype="&xsd;nonNegativeInteger">0</owl:minQualifiedCardinality>
				<owl:onDataRange rdf:resource="&xsd;boolean"/>
			</owl:Restriction>
		</rdfs:subClassOf>
		<rdfs:label xml:lang="en">damage or accident</rdfs:label>
		<rdfs:isDefinedBy rdf:resource="http://purl.org/uco/ns#"/>
		<skos:definition xml:lang="en">an event in which the vehicle is being damaged</skos:definition>
	</owl:Class>
	
	<owl:Class rdf:about="&auto-vc;DecorativeTrims">
		<rdfs:subClassOf rdf:resource="&auto-vc;ChoiceOrComponent"/>
		<rdfs:label xml:lang="en">decorative trims choice or component</rdfs:label>
		<rdfs:isDefinedBy rdf:resource="http://purl.org/vvo/ns#"/>
		<skos:definition xml:lang="en">The class of decorative trim choices or components (a &quot;MonoSelectGroup&quot; in automotive terminology), VW ID: 8</skos:definition>
	</owl:Class>
	
	<owl:Class rdf:about="&auto-vc;Derivative">
		<rdfs:subClassOf rdf:resource="&auto-mo;Model"/>
		<rdfs:subClassOf>
			<owl:Class>
				<owl:intersectionOf rdf:parseType="Collection">
					<owl:Restriction>
						<owl:onProperty rdf:resource="&auto-vc;capCode"/>
						<owl:minQualifiedCardinality rdf:datatype="&xsd;nonNegativeInteger">0</owl:minQualifiedCardinality>
						<owl:onDataRange rdf:resource="&xsd;string"/>
					</owl:Restriction>
					<owl:Restriction>
						<owl:onProperty rdf:resource="&auto-vc;capCode"/>
						<owl:maxQualifiedCardinality rdf:datatype="&xsd;nonNegativeInteger">1</owl:maxQualifiedCardinality>
						<owl:onDataRange rdf:resource="&xsd;string"/>
					</owl:Restriction>
				</owl:intersectionOf>
			</owl:Class>
		</rdfs:subClassOf>
		<rdfs:subClassOf>
			<owl:Class>
				<owl:intersectionOf rdf:parseType="Collection">
					<owl:Restriction>
						<owl:onProperty rdf:resource="&auto-vc;dhCode"/>
						<owl:minQualifiedCardinality rdf:datatype="&xsd;nonNegativeInteger">0</owl:minQualifiedCardinality>
						<owl:onDataRange rdf:resource="&xsd;string"/>
					</owl:Restriction>
					<owl:Restriction>
						<owl:onProperty rdf:resource="&auto-vc;dhCode"/>
						<owl:maxQualifiedCardinality rdf:datatype="&xsd;nonNegativeInteger">1</owl:maxQualifiedCardinality>
						<owl:onDataRange rdf:resource="&xsd;string"/>
					</owl:Restriction>
				</owl:intersectionOf>
			</owl:Class>
		</rdfs:subClassOf>
		<rdfs:subClassOf>
			<owl:Restriction>
				<owl:onProperty rdf:resource="&auto-vc;hasCompleteCarModel"/>
				<owl:onClass rdf:resource="&auto-vc;CompleteCarModel"/>
				<owl:minQualifiedCardinality rdf:datatype="&xsd;nonNegativeInteger">0</owl:minQualifiedCardinality>
			</owl:Restriction>
		</rdfs:subClassOf>
		<rdfs:subClassOf>
			<owl:Restriction>
				<owl:onProperty rdf:resource="&auto-vc;compatibility"/>
				<owl:onClass rdf:resource="&auto-vc;ConfigurationInfo"/>
				<owl:minQualifiedCardinality rdf:datatype="&xsd;nonNegativeInteger">0</owl:minQualifiedCardinality>
			</owl:Restriction>
		</rdfs:subClassOf>
		<rdfs:subClassOf>
			<owl:Restriction>
				<owl:onProperty rdf:resource="&auto-vc;hasSpecItems"/>
				<owl:onClass rdf:resource="&auto-vc;SpecItemCollection"/>
				<owl:minQualifiedCardinality rdf:datatype="&xsd;nonNegativeInteger">0</owl:minQualifiedCardinality>
			</owl:Restriction>
		</rdfs:subClassOf>
		<rdfs:label xml:lang="en">derivative</rdfs:label>
		<rdfs:isDefinedBy rdf:resource="http://purl.org/coo/ns#"/>
		<owl:disjointWith rdf:resource="&auto-vc;PropertySpecification"/>
		<owl:disjointWith rdf:resource="&auto-vc;SpecItemCollection"/>
		<owl:disjointWith rdf:resource="&auto-vc;Trim"/>
		<skos:definition xml:lang="en">A Derivative is an abstract entity specifying (1) the basic features plus (2) a set of functional (e.g. engine type) and non-functional configuration (e.g. upholstery) choices of a group of vehicles.
A Derivative has often a number of remaining configuration choices (coo:SpecItemCollection attached via coo:hasSpecItems), which will determine the actual properties of the resulting vehicle.    
A Derivative should be linked to its Trim via gr:isVariantOf, if available.

Examples: VW Golf S 1.6 TDI 3door Manual</skos:definition>
	</owl:Class>
	
	<owl:NamedIndividual rdf:about="&auto-vc;Diesel">
		<rdf:type rdf:resource="&auto-vc;FuelTypeValue"/>
		<rdfs:label xml:lang="en">diesel</rdfs:label>
		<dct:source>vso:FuelTypeValue</dct:source>
		<rdfs:isDefinedBy rdf:resource="http://purl.org/vvo/ns#"/>
		<skos:definition xml:lang="en">Diesel, VW ID: 2</skos:definition>
		<auto-vc:hasID>2</auto-vc:hasID>
	</owl:NamedIndividual>
	
	<owl:Class rdf:about="&auto-vc;DriveWheelConfigurationValue">
		<rdfs:subClassOf rdf:resource="&auto-mo;QualitativeValue"/>
		<rdfs:label xml:lang="en">drive wheel configuration value</rdfs:label>
		<dct:isPartOf rdf:resource="http://auto.schema.org"/>
		<dct:source rdf:resource="http://www.w3.org/wiki/WebSchemas/SchemaDotOrgSources#Automotive_Ontology_Working_Group"/>
		<sm:directSource rdf:resource="https://schema.org/DriveWheelConfigurationValue"/>
		<rdfs:isDefinedBy rdf:resource="http://purl.org/vso/ns"/>
		<skos:definition xml:lang="en">a value indicating which roadwheels will receive torque</skos:definition>
	</owl:Class>
	
	<owl:NamedIndividual rdf:about="&auto-vc;DrivingSchoolVehicleUsage">
		<rdf:type rdf:resource="&auto-vc;CarUsageType"/>
		<rdfs:label>driving school vehicle usage</rdfs:label>
		<dct:isPartOf rdf:resource="http://auto.schema.org"/>
		<dct:source rdf:resource="http://www.w3.org/wiki/WebSchemas/SchemaDotOrgSources#Automotive_Ontology_Working_Group"/>
		<skos:definition>Indicates the usage of the vehicle for driving school.</skos:definition>
	</owl:NamedIndividual>
	
	<owl:Class rdf:about="&auto-vc;EmissionStandardValue">
		<rdfs:subClassOf rdf:resource="&auto-mo;QualitativeValue"/>
		<rdfs:label xml:lang="en">emission standard value</rdfs:label>
		<rdfs:comment xml:lang="en">You can safely use any reasonable DBPedia URI, e.g. 
  http://dbpedia.org/resource/Super_Ultra_Low_Emission_Vehicle
  http://dbpedia.org/resource/Partial_zero-emissions_vehicle

See also http://en.wikipedia.org/wiki/Emissions_standard.

Unfortunately, there are no DBPedia identifiers for the popular Euro 1 - Euro 5 standards available.
If you cannot find a suitable identifier in DBPedia, define your own as an instance of vso:EmissionStandardValue.</rdfs:comment>
		<rdfs:isDefinedBy rdf:resource="http://purl.org/vso/ns"/>
		<skos:definition xml:lang="en">a value indicating the an emission standard</skos:definition>
	</owl:Class>
	
	<owl:Class rdf:about="&auto-vc;Engine">
		<rdfs:subClassOf rdf:resource="&auto-vc;ChoiceOrComponent"/>
		<rdfs:subClassOf>
			<owl:Class>
				<owl:intersectionOf rdf:parseType="Collection">
					<owl:Restriction>
						<owl:onProperty rdf:resource="&auto-vc;cylinderTypeId"/>
						<owl:minQualifiedCardinality rdf:datatype="&xsd;nonNegativeInteger">0</owl:minQualifiedCardinality>
						<owl:onDataRange rdf:resource="&xsd;string"/>
					</owl:Restriction>
					<owl:Restriction>
						<owl:onProperty rdf:resource="&auto-vc;cylinderTypeId"/>
						<owl:maxQualifiedCardinality rdf:datatype="&xsd;nonNegativeInteger">1</owl:maxQualifiedCardinality>
						<owl:onDataRange rdf:resource="&xsd;string"/>
					</owl:Restriction>
				</owl:intersectionOf>
			</owl:Class>
		</rdfs:subClassOf>
		<rdfs:subClassOf>
			<owl:Class>
				<owl:intersectionOf rdf:parseType="Collection">
					<owl:Restriction>
						<owl:onProperty rdf:resource="&auto-vc;fuelInjectionTypeId"/>
						<owl:minQualifiedCardinality rdf:datatype="&xsd;nonNegativeInteger">0</owl:minQualifiedCardinality>
						<owl:onDataRange rdf:resource="&xsd;string"/>
					</owl:Restriction>
					<owl:Restriction>
						<owl:onProperty rdf:resource="&auto-vc;fuelInjectionTypeId"/>
						<owl:maxQualifiedCardinality rdf:datatype="&xsd;nonNegativeInteger">1</owl:maxQualifiedCardinality>
						<owl:onDataRange rdf:resource="&xsd;string"/>
					</owl:Restriction>
				</owl:intersectionOf>
			</owl:Class>
		</rdfs:subClassOf>
		<rdfs:label xml:lang="en">engine choice or component</rdfs:label>
		<rdfs:isDefinedBy rdf:resource="http://purl.org/vvo/ns#"/>
		<skos:definition xml:lang="en">The class of engines as choices or components</skos:definition>
	</owl:Class>
	
	<owl:Class rdf:about="&auto-vc;EngineSpecification">
		<rdfs:subClassOf rdf:resource="&auto-mo;GenericallyDependentContinuant"/>
		<rdfs:subClassOf>
			<owl:Restriction>
				<owl:onProperty rdf:resource="&auto-vc;engineType"/>
				<owl:onClass rdf:resource="&auto-mo;QualitativeValue"/>
				<owl:minQualifiedCardinality rdf:datatype="&xsd;nonNegativeInteger">0</owl:minQualifiedCardinality>
			</owl:Restriction>
		</rdfs:subClassOf>
		<rdfs:subClassOf>
			<owl:Restriction>
				<owl:onProperty rdf:resource="&auto-vc;engineDisplacement"/>
				<owl:onClass rdf:resource="&auto-mo;QuantitativeValue"/>
				<owl:minQualifiedCardinality rdf:datatype="&xsd;nonNegativeInteger">0</owl:minQualifiedCardinality>
			</owl:Restriction>
		</rdfs:subClassOf>
		<rdfs:subClassOf>
			<owl:Restriction>
				<owl:onProperty rdf:resource="&auto-vc;enginePower"/>
				<owl:onClass rdf:resource="&auto-mo;QuantitativeValue"/>
				<owl:minQualifiedCardinality rdf:datatype="&xsd;nonNegativeInteger">0</owl:minQualifiedCardinality>
			</owl:Restriction>
		</rdfs:subClassOf>
		<rdfs:subClassOf>
			<owl:Restriction>
				<owl:onProperty rdf:resource="&auto-vc;torque"/>
				<owl:onClass rdf:resource="&auto-mo;QuantitativeValue"/>
				<owl:minQualifiedCardinality rdf:datatype="&xsd;nonNegativeInteger">0</owl:minQualifiedCardinality>
			</owl:Restriction>
		</rdfs:subClassOf>
		<rdfs:subClassOf>
			<owl:Restriction>
				<owl:onProperty rdf:resource="&auto-vc;fuelType"/>
				<owl:someValuesFrom>
					<owl:Class>
						<owl:unionOf rdf:parseType="Collection">
							<rdf:Description rdf:about="&auto-mo;QualitativeValue">
							</rdf:Description>
							<rdf:Description rdf:about="&auto-mo;TextValue">
							</rdf:Description>
						</owl:unionOf>
					</owl:Class>
				</owl:someValuesFrom>
			</owl:Restriction>
		</rdfs:subClassOf>
		<rdfs:label xml:lang="en">engine specification</rdfs:label>
		<dct:isPartOf rdf:resource="http://auto.schema.org"/>
		<dct:source rdf:resource="http://www.w3.org/wiki/WebSchemas/SchemaDotOrgSources#Automotive_Ontology_Working_Group"/>
		<sm:directSource rdf:resource="https://schema.org/EngineSpecification"/>
		<skos:definition xml:lang="en">information about the engine of the vehicle. A vehicle can have multiple engines represented by multiple engine specification entities</skos:definition>
	</owl:Class>
	
	<owl:Class rdf:about="&auto-vc;EngineTypeValue">
		<rdfs:subClassOf rdf:resource="&auto-mo;QualitativeValue"/>
		<rdfs:label xml:lang="en">engine type value</rdfs:label>
		<rdfs:comment xml:lang="en">You can safely use any reasonable DBPedia URI, e.g. 
  http://dbpedia.org/resource/Two-stroke_engine
  http://dbpedia.org/resource/Four-stroke_engine
  http://dbpedia.org/resource/Wankel_engine
  http://dbpedia.org/resource/Electric_motor</rdfs:comment>
		<rdfs:isDefinedBy rdf:resource="http://purl.org/vso/ns"/>
		<skos:definition xml:lang="en">a value indicating an engine type</skos:definition>
	</owl:Class>
	
	<owl:NamedIndividual rdf:about="&auto-vc;Euro1">
		<rdf:type rdf:resource="&auto-vc;EmissionStandardValue"/>
		<rdfs:label xml:lang="en">Euro 1</rdfs:label>
		<dct:source>vso:EmissionStandardValue</dct:source>
		<rdfs:isDefinedBy rdf:resource="http://purl.org/vvo/ns#"/>
		<skos:definition xml:lang="en">The emission standard EURO 1</skos:definition>
	</owl:NamedIndividual>
	
	<owl:NamedIndividual rdf:about="&auto-vc;Euro2">
		<rdf:type rdf:resource="&auto-vc;EmissionStandardValue"/>
		<rdfs:label xml:lang="en">Euro 2</rdfs:label>
		<dct:source>vso:EmissionStandardValue</dct:source>
		<rdfs:isDefinedBy rdf:resource="http://purl.org/vvo/ns#"/>
		<skos:definition xml:lang="en">The emission standard EURO 2</skos:definition>
	</owl:NamedIndividual>
	
	<owl:NamedIndividual rdf:about="&auto-vc;Euro3">
		<rdf:type rdf:resource="&auto-vc;EmissionStandardValue"/>
		<rdfs:label xml:lang="en">Euro 3</rdfs:label>
		<dct:source>vso:EmissionStandardValue</dct:source>
		<rdfs:isDefinedBy rdf:resource="http://purl.org/vvo/ns#"/>
		<skos:definition xml:lang="en">The emission standard EURO 3</skos:definition>
	</owl:NamedIndividual>
	
	<owl:NamedIndividual rdf:about="&auto-vc;Euro4">
		<rdf:type rdf:resource="&auto-vc;EmissionStandardValue"/>
		<rdfs:label xml:lang="en">Euro 4</rdfs:label>
		<dct:source>vso:EmissionStandardValue</dct:source>
		<rdfs:isDefinedBy rdf:resource="http://purl.org/vvo/ns#"/>
		<skos:definition xml:lang="en">The emission standard EURO 4</skos:definition>
	</owl:NamedIndividual>
	
	<owl:NamedIndividual rdf:about="&auto-vc;ExtraUrban">
		<rdf:type rdf:resource="&auto-vc;TrafficPattern"/>
		<rdfs:label xml:lang="en">extra urban</rdfs:label>
		<dct:source>vvo:TrafficPattern</dct:source>
		<rdfs:isDefinedBy rdf:resource="http://purl.org/vvo/ns#"/>
		<skos:definition xml:lang="en">Extra urban as a traffic pattern</skos:definition>
	</owl:NamedIndividual>
	
	<owl:Class rdf:about="&auto-vc;FeatureValue">
		<rdfs:subClassOf rdf:resource="&auto-mo;QualitativeValue"/>
		<rdfs:label xml:lang="en">feature value</rdfs:label>
		<rdfs:comment xml:lang="en">You can safely use any reasonable DBPedia URI, e.g. 
  http://dbpedia.org/resource/Anti-lock_braking_system
  http://dbpedia.org/resource/Electronic_stability_control
  http://dbpedia.org/resource/Armrest
  http://dbpedia.org/resource/Spoiler_%28automotive%29
  http://dbpedia.org/resource/CD_Changer
  http://dbpedia.org/resource/Cup_holder
  http://dbpedia.org/resource/Tow_hitch
  http://dbpedia.org/resource/Power_window
  http://dbpedia.org/resource/Power_steering
  http://dbpedia.org/resource/Air_conditioner
  http://dbpedia.org/resource/Child_safety_lock
  http://dbpedia.org/resource/Parking_sensors</rdfs:comment>
		<rdfs:isDefinedBy rdf:resource="http://purl.org/vso/ns"/>
		<skos:definition xml:lang="en">a value indicating the features or accessories that are attached to or belong to a vehicle</skos:definition>
	</owl:Class>
	
	<owl:Class rdf:about="&auto-vc;Financing">
		<rdfs:subClassOf rdf:resource="&auto-vc;PaymentMethod"/>
		<rdfs:subClassOf>
			<owl:Class>
				<owl:intersectionOf rdf:parseType="Collection">
					<owl:Restriction>
						<owl:onProperty rdf:resource="&auto-vc;advancedPayment"/>
						<owl:onClass rdf:resource="&auto-vc;PriceSpecification"/>
						<owl:minQualifiedCardinality rdf:datatype="&xsd;nonNegativeInteger">0</owl:minQualifiedCardinality>
					</owl:Restriction>
					<owl:Restriction>
						<owl:onProperty rdf:resource="&auto-vc;advancedPayment"/>
						<owl:onClass rdf:resource="&auto-vc;PriceSpecification"/>
						<owl:maxQualifiedCardinality rdf:datatype="&xsd;nonNegativeInteger">1</owl:maxQualifiedCardinality>
					</owl:Restriction>
				</owl:intersectionOf>
			</owl:Class>
		</rdfs:subClassOf>
		<rdfs:subClassOf>
			<owl:Class>
				<owl:intersectionOf rdf:parseType="Collection">
					<owl:Restriction>
						<owl:onProperty rdf:resource="&auto-vc;credit"/>
						<owl:onClass rdf:resource="&auto-vc;PriceSpecification"/>
						<owl:minQualifiedCardinality rdf:datatype="&xsd;nonNegativeInteger">0</owl:minQualifiedCardinality>
					</owl:Restriction>
					<owl:Restriction>
						<owl:onProperty rdf:resource="&auto-vc;credit"/>
						<owl:onClass rdf:resource="&auto-vc;PriceSpecification"/>
						<owl:maxQualifiedCardinality rdf:datatype="&xsd;nonNegativeInteger">1</owl:maxQualifiedCardinality>
					</owl:Restriction>
				</owl:intersectionOf>
			</owl:Class>
		</rdfs:subClassOf>
		<rdfs:subClassOf>
			<owl:Class>
				<owl:intersectionOf rdf:parseType="Collection">
					<owl:Restriction>
						<owl:onProperty rdf:resource="&auto-vc;customerCashPrice"/>
						<owl:onClass rdf:resource="&auto-vc;PriceSpecification"/>
						<owl:minQualifiedCardinality rdf:datatype="&xsd;nonNegativeInteger">0</owl:minQualifiedCardinality>
					</owl:Restriction>
					<owl:Restriction>
						<owl:onProperty rdf:resource="&auto-vc;customerCashPrice"/>
						<owl:onClass rdf:resource="&auto-vc;PriceSpecification"/>
						<owl:maxQualifiedCardinality rdf:datatype="&xsd;nonNegativeInteger">1</owl:maxQualifiedCardinality>
					</owl:Restriction>
				</owl:intersectionOf>
			</owl:Class>
		</rdfs:subClassOf>
		<rdfs:subClassOf>
			<owl:Class>
				<owl:intersectionOf rdf:parseType="Collection">
					<owl:Restriction>
						<owl:onProperty rdf:resource="&auto-vc;customerDeposit"/>
						<owl:onClass rdf:resource="&auto-vc;PriceSpecification"/>
						<owl:minQualifiedCardinality rdf:datatype="&xsd;nonNegativeInteger">0</owl:minQualifiedCardinality>
					</owl:Restriction>
					<owl:Restriction>
						<owl:onProperty rdf:resource="&auto-vc;customerDeposit"/>
						<owl:onClass rdf:resource="&auto-vc;PriceSpecification"/>
						<owl:maxQualifiedCardinality rdf:datatype="&xsd;nonNegativeInteger">1</owl:maxQualifiedCardinality>
					</owl:Restriction>
				</owl:intersectionOf>
			</owl:Class>
		</rdfs:subClassOf>
		<rdfs:subClassOf>
			<owl:Class>
				<owl:intersectionOf rdf:parseType="Collection">
					<owl:Restriction>
						<owl:onProperty rdf:resource="&auto-vc;depositContribution"/>
						<owl:onClass rdf:resource="&auto-vc;PriceSpecification"/>
						<owl:minQualifiedCardinality rdf:datatype="&xsd;nonNegativeInteger">0</owl:minQualifiedCardinality>
					</owl:Restriction>
					<owl:Restriction>
						<owl:onProperty rdf:resource="&auto-vc;depositContribution"/>
						<owl:onClass rdf:resource="&auto-vc;PriceSpecification"/>
						<owl:maxQualifiedCardinality rdf:datatype="&xsd;nonNegativeInteger">1</owl:maxQualifiedCardinality>
					</owl:Restriction>
				</owl:intersectionOf>
			</owl:Class>
		</rdfs:subClassOf>
		<rdfs:subClassOf>
			<owl:Class>
				<owl:intersectionOf rdf:parseType="Collection">
					<owl:Restriction>
						<owl:onProperty rdf:resource="&auto-vc;discount"/>
						<owl:onClass rdf:resource="&auto-vc;PriceSpecification"/>
						<owl:minQualifiedCardinality rdf:datatype="&xsd;nonNegativeInteger">0</owl:minQualifiedCardinality>
					</owl:Restriction>
					<owl:Restriction>
						<owl:onProperty rdf:resource="&auto-vc;discount"/>
						<owl:onClass rdf:resource="&auto-vc;PriceSpecification"/>
						<owl:maxQualifiedCardinality rdf:datatype="&xsd;nonNegativeInteger">1</owl:maxQualifiedCardinality>
					</owl:Restriction>
				</owl:intersectionOf>
			</owl:Class>
		</rdfs:subClassOf>
		<rdfs:subClassOf>
			<owl:Class>
				<owl:intersectionOf rdf:parseType="Collection">
					<owl:Restriction>
						<owl:onProperty rdf:resource="&auto-vc;excessMileage"/>
						<owl:onClass rdf:resource="&auto-vc;PriceSpecification"/>
						<owl:minQualifiedCardinality rdf:datatype="&xsd;nonNegativeInteger">0</owl:minQualifiedCardinality>
					</owl:Restriction>
					<owl:Restriction>
						<owl:onProperty rdf:resource="&auto-vc;excessMileage"/>
						<owl:onClass rdf:resource="&auto-vc;PriceSpecification"/>
						<owl:maxQualifiedCardinality rdf:datatype="&xsd;nonNegativeInteger">1</owl:maxQualifiedCardinality>
					</owl:Restriction>
				</owl:intersectionOf>
			</owl:Class>
		</rdfs:subClassOf>
		<rdfs:subClassOf>
			<owl:Class>
				<owl:intersectionOf rdf:parseType="Collection">
					<owl:Restriction>
						<owl:onProperty rdf:resource="&auto-vc;finalPaymentFee"/>
						<owl:onClass rdf:resource="&auto-vc;PriceSpecification"/>
						<owl:minQualifiedCardinality rdf:datatype="&xsd;nonNegativeInteger">0</owl:minQualifiedCardinality>
					</owl:Restriction>
					<owl:Restriction>
						<owl:onProperty rdf:resource="&auto-vc;finalPaymentFee"/>
						<owl:onClass rdf:resource="&auto-vc;PriceSpecification"/>
						<owl:maxQualifiedCardinality rdf:datatype="&xsd;nonNegativeInteger">1</owl:maxQualifiedCardinality>
					</owl:Restriction>
				</owl:intersectionOf>
			</owl:Class>
		</rdfs:subClassOf>
		<rdfs:subClassOf>
			<owl:Class>
				<owl:intersectionOf rdf:parseType="Collection">
					<owl:Restriction>
						<owl:onProperty rdf:resource="&auto-vc;firstMonthlyPaymentFee"/>
						<owl:onClass rdf:resource="&auto-vc;PriceSpecification"/>
						<owl:minQualifiedCardinality rdf:datatype="&xsd;nonNegativeInteger">0</owl:minQualifiedCardinality>
					</owl:Restriction>
					<owl:Restriction>
						<owl:onProperty rdf:resource="&auto-vc;firstMonthlyPaymentFee"/>
						<owl:onClass rdf:resource="&auto-vc;PriceSpecification"/>
						<owl:maxQualifiedCardinality rdf:datatype="&xsd;nonNegativeInteger">1</owl:maxQualifiedCardinality>
					</owl:Restriction>
				</owl:intersectionOf>
			</owl:Class>
		</rdfs:subClassOf>
		<rdfs:subClassOf>
			<owl:Class>
				<owl:intersectionOf rdf:parseType="Collection">
					<owl:Restriction>
						<owl:onProperty rdf:resource="&auto-vc;monthlyPayment"/>
						<owl:onClass rdf:resource="&auto-vc;PriceSpecification"/>
						<owl:minQualifiedCardinality rdf:datatype="&xsd;nonNegativeInteger">0</owl:minQualifiedCardinality>
					</owl:Restriction>
					<owl:Restriction>
						<owl:onProperty rdf:resource="&auto-vc;monthlyPayment"/>
						<owl:onClass rdf:resource="&auto-vc;PriceSpecification"/>
						<owl:maxQualifiedCardinality rdf:datatype="&xsd;nonNegativeInteger">1</owl:maxQualifiedCardinality>
					</owl:Restriction>
				</owl:intersectionOf>
			</owl:Class>
		</rdfs:subClassOf>
		<rdfs:subClassOf>
			<owl:Class>
				<owl:intersectionOf rdf:parseType="Collection">
					<owl:Restriction>
						<owl:onProperty rdf:resource="&auto-vc;otrRetailPrice"/>
						<owl:onClass rdf:resource="&auto-vc;PriceSpecification"/>
						<owl:minQualifiedCardinality rdf:datatype="&xsd;nonNegativeInteger">0</owl:minQualifiedCardinality>
					</owl:Restriction>
					<owl:Restriction>
						<owl:onProperty rdf:resource="&auto-vc;otrRetailPrice"/>
						<owl:onClass rdf:resource="&auto-vc;PriceSpecification"/>
						<owl:maxQualifiedCardinality rdf:datatype="&xsd;nonNegativeInteger">1</owl:maxQualifiedCardinality>
					</owl:Restriction>
				</owl:intersectionOf>
			</owl:Class>
		</rdfs:subClassOf>
		<rdfs:subClassOf>
			<owl:Class>
				<owl:intersectionOf rdf:parseType="Collection">
					<owl:Restriction>
						<owl:onProperty rdf:resource="&auto-vc;scrappageContribution"/>
						<owl:onClass rdf:resource="&auto-vc;PriceSpecification"/>
						<owl:minQualifiedCardinality rdf:datatype="&xsd;nonNegativeInteger">0</owl:minQualifiedCardinality>
					</owl:Restriction>
					<owl:Restriction>
						<owl:onProperty rdf:resource="&auto-vc;scrappageContribution"/>
						<owl:onClass rdf:resource="&auto-vc;PriceSpecification"/>
						<owl:maxQualifiedCardinality rdf:datatype="&xsd;nonNegativeInteger">1</owl:maxQualifiedCardinality>
					</owl:Restriction>
				</owl:intersectionOf>
			</owl:Class>
		</rdfs:subClassOf>
		<rdfs:subClassOf>
			<owl:Class>
				<owl:intersectionOf rdf:parseType="Collection">
					<owl:Restriction>
						<owl:onProperty rdf:resource="&auto-vc;totalPayable"/>
						<owl:onClass rdf:resource="&auto-vc;PriceSpecification"/>
						<owl:minQualifiedCardinality rdf:datatype="&xsd;nonNegativeInteger">0</owl:minQualifiedCardinality>
					</owl:Restriction>
					<owl:Restriction>
						<owl:onProperty rdf:resource="&auto-vc;totalPayable"/>
						<owl:onClass rdf:resource="&auto-vc;PriceSpecification"/>
						<owl:maxQualifiedCardinality rdf:datatype="&xsd;nonNegativeInteger">1</owl:maxQualifiedCardinality>
					</owl:Restriction>
				</owl:intersectionOf>
			</owl:Class>
		</rdfs:subClassOf>
		<rdfs:subClassOf>
			<owl:Class>
				<owl:intersectionOf rdf:parseType="Collection">
					<owl:Restriction>
						<owl:onProperty rdf:resource="&auto-vc;shortSubtitle"/>
						<owl:minQualifiedCardinality rdf:datatype="&xsd;nonNegativeInteger">0</owl:minQualifiedCardinality>
						<owl:onDataRange rdf:resource="&rdf;PlainLiteral"/>
					</owl:Restriction>
					<owl:Restriction>
						<owl:onProperty rdf:resource="&auto-vc;shortSubtitle"/>
						<owl:maxQualifiedCardinality rdf:datatype="&xsd;nonNegativeInteger">1</owl:maxQualifiedCardinality>
						<owl:onDataRange rdf:resource="&rdf;PlainLiteral"/>
					</owl:Restriction>
				</owl:intersectionOf>
			</owl:Class>
		</rdfs:subClassOf>
		<rdfs:subClassOf>
			<owl:Class>
				<owl:intersectionOf rdf:parseType="Collection">
					<owl:Restriction>
						<owl:onProperty rdf:resource="&auto-vc;shortTitle"/>
						<owl:minQualifiedCardinality rdf:datatype="&xsd;nonNegativeInteger">0</owl:minQualifiedCardinality>
						<owl:onDataRange rdf:resource="&rdf;PlainLiteral"/>
					</owl:Restriction>
					<owl:Restriction>
						<owl:onProperty rdf:resource="&auto-vc;shortTitle"/>
						<owl:maxQualifiedCardinality rdf:datatype="&xsd;nonNegativeInteger">1</owl:maxQualifiedCardinality>
						<owl:onDataRange rdf:resource="&rdf;PlainLiteral"/>
					</owl:Restriction>
				</owl:intersectionOf>
			</owl:Class>
		</rdfs:subClassOf>
		<rdfs:subClassOf>
			<owl:Class>
				<owl:intersectionOf rdf:parseType="Collection">
					<owl:Restriction>
						<owl:onProperty rdf:resource="&auto-vc;subtitle"/>
						<owl:minQualifiedCardinality rdf:datatype="&xsd;nonNegativeInteger">0</owl:minQualifiedCardinality>
						<owl:onDataRange rdf:resource="&rdf;PlainLiteral"/>
					</owl:Restriction>
					<owl:Restriction>
						<owl:onProperty rdf:resource="&auto-vc;subtitle"/>
						<owl:maxQualifiedCardinality rdf:datatype="&xsd;nonNegativeInteger">1</owl:maxQualifiedCardinality>
						<owl:onDataRange rdf:resource="&rdf;PlainLiteral"/>
					</owl:Restriction>
				</owl:intersectionOf>
			</owl:Class>
		</rdfs:subClassOf>
		<rdfs:subClassOf>
			<owl:Class>
				<owl:intersectionOf rdf:parseType="Collection">
					<owl:Restriction>
						<owl:onProperty rdf:resource="&auto-vc;termsAndConditions"/>
						<owl:minQualifiedCardinality rdf:datatype="&xsd;nonNegativeInteger">0</owl:minQualifiedCardinality>
						<owl:onDataRange rdf:resource="&rdf;PlainLiteral"/>
					</owl:Restriction>
					<owl:Restriction>
						<owl:onProperty rdf:resource="&auto-vc;termsAndConditions"/>
						<owl:maxQualifiedCardinality rdf:datatype="&xsd;nonNegativeInteger">1</owl:maxQualifiedCardinality>
						<owl:onDataRange rdf:resource="&rdf;PlainLiteral"/>
					</owl:Restriction>
				</owl:intersectionOf>
			</owl:Class>
		</rdfs:subClassOf>
		<rdfs:subClassOf>
			<owl:Class>
				<owl:intersectionOf rdf:parseType="Collection">
					<owl:Restriction>
						<owl:onProperty rdf:resource="&auto-vc;apr"/>
						<owl:minQualifiedCardinality rdf:datatype="&xsd;nonNegativeInteger">0</owl:minQualifiedCardinality>
						<owl:onDataRange rdf:resource="&xsd;decimal"/>
					</owl:Restriction>
					<owl:Restriction>
						<owl:onProperty rdf:resource="&auto-vc;apr"/>
						<owl:maxQualifiedCardinality rdf:datatype="&xsd;nonNegativeInteger">1</owl:maxQualifiedCardinality>
						<owl:onDataRange rdf:resource="&xsd;decimal"/>
					</owl:Restriction>
				</owl:intersectionOf>
			</owl:Class>
		</rdfs:subClassOf>
		<rdfs:subClassOf>
			<owl:Class>
				<owl:intersectionOf rdf:parseType="Collection">
					<owl:Restriction>
						<owl:onProperty rdf:resource="&auto-vc;finalPayment"/>
						<owl:minQualifiedCardinality rdf:datatype="&xsd;nonNegativeInteger">0</owl:minQualifiedCardinality>
						<owl:onDataRange rdf:resource="&xsd;decimal"/>
					</owl:Restriction>
					<owl:Restriction>
						<owl:onProperty rdf:resource="&auto-vc;finalPayment"/>
						<owl:maxQualifiedCardinality rdf:datatype="&xsd;nonNegativeInteger">1</owl:maxQualifiedCardinality>
						<owl:onDataRange rdf:resource="&xsd;decimal"/>
					</owl:Restriction>
				</owl:intersectionOf>
			</owl:Class>
		</rdfs:subClassOf>
		<rdfs:subClassOf>
			<owl:Class>
				<owl:intersectionOf rdf:parseType="Collection">
					<owl:Restriction>
						<owl:onProperty rdf:resource="&auto-vc;noOfMonthlyPayments"/>
						<owl:minQualifiedCardinality rdf:datatype="&xsd;nonNegativeInteger">0</owl:minQualifiedCardinality>
						<owl:onDataRange rdf:resource="&xsd;decimal"/>
					</owl:Restriction>
					<owl:Restriction>
						<owl:onProperty rdf:resource="&auto-vc;noOfMonthlyPayments"/>
						<owl:maxQualifiedCardinality rdf:datatype="&xsd;nonNegativeInteger">1</owl:maxQualifiedCardinality>
						<owl:onDataRange rdf:resource="&xsd;decimal"/>
					</owl:Restriction>
				</owl:intersectionOf>
			</owl:Class>
		</rdfs:subClassOf>
		<rdfs:label xml:lang="en">financing</rdfs:label>
		<rdfs:isDefinedBy rdf:resource="http://purl.org/vvo/ns#"/>
		<skos:definition xml:lang="en">the specification of a payment option via staged payments</skos:definition>
	</owl:Class>
	
	<owl:NamedIndividual rdf:about="&auto-vc;FourWheelDriveConfiguration">
		<rdf:type rdf:resource="&auto-vc;DriveWheelConfigurationValue"/>
		<rdfs:label xml:lang="en">four-wheel drive</rdfs:label>
		<skos:definition xml:lang="en">Four-wheel Drive is a transmission layout where the engine primarily drives two wheels with a part-time four-wheel drive capability.</skos:definition>
	</owl:NamedIndividual>
	
	<owl:NamedIndividual rdf:about="&auto-vc;FrontWheelDriveConfiguration">
		<rdf:type rdf:resource="&auto-vc;DriveWheelConfigurationValue"/>
		<rdfs:label xml:lang="en">front-wheel drive</rdfs:label>
		<skos:definition xml:lang="en">Front-wheel drive is a transmission layout where the engine drives the front wheels.</skos:definition>
		<fibo-fnd-utl-av:synonym xml:lang="en">FWD</fibo-fnd-utl-av:synonym>
	</owl:NamedIndividual>
	
	<owl:Class rdf:about="&auto-vc;FuelQuantity">
		<rdfs:subClassOf rdf:resource="&auto-mo;QuantitativeValueFloat"/>
		<rdfs:label xml:lang="en">fuel quantity</rdfs:label>
		<rdfs:isDefinedBy rdf:resource="http://purl.org/vso/ns"/>
		<skos:definition xml:lang="en">a value indicating an amount of fuel</skos:definition>
	</owl:Class>
	
	<owl:Class rdf:about="&auto-vc;FuelTypeValue">
		<rdfs:subClassOf rdf:resource="&auto-mo;QualitativeValue"/>
		<rdfs:label xml:lang="en">fuel type value</rdfs:label>
		<rdfs:comment xml:lang="en">You can safely use any reasonable DBPedia URI, e.g. 
  http://dbpedia.org/resource/Gasoline
  http://dbpedia.org/resource/Diesel
  http://dbpedia.org/resource/Biodiesel
  http://dbpedia.org/resource/Kerosene</rdfs:comment>
		<rdfs:isDefinedBy rdf:resource="http://purl.org/vso/ns"/>
		<skos:definition xml:lang="en">a value indicating a type of fuel</skos:definition>
	</owl:Class>
	
	<owl:Class rdf:about="&auto-vc;FullTrailer">
		<rdfs:subClassOf rdf:resource="&auto-vc;Trailer"/>
		<rdfs:label xml:lang="en">full trailer</rdfs:label>
		<rdfs:comment xml:lang="en">An auxiliary undercarriage assembly, commonly known as a converter dolly and consisting of a chassis, fifth wheel and one or more tow bars, is sometimes used to convert a semitrailer to a full trailer. A semitrailer equipped with a converter dolly is considered to be a full trailer.</rdfs:comment>
		<skos:definition xml:lang="en">A trailer, other than a pole trailer, designed for carrying property and so constructed that no part of its weight rests upon or is carried by the towing road vehicle.</skos:definition>
		<fibo-fnd-utl-av:adaptedFrom>ANSI D.16-2017, section 2.2.18</fibo-fnd-utl-av:adaptedFrom>
	</owl:Class>
	
	<owl:NamedIndividual rdf:about="&auto-vc;Garage">
		<rdf:type rdf:resource="&auto-vc;ParkingType"/>
		<rdfs:label xml:lang="en">garage</rdfs:label>
		<rdfs:isDefinedBy rdf:resource="http://purl.org/uco/ns#"/>
		<skos:definition xml:lang="en">The parking of a vehicle in a closed garage</skos:definition>
	</owl:NamedIndividual>
	
	<owl:NamedIndividual rdf:about="&auto-vc;GearboxAutomatic">
		<rdf:type rdf:resource="&auto-vc;GearboxTypeValue"/>
		<rdfs:label xml:lang="en">automatic</rdfs:label>
		<dct:source>vvo:GearboxTypeValue</dct:source>
		<rdfs:isDefinedBy rdf:resource="http://purl.org/vvo/ns#"/>
		<skos:definition xml:lang="en">Automatic gearbox, VW ID: 2</skos:definition>
		<auto-vc:hasID>2</auto-vc:hasID>
	</owl:NamedIndividual>
	
	<owl:NamedIndividual rdf:about="&auto-vc;GearboxDSG">
		<rdf:type rdf:resource="&auto-vc;GearboxTypeValue"/>
		<rdfs:label xml:lang="en">DSG</rdfs:label>
		<dct:source>vvo:GearboxTypeValue</dct:source>
		<rdfs:isDefinedBy rdf:resource="http://purl.org/vvo/ns#"/>
		<skos:definition xml:lang="en">DSG gearbox, VW ID: 3</skos:definition>
		<auto-vc:hasID>3</auto-vc:hasID>
	</owl:NamedIndividual>
	
	<owl:NamedIndividual rdf:about="&auto-vc;GearboxManual">
		<rdf:type rdf:resource="&auto-vc;GearboxTypeValue"/>
		<rdfs:label xml:lang="en">manual</rdfs:label>
		<dct:source>vvo:GearboxTypeValue</dct:source>
		<rdfs:isDefinedBy rdf:resource="http://purl.org/vvo/ns#"/>
		<skos:definition xml:lang="en">Manual gearbox, VW ID: 1</skos:definition>
		<auto-vc:hasID>1</auto-vc:hasID>
	</owl:NamedIndividual>
	
	<owl:Class rdf:about="&auto-vc;GearboxTypeValue">
		<rdfs:subClassOf rdf:resource="&auto-mo;QualitativeValue"/>
		<rdfs:label xml:lang="en">gearbox type value</rdfs:label>
		<rdfs:isDefinedBy rdf:resource="http://purl.org/vvo/ns#"/>
		<skos:definition xml:lang="en">A value indicating a gearbox type.</skos:definition>
	</owl:Class>
	
	<owl:Class rdf:about="&auto-vc;HeavyHaulerTrailer">
		<rdfs:subClassOf rdf:resource="&auto-vc;FullTrailer"/>
		<rdfs:label xml:lang="en">heavy hauler trailer</rdfs:label>
		<skos:definition xml:lang="en">trailer whose brakes lines are designed to adapt to separation or extension of the vehicle frame and/or which body consists only of a platform whose primary cargo-carrying surface is not more than 1,016 mm (40 inches) above the ground in an unloaded condition, except that it may include sides that are designed to be easily removable and a permanent “front-end structure”, but that is not a container chassis trailer</skos:definition>
	</owl:Class>
	
	<owl:Class rdf:about="&auto-vc;HeavyTruck">
		<rdfs:subClassOf rdf:resource="&auto-vc;Truck"/>
		<rdfs:label xml:lang="en">heavy truck</rdfs:label>
		<skos:definition xml:lang="en">A truck which has a gross vehicle weight rating (GVWR) of more than 26,000 pounds (11,793 kilograms).</skos:definition>
		<fibo-fnd-utl-av:adaptedFrom>ANSI D.16-2017, section 2.2.26</fibo-fnd-utl-av:adaptedFrom>
	</owl:Class>
	
	<owl:Class rdf:about="&auto-vc;HorizontalDischargeTrailer">
		<rdfs:subClassOf rdf:resource="&auto-vc;FullTrailer"/>
		<rdfs:label xml:lang="en">road construction controlled horizontal discharge trailer</rdfs:label>
		<skos:definition xml:lang="en">trailer or semitrailer that is equipped with a mechanical drive and a conveyor to deliver asphalt and other road building materials, in a controlled horizontal manner, into a lay down machine or paving equipment for road construction and paving operations</skos:definition>
	</owl:Class>
	
	<owl:Class rdf:about="&auto-vc;HumanPoweredLandVehicle">
		<rdfs:subClassOf rdf:resource="&auto-vc;RoadVehicle"/>
		<rdfs:label xml:lang="en">human powered land vehicle</rdfs:label>
		<skos:definition xml:lang="en">land vehicle propelled over ground by human power</skos:definition>
	</owl:Class>
	
	<owl:NamedIndividual rdf:about="&auto-vc;Hybrid">
		<rdf:type rdf:resource="&auto-vc;FuelTypeValue"/>
		<rdfs:label xml:lang="en">hybrid</rdfs:label>
		<dct:source>vso:FuelTypeValue</dct:source>
		<rdfs:isDefinedBy rdf:resource="http://purl.org/vvo/ns#"/>
		<skos:definition xml:lang="en">Hybrid, VW ID: 3</skos:definition>
		<auto-vc:hasID>3</auto-vc:hasID>
	</owl:NamedIndividual>
	
	<owl:NamedIndividual rdf:about="&auto-vc;IndependentDealer">
		<rdf:type rdf:resource="&auto-vc;BusinessEntityType"/>
		<rdfs:label xml:lang="en">independent dealer</rdfs:label>
		<rdfs:isDefinedBy rdf:resource="http://purl.org/uco/ns#"/>
		<skos:definition xml:lang="en">An independent dealer</skos:definition>
	</owl:NamedIndividual>
	
	<owl:Class rdf:about="&auto-vc;IntercityBus">
		<rdfs:subClassOf rdf:resource="&auto-vc;Bus"/>
		<rdfs:label xml:lang="en">intercity bus</rdfs:label>
		<skos:definition xml:lang="en">A bus used for long-distance passenger transportation between cities over fixed routes with regular schedules.</skos:definition>
		<fibo-fnd-utl-av:adaptedFrom>ANSI D.16-2017, section 2.2.10.4</fibo-fnd-utl-av:adaptedFrom>
	</owl:Class>
	
	<owl:Class rdf:about="&auto-vc;Kayak">
		<rdfs:subClassOf rdf:resource="&auto-vc;Watercraft"/>
		<rdfs:label xml:lang="en">kayak</rdfs:label>
		<rdfs:isDefinedBy rdf:resource="http://purl.org/vso/ns"/>
		<rdfs:seeAlso rdf:resource="http://dbpedia.org/resource/Kayak"/>
		<rdfs:seeAlso rdf:resource="http://en.wikipedia.org/wiki/Kayak"/>
		<skos:definition xml:lang="en">a small human-powered watercraft that traditionally has a covered deck, and one or more cockpits, each seating one paddler who strokes a double-bladed paddle. In this ontology, kayaks are considered watercrafts of their own kind, not a subtype of boat</skos:definition>
	</owl:Class>
	
	<owl:Class rdf:about="&auto-vc;LandVehicle">
		<rdfs:subClassOf rdf:resource="&auto-vc;Vehicle"/>
		<rdfs:label xml:lang="en">land vehicle</rdfs:label>
		<rdfs:comment>QName: auto-vc-vc:LandVehicle</rdfs:comment>
		<rdfs:isDefinedBy rdf:resource="https://spec.edmcouncil.org/auto/ontology/VC/VehicleCore/"/>
		<skos:definition xml:lang="en">A transport vehicle which is neither an aircraft nor a watercraft.</skos:definition>
		<fibo-fnd-utl-av:adaptedFrom>ANSI D.16-2017, section 2.1.7</fibo-fnd-utl-av:adaptedFrom>
	</owl:Class>
	
	<owl:Class rdf:about="&auto-vc;LargeBus">
		<rdfs:subClassOf rdf:resource="&auto-vc;Bus"/>
		<rdfs:label xml:lang="en">large bus</rdfs:label>
		<skos:definition xml:lang="en">A bus with seating for sixteen or more persons, including the driver.</skos:definition>
		<fibo-fnd-utl-av:adaptedFrom>ANSI D.16-2017, section 2.2.10.2</fibo-fnd-utl-av:adaptedFrom>
	</owl:Class>
	
	<owl:Class rdf:about="&auto-vc;LargeMotorcycle">
		<rdfs:subClassOf rdf:resource="&auto-vc;Motorcycle"/>
		<rdfs:label xml:lang="en">large motorcycle</rdfs:label>
		<skos:definition xml:lang="en">Any motorcycle other than a motor-driven cycle.</skos:definition>
		<fibo-fnd-utl-av:adaptedFrom>ANSI D.16-2017, section 2.2.9.2</fibo-fnd-utl-av:adaptedFrom>
	</owl:Class>
	
	<owl:Class rdf:about="&auto-vc;LargeSpecialVehicle">
		<rdfs:subClassOf rdf:resource="&auto-vc;SpecialVehicle"/>
		<rdfs:label xml:lang="pl">duży pojazd specjalny</rdfs:label>
		<rdfs:label xml:lang="en">large special vehicle</rdfs:label>
		<rdfs:seeAlso>source: https://www.toyota-ti.ac.jp/Lab/Denshi/COIN/Ontology/TTICore-0.03/TTICarOnto.owl</rdfs:seeAlso>
		<skos:definition xml:lang="en">special vehicle which is considered large</skos:definition>
	</owl:Class>
	
	<owl:NamedIndividual rdf:about="&auto-vc;LeftHandDriving">
		<rdf:type rdf:resource="&auto-vc;SteeringPositionValue"/>
		<rdfs:label xml:lang="en">left hand drive</rdfs:label>
		<skos:definition xml:lang="en">The steering position is on the left side of the vehicle (viewed from the main direction of driving). For cars this means that you drive on the right side of the road.</skos:definition>
	</owl:NamedIndividual>
	
	<owl:Class rdf:about="&auto-vc;LightTruck">
		<rdfs:subClassOf rdf:resource="&auto-vc;Truck"/>
		<rdfs:label xml:lang="en">light truck</rdfs:label>
		<skos:definition xml:lang="en">A truck which has a gross vehicle weight rating (GVWR) of 10,000 pounds (4,536 kilograms) or less</skos:definition>
		<fibo-fnd-utl-av:adaptedFrom>ANSI D.16-2017, section 2.2.24</fibo-fnd-utl-av:adaptedFrom>
	</owl:Class>
	
	<owl:Class rdf:about="&auto-vc;LowSpeedVehicle">
		<rdfs:subClassOf rdf:resource="&auto-vc;Car"/>
		<rdfs:label xml:lang="en">low speed vehicle</rdfs:label>
		<rdfs:comment xml:lang="en">LSVs are required to be equipped with basic items of safety equipment: headlamps, stop lamps, turn signal lamps, tail lamps, reflex reflectors, parking brake, windshields of either type AS-1 or AS-5 glazing, rearview mirrors, seat belts and vehicle identification numbers (VINs).</rdfs:comment>
		<skos:definition xml:lang="en">A motor vehicle with four or more wheels whose top speed is greater than 20 miles per hour, but not greater than 25 miles per hour.</skos:definition>
	</owl:Class>
	
	<owl:Class rdf:about="&auto-vc;MediumTruck">
		<rdfs:subClassOf rdf:resource="&auto-vc;Truck"/>
		<rdfs:label xml:lang="en">medium truck</rdfs:label>
		<skos:definition xml:lang="en">A truck which has a gross vehicle weight rating (GVWR) of more than 10,000 pounds and less than or equal to 26,000 pounds (4,536 to 11,793 kilograms).</skos:definition>
		<fibo-fnd-utl-av:adaptedFrom>ANSI D.16-2017, section 2.2.25</fibo-fnd-utl-av:adaptedFrom>
	</owl:Class>
	
	<owl:Class rdf:about="&auto-vc;ModificationOrMaintenance">
		<rdfs:subClassOf rdf:resource="&auto-mo;Process"/>
		<rdfs:subClassOf>
			<owl:Restriction>
				<owl:onProperty rdf:resource="&auto-vc;partAdded"/>
				<owl:minCardinality rdf:datatype="&xsd;nonNegativeInteger">0</owl:minCardinality>
			</owl:Restriction>
		</rdfs:subClassOf>
		<rdfs:subClassOf>
			<owl:Restriction>
				<owl:onProperty rdf:resource="&auto-vc;partRemoved"/>
				<owl:minCardinality rdf:datatype="&xsd;nonNegativeInteger">0</owl:minCardinality>
			</owl:Restriction>
		</rdfs:subClassOf>
		<rdfs:subClassOf>
			<owl:Restriction>
				<owl:onProperty rdf:resource="&auto-vc;partReplaced"/>
				<owl:minCardinality rdf:datatype="&xsd;nonNegativeInteger">0</owl:minCardinality>
			</owl:Restriction>
		</rdfs:subClassOf>
		<rdfs:subClassOf>
			<owl:Restriction>
				<owl:onProperty rdf:resource="&auto-vc;carriedOutBy"/>
				<owl:onClass>
					<owl:Class>
						<owl:unionOf rdf:parseType="Collection">
							<rdf:Description rdf:about="&auto-vc;BusinessEntity">
							</rdf:Description>
							<rdf:Description rdf:about="&auto-vc;BusinessEntityType">
							</rdf:Description>
						</owl:unionOf>
					</owl:Class>
				</owl:onClass>
				<owl:minQualifiedCardinality rdf:datatype="&xsd;nonNegativeInteger">0</owl:minQualifiedCardinality>
			</owl:Restriction>
		</rdfs:subClassOf>
		<rdfs:subClassOf>
			<owl:Restriction>
				<owl:onProperty rdf:resource="&auto-vc;airbagDeployment"/>
				<owl:minQualifiedCardinality rdf:datatype="&xsd;nonNegativeInteger">0</owl:minQualifiedCardinality>
				<owl:onDataRange rdf:resource="&xsd;boolean"/>
			</owl:Restriction>
		</rdfs:subClassOf>
		<rdfs:subClassOf>
			<owl:Restriction>
				<owl:onProperty rdf:resource="&auto-vc;notAtFaultAccident"/>
				<owl:minQualifiedCardinality rdf:datatype="&xsd;nonNegativeInteger">0</owl:minQualifiedCardinality>
				<owl:onDataRange rdf:resource="&xsd;boolean"/>
			</owl:Restriction>
		</rdfs:subClassOf>
		<rdfs:subClassOf>
			<owl:Restriction>
				<owl:onProperty rdf:resource="&auto-vc;originalPartsOnly"/>
				<owl:minQualifiedCardinality rdf:datatype="&xsd;nonNegativeInteger">0</owl:minQualifiedCardinality>
				<owl:onDataRange rdf:resource="&xsd;boolean"/>
			</owl:Restriction>
		</rdfs:subClassOf>
		<rdfs:subClassOf>
			<owl:Restriction>
				<owl:onProperty rdf:resource="&auto-vc;repaired"/>
				<owl:minQualifiedCardinality rdf:datatype="&xsd;nonNegativeInteger">0</owl:minQualifiedCardinality>
				<owl:onDataRange rdf:resource="&xsd;boolean"/>
			</owl:Restriction>
		</rdfs:subClassOf>
		<rdfs:subClassOf>
			<owl:Restriction>
				<owl:onProperty rdf:resource="&auto-vc;structuralDamage"/>
				<owl:minQualifiedCardinality rdf:datatype="&xsd;nonNegativeInteger">0</owl:minQualifiedCardinality>
				<owl:onDataRange rdf:resource="&xsd;boolean"/>
			</owl:Restriction>
		</rdfs:subClassOf>
		<rdfs:label xml:lang="en">modification or maintenance</rdfs:label>
		<rdfs:comment xml:lang="en">Typical examples are the replacement of the engine or the installation of a trailor-hitch.</rdfs:comment>
		<rdfs:isDefinedBy rdf:resource="http://purl.org/uco/ns#"/>
		<skos:definition xml:lang="en">an event in which a part of the vehicle is being replaced or removed, or a new part is being added.</skos:definition>
	</owl:Class>
	
	<owl:NamedIndividual rdf:about="&auto-vc;MoneyBack">
		<rdfs:label xml:lang="en">money-back guarantee</rdfs:label>
		<rdfs:isDefinedBy rdf:resource="http://purl.org/uco/ns#"/>
		<skos:definition xml:lang="en">The promise to take back the vehicle without any specific reason for a full refund within a certain amount of time</skos:definition>
	</owl:NamedIndividual>
	
	<owl:Class rdf:about="&auto-vc;Moped">
		<rdfs:subClassOf rdf:resource="&auto-vc;Motorcycle"/>
		<rdfs:label xml:lang="en">moped</rdfs:label>
		<skos:definition xml:lang="en">A speed-limited motor-driven cycle which may be propelled by pedaling.</skos:definition>
		<fibo-fnd-utl-av:adaptedFrom>ANSI D.16-2017, section 2.2.9.4</fibo-fnd-utl-av:adaptedFrom>
	</owl:Class>
	
	<owl:Class rdf:about="&auto-vc;Motor-drivenCycle">
		<rdfs:subClassOf rdf:resource="&auto-vc;Motorcycle"/>
		<rdfs:label xml:lang="en">motor-driven cycle</rdfs:label>
		<skos:definition xml:lang="en">Any motorcycle having an engine with less than 150 cubic centimeters displacement or with 5-brake horsepower or less.</skos:definition>
		<fibo-fnd-utl-av:adaptedFrom>ANSI D.16-2017, section 2.2.9.1</fibo-fnd-utl-av:adaptedFrom>
	</owl:Class>
	
	<owl:Class rdf:about="&auto-vc;MotorBoat">
		<rdfs:subClassOf rdf:resource="&auto-vc;Boat"/>
		<rdfs:label xml:lang="en">motor boat</rdfs:label>
		<rdfs:isDefinedBy rdf:resource="http://purl.org/vso/ns"/>
		<rdfs:seeAlso rdf:resource="http://dbpedia.org/resource/Motorboat"/>
		<rdfs:seeAlso rdf:resource="http://en.wikipedia.org/wiki/Motorboat"/>
		<skos:definition xml:lang="en">a boat which is powered by an engine</skos:definition>
	</owl:Class>
	
	<owl:Class rdf:about="&auto-vc;MotorVehicleIn-transport">
		<rdfs:subClassOf rdf:resource="&auto-mo;Role"/>
		<rdfs:label xml:lang="en">motor vehicle in-transport</rdfs:label>
		<rdfs:comment xml:lang="en">A motor vehicle that is In-transport state.</rdfs:comment>
		<rdfs:comment xml:lang="en">See In-transport</rdfs:comment>
		<skos:definition xml:lang="en">motor vehicle on a roadway or in motion within or outside the trafficway</skos:definition>
		<fibo-fnd-utl-av:adaptedFrom>ANSI D.16-2017, section 2.2.34</fibo-fnd-utl-av:adaptedFrom>
	</owl:Class>
	
	<owl:Class rdf:about="&auto-vc;Motorcycle">
		<rdfs:subClassOf rdf:resource="&auto-vc;MotorizedRoadVehicle"/>
		<rdfs:label xml:lang="pl">motocykl</rdfs:label>
		<rdfs:label xml:lang="en">motorcycle</rdfs:label>
		<rdfs:comment>QName: auto-vc-vc:Motorcycle</rdfs:comment>
		<dct:isPartOf rdf:resource="http://auto.schema.org"/>
		<dct:source rdf:resource="http://www.w3.org/wiki/WebSchemas/SchemaDotOrgSources#Automotive_Ontology_Working_Group"/>
		<sm:directSource rdf:resource="https://schema.org/Motorcycle"/>
		<rdfs:isDefinedBy rdf:resource="http://purl.org/vso/ns"/>
		<rdfs:isDefinedBy rdf:resource="https://spec.edmcouncil.org/auto/ontology/VC/VehicleCore/"/>
		<rdfs:seeAlso rdf:resource="http://dbpedia.org/resource/Motorcycle"/>
		<rdfs:seeAlso rdf:resource="http://en.wikipedia.org/wiki/Motorcycle"/>
		<skos:definition xml:lang="en">Any motor vehicle having a seat or saddle for the use of its operator and designed to travel on not more than three wheels in contact with the ground.</skos:definition>
		<skos:definition xml:lang="en">a single-track, two-wheeled motor vehicle</skos:definition>
		<skos:definition xml:lang="pl">pojazd samochodowy zaopatrzony w silnik spalinowy, dwukołowy lub z bocznym wózkiem – wielośladowy</skos:definition>
		<fibo-fnd-utl-av:adaptedFrom>ANSI D.16-2017, section 2.2.9</fibo-fnd-utl-av:adaptedFrom>
		<fibo-fnd-utl-av:synonym xml:lang="en">motorbike</fibo-fnd-utl-av:synonym>
	</owl:Class>
	
	<owl:Class rdf:about="&auto-vc;MotorizedBicycle">
		<rdfs:subClassOf rdf:resource="&auto-vc;MotorizedRoadVehicle"/>
		<rdfs:label xml:lang="en">motorized bicycle</rdfs:label>
		<dct:isPartOf rdf:resource="http://auto.schema.org"/>
		<dct:source rdf:resource="http://www.w3.org/wiki/WebSchemas/SchemaDotOrgSources#Automotive_Ontology_Working_Group"/>
		<sm:directSource rdf:resource="https://schema.org/MotorizedBicycle"/>
		<rdfs:isDefinedBy rdf:resource="http://purl.org/vso/ns"/>
		<rdfs:seeAlso rdf:resource="http://dbpedia.org/resource/Motorized_bicycle"/>
		<rdfs:seeAlso rdf:resource="http://en.wikipedia.org/wiki/Motorized_bicycle"/>
		<skos:definition xml:lang="en">a bicycle with an attached motor used to power the vehicle, or to assist with pedaling</skos:definition>
	</owl:Class>
	
	<owl:Class rdf:about="&auto-vc;MotorizedRoadVehicle">
		<rdfs:subClassOf rdf:resource="&auto-vc;RoadVehicle"/>
		<rdfs:subClassOf>
			<owl:Restriction>
				<owl:onProperty rdf:resource="&auto-vc;acrissCode"/>
				<owl:minQualifiedCardinality rdf:datatype="&xsd;nonNegativeInteger">0</owl:minQualifiedCardinality>
				<owl:onDataRange rdf:resource="&xsd;string"/>
			</owl:Restriction>
		</rdfs:subClassOf>
		<rdfs:subClassOf>
			<owl:Restriction>
				<owl:onProperty rdf:resource="&auto-vc;insuranceGroup"/>
				<owl:minQualifiedCardinality rdf:datatype="&xsd;nonNegativeInteger">0</owl:minQualifiedCardinality>
				<owl:onDataRange rdf:resource="&xsd;string"/>
			</owl:Restriction>
		</rdfs:subClassOf>
		<rdfs:subClassOf>
			<owl:Restriction>
				<owl:onProperty rdf:resource="&auto-vc;insuranceGroup50"/>
				<owl:minQualifiedCardinality rdf:datatype="&xsd;nonNegativeInteger">0</owl:minQualifiedCardinality>
				<owl:onDataRange rdf:resource="&xsd;string"/>
			</owl:Restriction>
		</rdfs:subClassOf>
		<rdfs:subClassOf>
			<owl:Restriction>
				<owl:onProperty rdf:resource="&auto-vc;productCode"/>
				<owl:minQualifiedCardinality rdf:datatype="&xsd;nonNegativeInteger">0</owl:minQualifiedCardinality>
				<owl:onDataRange rdf:resource="&xsd;string"/>
			</owl:Restriction>
		</rdfs:subClassOf>
		<rdfs:label xml:lang="en">motorized road vehicle</rdfs:label>
		<rdfs:comment xml:lang="en">See 2.2.7.1, 2.2.7.2, 2.2.9 - 2.2.26</rdfs:comment>
		<rdfs:isDefinedBy rdf:resource="http://purl.org/vso/ns"/>
		<rdfs:seeAlso rdf:resource="http://dbpedia.org/resource/Motor_vehicle"/>
		<rdfs:seeAlso rdf:resource="http://en.wikipedia.org/wiki/Motor_vehicle"/>
		<skos:definition xml:lang="en">Any motorized (mechanically or electrically powered) road vehicle not operated on rails.</skos:definition>
		<skos:definition xml:lang="en">a wheeled land vehicle whose main propulsion is provided by an engine or motor</skos:definition>
		<fibo-fnd-utl-av:adaptedFrom>ANSI D.16-2017, section 2.2.7</fibo-fnd-utl-av:adaptedFrom>
	</owl:Class>
	
	<owl:Class rdf:about="&auto-vc;MyCar">
		<rdfs:subClassOf rdf:resource="&auto-mo;Role"/>
		<rdfs:label xml:lang="en">my car</rdfs:label>
		<rdfs:label xml:lang="pl">mój samochód</rdfs:label>
		<rdfs:seeAlso xml:lang="en">source: https://www.toyota-ti.ac.jp/Lab/Denshi/COIN/Ontology/TTICore-0.03/TTICarOnto.owl</rdfs:seeAlso>
		<skos:definition xml:lang="en">vehicle that legally belongs to the subject</skos:definition>
	</owl:Class>
	
	<owl:Class rdf:about="&auto-vc;Offering">
		<rdfs:subClassOf rdf:resource="&auto-mo;GenericallyDependentContinuant"/>
		<rdfs:subClassOf>
			<owl:Class>
				<owl:intersectionOf rdf:parseType="Collection">
					<owl:Restriction>
						<owl:onProperty rdf:resource="&auto-vc;shortSubtitle"/>
						<owl:minQualifiedCardinality rdf:datatype="&xsd;nonNegativeInteger">0</owl:minQualifiedCardinality>
						<owl:onDataRange rdf:resource="&rdf;PlainLiteral"/>
					</owl:Restriction>
					<owl:Restriction>
						<owl:onProperty rdf:resource="&auto-vc;shortSubtitle"/>
						<owl:maxQualifiedCardinality rdf:datatype="&xsd;nonNegativeInteger">1</owl:maxQualifiedCardinality>
						<owl:onDataRange rdf:resource="&rdf;PlainLiteral"/>
					</owl:Restriction>
				</owl:intersectionOf>
			</owl:Class>
		</rdfs:subClassOf>
		<rdfs:subClassOf>
			<owl:Class>
				<owl:intersectionOf rdf:parseType="Collection">
					<owl:Restriction>
						<owl:onProperty rdf:resource="&auto-vc;shortTitle"/>
						<owl:minQualifiedCardinality rdf:datatype="&xsd;nonNegativeInteger">0</owl:minQualifiedCardinality>
						<owl:onDataRange rdf:resource="&rdf;PlainLiteral"/>
					</owl:Restriction>
					<owl:Restriction>
						<owl:onProperty rdf:resource="&auto-vc;shortTitle"/>
						<owl:maxQualifiedCardinality rdf:datatype="&xsd;nonNegativeInteger">1</owl:maxQualifiedCardinality>
						<owl:onDataRange rdf:resource="&rdf;PlainLiteral"/>
					</owl:Restriction>
				</owl:intersectionOf>
			</owl:Class>
		</rdfs:subClassOf>
		<rdfs:subClassOf>
			<owl:Class>
				<owl:intersectionOf rdf:parseType="Collection">
					<owl:Restriction>
						<owl:onProperty rdf:resource="&auto-vc;subtitle"/>
						<owl:minQualifiedCardinality rdf:datatype="&xsd;nonNegativeInteger">0</owl:minQualifiedCardinality>
						<owl:onDataRange rdf:resource="&rdf;PlainLiteral"/>
					</owl:Restriction>
					<owl:Restriction>
						<owl:onProperty rdf:resource="&auto-vc;subtitle"/>
						<owl:maxQualifiedCardinality rdf:datatype="&xsd;nonNegativeInteger">1</owl:maxQualifiedCardinality>
						<owl:onDataRange rdf:resource="&rdf;PlainLiteral"/>
					</owl:Restriction>
				</owl:intersectionOf>
			</owl:Class>
		</rdfs:subClassOf>
		<rdfs:subClassOf>
			<owl:Class>
				<owl:intersectionOf rdf:parseType="Collection">
					<owl:Restriction>
						<owl:onProperty rdf:resource="&auto-vc;termsAndConditions"/>
						<owl:minQualifiedCardinality rdf:datatype="&xsd;nonNegativeInteger">0</owl:minQualifiedCardinality>
						<owl:onDataRange rdf:resource="&rdf;PlainLiteral"/>
					</owl:Restriction>
					<owl:Restriction>
						<owl:onProperty rdf:resource="&auto-vc;termsAndConditions"/>
						<owl:maxQualifiedCardinality rdf:datatype="&xsd;nonNegativeInteger">1</owl:maxQualifiedCardinality>
						<owl:onDataRange rdf:resource="&rdf;PlainLiteral"/>
					</owl:Restriction>
				</owl:intersectionOf>
			</owl:Class>
		</rdfs:subClassOf>
		<rdfs:subClassOf>
			<owl:Class>
				<owl:intersectionOf rdf:parseType="Collection">
					<owl:Restriction>
						<owl:onProperty rdf:resource="&auto-vc;offerPromoCode"/>
						<owl:minQualifiedCardinality rdf:datatype="&xsd;nonNegativeInteger">0</owl:minQualifiedCardinality>
						<owl:onDataRange rdf:resource="&xsd;string"/>
					</owl:Restriction>
					<owl:Restriction>
						<owl:onProperty rdf:resource="&auto-vc;offerPromoCode"/>
						<owl:maxQualifiedCardinality rdf:datatype="&xsd;nonNegativeInteger">1</owl:maxQualifiedCardinality>
						<owl:onDataRange rdf:resource="&xsd;string"/>
					</owl:Restriction>
				</owl:intersectionOf>
			</owl:Class>
		</rdfs:subClassOf>
		<rdfs:label>offering</rdfs:label>
		<skos:definition xml:lang="en">thing offered especially as a gift or contribution</skos:definition>
	</owl:Class>
	
	<owl:Class rdf:about="&auto-vc;OtherBus">
		<rdfs:subClassOf rdf:resource="&auto-vc;Bus"/>
		<rdfs:label xml:lang="en">other bus</rdfs:label>
		<skos:definition xml:lang="en">Any bus used for transportation purposes other than school bus, transit bus, intercity bus or charter bus.</skos:definition>
		<fibo-fnd-utl-av:adaptedFrom>ANSI D.16-2017, section 2.2.10.6</fibo-fnd-utl-av:adaptedFrom>
	</owl:Class>
	
	<owl:Class rdf:about="&auto-vc;OwnershipInfo">
		<rdfs:subClassOf rdf:resource="&auto-mo;Quality"/>
		<rdfs:subClassOf>
			<owl:Restriction>
				<owl:onProperty rdf:resource="&auto-vc;mileageInitial"/>
				<owl:onClass rdf:resource="&auto-mo;QualitativeValue"/>
				<owl:minQualifiedCardinality rdf:datatype="&xsd;nonNegativeInteger">0</owl:minQualifiedCardinality>
			</owl:Restriction>
		</rdfs:subClassOf>
		<rdfs:subClassOf>
			<owl:Restriction>
				<owl:onProperty rdf:resource="&auto-vc;mileageEnd"/>
				<owl:onClass rdf:resource="&auto-mo;QuantitativeValue"/>
				<owl:minQualifiedCardinality rdf:datatype="&xsd;nonNegativeInteger">0</owl:minQualifiedCardinality>
			</owl:Restriction>
		</rdfs:subClassOf>
		<rdfs:subClassOf>
			<owl:Restriction>
				<owl:onProperty rdf:resource="&auto-vc;usage"/>
				<owl:onClass rdf:resource="&auto-vc;CarUsageType"/>
				<owl:minQualifiedCardinality rdf:datatype="&xsd;nonNegativeInteger">0</owl:minQualifiedCardinality>
			</owl:Restriction>
		</rdfs:subClassOf>
		<rdfs:subClassOf>
			<owl:Restriction>
				<owl:onProperty rdf:resource="&auto-vc;contains"/>
				<owl:onClass rdf:resource="&auto-vc;OwnershipInfo"/>
				<owl:minQualifiedCardinality rdf:datatype="&xsd;nonNegativeInteger">0</owl:minQualifiedCardinality>
			</owl:Restriction>
		</rdfs:subClassOf>
		<rdfs:subClassOf>
			<owl:Restriction>
				<owl:onProperty rdf:resource="&auto-vc;parking"/>
				<owl:onClass rdf:resource="&auto-vc;ParkingType"/>
				<owl:minQualifiedCardinality rdf:datatype="&xsd;nonNegativeInteger">0</owl:minQualifiedCardinality>
			</owl:Restriction>
		</rdfs:subClassOf>
		<rdfs:subClassOf>
			<owl:Restriction>
				<owl:onProperty rdf:resource="&auto-vc;pets"/>
				<owl:onClass rdf:resource="&auto-vc;Species"/>
				<owl:minQualifiedCardinality rdf:datatype="&xsd;nonNegativeInteger">0</owl:minQualifiedCardinality>
			</owl:Restriction>
		</rdfs:subClassOf>
		<rdfs:subClassOf>
			<owl:Restriction>
				<owl:onProperty rdf:resource="&auto-vc;mainLocation"/>
				<owl:onClass>
					<owl:Class>
						<owl:unionOf rdf:parseType="Collection">
							<rdf:Description rdf:about="&auto-mo;Location">
							</rdf:Description>
							<rdf:Description rdf:about="&auto-mo;PostalAddress">
							</rdf:Description>
						</owl:unionOf>
					</owl:Class>
				</owl:onClass>
				<owl:minQualifiedCardinality rdf:datatype="&xsd;nonNegativeInteger">0</owl:minQualifiedCardinality>
			</owl:Restriction>
		</rdfs:subClassOf>
		<rdfs:subClassOf>
			<owl:Restriction>
				<owl:onProperty rdf:resource="&auto-vc;currentOwner"/>
				<owl:onClass>
					<owl:Class>
						<owl:unionOf rdf:parseType="Collection">
							<rdf:Description rdf:about="&auto-mo;Organization">
							</rdf:Description>
							<rdf:Description rdf:about="&auto-mo;Person">
							</rdf:Description>
						</owl:unionOf>
					</owl:Class>
				</owl:onClass>
				<owl:minQualifiedCardinality rdf:datatype="&xsd;nonNegativeInteger">0</owl:minQualifiedCardinality>
			</owl:Restriction>
		</rdfs:subClassOf>
		<rdfs:subClassOf>
			<owl:Restriction>
				<owl:onProperty rdf:resource="&auto-vc;owner"/>
				<owl:onClass>
					<owl:Class>
						<owl:unionOf rdf:parseType="Collection">
							<rdf:Description rdf:about="&auto-mo;Organization">
							</rdf:Description>
							<rdf:Description rdf:about="&auto-mo;Person">
							</rdf:Description>
						</owl:unionOf>
					</owl:Class>
				</owl:onClass>
				<owl:minQualifiedCardinality rdf:datatype="&xsd;nonNegativeInteger">0</owl:minQualifiedCardinality>
			</owl:Restriction>
		</rdfs:subClassOf>
		<rdfs:subClassOf>
			<owl:Restriction>
				<owl:onProperty rdf:resource="&auto-vc;smoking"/>
				<owl:minQualifiedCardinality rdf:datatype="&xsd;nonNegativeInteger">0</owl:minQualifiedCardinality>
				<owl:onDataRange rdf:resource="&xsd;boolean"/>
			</owl:Restriction>
		</rdfs:subClassOf>
		<rdfs:subClassOf>
			<owl:Restriction>
				<owl:onProperty rdf:resource="&auto-vc;from"/>
				<owl:minQualifiedCardinality rdf:datatype="&xsd;nonNegativeInteger">0</owl:minQualifiedCardinality>
				<owl:onDataRange rdf:resource="&xsd;dateTime"/>
			</owl:Restriction>
		</rdfs:subClassOf>
		<rdfs:subClassOf>
			<owl:Restriction>
				<owl:onProperty rdf:resource="&auto-vc;to"/>
				<owl:minQualifiedCardinality rdf:datatype="&xsd;nonNegativeInteger">0</owl:minQualifiedCardinality>
				<owl:onDataRange rdf:resource="&xsd;dateTime"/>
			</owl:Restriction>
		</rdfs:subClassOf>
		<rdfs:subClassOf>
			<owl:Restriction>
				<owl:onProperty rdf:resource="&auto-vc;numberOfDrivers"/>
				<owl:minQualifiedCardinality rdf:datatype="&xsd;nonNegativeInteger">0</owl:minQualifiedCardinality>
				<owl:onDataRange rdf:resource="&xsd;integer"/>
			</owl:Restriction>
		</rdfs:subClassOf>
		<rdfs:subClassOf>
			<owl:Restriction>
				<owl:onProperty rdf:resource="&auto-vc;licensePlate"/>
				<owl:minQualifiedCardinality rdf:datatype="&xsd;nonNegativeInteger">0</owl:minQualifiedCardinality>
				<owl:onDataRange rdf:resource="&xsd;string"/>
			</owl:Restriction>
		</rdfs:subClassOf>
		<rdfs:label xml:lang="en">ownership info</rdfs:label>
		<rdfs:isDefinedBy rdf:resource="http://purl.org/uco/ns#"/>
		<skos:definition xml:lang="en">a structured value representing information about the period of ownership of a vehicle by a person or organisation</skos:definition>
	</owl:Class>
	
	<owl:Class rdf:about="&auto-vc;Paint">
		<rdfs:subClassOf rdf:resource="&auto-vc;ChoiceOrComponent"/>
		<rdfs:label xml:lang="en">paint choice or component</rdfs:label>
		<rdfs:isDefinedBy rdf:resource="http://purl.org/vvo/ns#"/>
		<skos:definition xml:lang="en">The class of paint choices or components (a &quot;MonoSelectGroup&quot; in automotive terminology), VW ID: 3</skos:definition>
	</owl:Class>
	
	<owl:Class rdf:about="&auto-vc;ParkedMotorVehicle">
		<rdfs:subClassOf rdf:resource="&auto-mo;Role"/>
		<rdfs:label xml:lang="en">parked motor vehicle</rdfs:label>
		<skos:definition xml:lang="en">A motor vehicle not in- transport, other than a working motor vehicle, that is not in motion and not located on the roadway.</skos:definition>
		<fibo-fnd-utl-av:adaptedFrom>ANSI D.16-2017, section 2.2.34.2</fibo-fnd-utl-av:adaptedFrom>
	</owl:Class>
	
	<owl:Class rdf:about="&auto-vc;Parking">
		<rdfs:subClassOf rdf:resource="&auto-vc;ChoiceOrComponent"/>
		<rdfs:label xml:lang="en">parking choice or component</rdfs:label>
		<rdfs:isDefinedBy rdf:resource="http://purl.org/vvo/ns#"/>
		<skos:definition xml:lang="en">The class of parking-related choices or components (a &quot;MonoSelectGroup&quot; in automotive terminology), VW ID: 7</skos:definition>
	</owl:Class>
	
	<owl:Class rdf:about="&auto-vc;ParkingType">
		<rdfs:subClassOf rdf:resource="&auto-mo;QualitativeValue"/>
		<rdfs:label xml:lang="en">parking type</rdfs:label>
		<rdfs:comment xml:lang="en">You can use DBpedia URIs for additional types.</rdfs:comment>
		<rdfs:isDefinedBy rdf:resource="http://purl.org/uco/ns#"/>
		<skos:definition xml:lang="en">a type of parking for a vehicle, e.g. in a garage, on the street (open-sky), or in a carport</skos:definition>
	</owl:Class>
	
	<owl:Class rdf:about="&auto-vc;PassengerCar">
		<rdfs:subClassOf rdf:resource="&auto-vc;RegularVehicle"/>
		<rdfs:label xml:lang="en">passenger car</rdfs:label>
		<rdfs:label xml:lang="pl">samochód osobowy</rdfs:label>
		<rdfs:seeAlso xml:lang="en">source: https://www.toyota-ti.ac.jp/Lab/Denshi/COIN/Ontology/TTICore-0.03/TTICarOnto.owl</rdfs:seeAlso>
		<skos:definition xml:lang="en">a road motor vehicle, other than a motor cycle, intended for the carriage of passengers and designed to seat no more than nine persons including the driver</skos:definition>
		<skos:definition xml:lang="pl">pojazd samochodowy przeznaczony konstrukcyjnie do przewozu nie więcej niż 9 osób łącznie z kierowcą oraz ich bagażu;</skos:definition>
	</owl:Class>
	
	<owl:Class rdf:about="&auto-vc;PassengerVan">
		<rdfs:subClassOf rdf:resource="&auto-vc;Van"/>
		<rdfs:label xml:lang="en">passenger van</rdfs:label>
		<skos:definition xml:lang="en">Any van where the area behind the driver or cab is designated for carrying passengers.</skos:definition>
		<fibo-fnd-utl-av:adaptedFrom>ANSI D.16-2017, section 2.2.14.1</fibo-fnd-utl-av:adaptedFrom>
	</owl:Class>
	
	<owl:Class rdf:about="&auto-vc;PaymentMethod">
		<rdfs:subClassOf rdf:resource="&auto-mo;QualitativeValue"/>
		<rdfs:label xml:lang="en">payment method</rdfs:label>
		<skos:definition xml:lang="en">value indicating the payment method of a payment</skos:definition>
	</owl:Class>
	
	<owl:Class rdf:about="&auto-vc;Pedalcycle">
		<rdfs:subClassOf rdf:resource="&auto-vc;HumanPoweredLandVehicle"/>
		<rdfs:label xml:lang="en">pedalcycle</rdfs:label>
		<skos:definition xml:lang="en">A non-motorized other road vehicle propelled by pedaling.</skos:definition>
	</owl:Class>
	
	<owl:NamedIndividual rdf:about="&auto-vc;Petrol">
		<rdf:type rdf:resource="&auto-vc;FuelTypeValue"/>
		<rdfs:label xml:lang="en">petrol</rdfs:label>
		<dct:source>vso:FuelTypeValue</dct:source>
		<rdfs:isDefinedBy rdf:resource="http://purl.org/vvo/ns#"/>
		<skos:definition xml:lang="en">Petrol, VW ID: 1</skos:definition>
		<auto-vc:hasID>1</auto-vc:hasID>
	</owl:NamedIndividual>
	
	<owl:Class rdf:about="&auto-vc;PoleTrailer">
		<rdfs:subClassOf rdf:resource="&auto-vc;Trailer"/>
		<rdfs:label xml:lang="en">pole trailer</rdfs:label>
		<skos:definition xml:lang="en">A trailer designed to be attached to the towing road vehicle by means of a reach or pole, or by being boomed or otherwise secured to the towing road vehicle, and ordinarily used for carrying property of a long or irregular shape such as poles, pipes or structural members that are generally capable of sustaining themselves as beams between the supporting connections.</skos:definition>
	</owl:Class>
	
	<owl:Class rdf:about="&auto-vc;PriceSpecification">
		<rdfs:subClassOf rdf:resource="&auto-mo;ValueSpace"/>
		<rdfs:label xml:lang="en">price specification</rdfs:label>
		<skos:definition xml:lang="en">indication of the unit price and delivery or payment charges</skos:definition>
	</owl:Class>
	
	<owl:NamedIndividual rdf:about="&auto-vc;Private">
		<rdf:type rdf:resource="&auto-vc;CarUsageType"/>
		<rdfs:label xml:lang="en">private</rdfs:label>
		<rdfs:isDefinedBy rdf:resource="http://purl.org/uco/ns#"/>
		<skos:definition xml:lang="en">The usage of a vehicle soleley for private purposes</skos:definition>
	</owl:NamedIndividual>
	
	<owl:Class rdf:about="&auto-vc;PropertySpecification">
		<rdfs:subClassOf rdf:resource="&auto-mo;Model"/>
		<rdfs:label xml:lang="en">property speciﬁcation</rdfs:label>
		<rdfs:isDefinedBy rdf:resource="http://purl.org/coo/ns#"/>
		<owl:disjointWith rdf:resource="&auto-vc;SpecItemCollection"/>
		<owl:disjointWith rdf:resource="&auto-vc;Trim"/>
		<skos:definition xml:lang="en">A Property Specification is an abstract entity specifying a set of properties for a vehicle that results from a single choice or the combination of two or more choices and that override the individual properties of the resulting vehicle.

Example 1: Power steering and Air conditioning in combination reduce the available engine power from 90 kW to 89 kW.
Example 2: Choosing the color option &quot;blue&quot; changes the color of the car to &quot;blue&quot;.</skos:definition>
	</owl:Class>
	
	<owl:Class rdf:about="&auto-vc;PulpwoodTrailer">
		<rdfs:subClassOf rdf:resource="&auto-vc;FullTrailer"/>
		<rdfs:label xml:lang="en">pulpwood trailer</rdfs:label>
		<skos:definition xml:lang="en">trailer or semitrailer that is designed exclusively for harvesting logs or pulpwood and constructed with a skeletal frame with no means for attachment of a solid bed, body, or container</skos:definition>
	</owl:Class>
	
	<owl:Class rdf:about="&auto-vc;Quadracycle">
		<rdfs:subClassOf rdf:resource="&auto-vc;Pedalcycle"/>
		<rdfs:label xml:lang="en">quadracycle</rdfs:label>
		<rdfs:isDefinedBy rdf:resource="http://purl.org/vso/ns"/>
		<rdfs:seeAlso rdf:resource="http://dbpedia.org/resource/Quadracycle"/>
		<rdfs:seeAlso rdf:resource="http://en.wikipedia.org/wiki/Quadracycle"/>
		<skos:definition xml:lang="en">a four-wheeled human-powered vehicle. It is also referred to as a quadricycle, quadcycle pedal car or four-wheeled bicycle</skos:definition>
	</owl:Class>
	
	<owl:Class rdf:about="&auto-vc;RailwayTrain">
		<rdfs:subClassOf rdf:resource="&auto-vc;RailwayVehicle"/>
		<rdfs:label xml:lang="en">train</rdfs:label>
		<skos:definition xml:lang="en">Any motorized railway vehicle.</skos:definition>
		<fibo-fnd-utl-av:adaptedFrom>ANSI D.16-2017, section 2.2.5</fibo-fnd-utl-av:adaptedFrom>
	</owl:Class>
	
	<owl:Class rdf:about="&auto-vc;RailwayVehicle">
		<rdfs:subClassOf rdf:resource="&auto-vc;LandVehicle"/>
		<rdfs:label xml:lang="en">railway vehicle</rdfs:label>
		<skos:definition xml:lang="en">Any land vehicle that is (1) designed primarily for, or in use for, moving persons or property from one place to another on rails and (2) not in use on a land way other than a railway.</skos:definition>
		<fibo-fnd-utl-av:adaptedFrom>ANSI D.16-2017, section 2.2.4</fibo-fnd-utl-av:adaptedFrom>
	</owl:Class>
	
	<owl:NamedIndividual rdf:about="&auto-vc;RearWheelDriveConfiguration">
		<rdf:type rdf:resource="&auto-vc;DriveWheelConfigurationValue"/>
		<rdfs:label xml:lang="en">rear-wheel drive</rdfs:label>
		<skos:definition xml:lang="en">Rear-wheel drive is a transmission layout where the engine drives the rear wheels.</skos:definition>
		<fibo-fnd-utl-av:synonym xml:lang="en">RWD</fibo-fnd-utl-av:synonym>
	</owl:NamedIndividual>
	
	<owl:Class rdf:about="&auto-vc;RegularVehicle">
		<rdfs:subClassOf rdf:resource="&auto-vc;Car"/>
		<rdfs:label xml:lang="en">regular vehicle</rdfs:label>
		<rdfs:label xml:lang="pl">zwykły pojazd</rdfs:label>
		<rdfs:seeAlso xml:lang="en">source: https://www.toyota-ti.ac.jp/Lab/Denshi/COIN/Ontology/TTICore-0.03/TTICarOnto.owl</rdfs:seeAlso>
		<skos:definition xml:lang="en">normal vehicle used for daily commuting</skos:definition>
	</owl:Class>
	
	<owl:Class rdf:about="&auto-vc;RelativePriceSpecification">
		<rdfs:subClassOf rdf:resource="&auto-vc;PriceSpecification"/>
		<rdfs:label xml:lang="en">relative price specification</rdfs:label>
		<skos:definition xml:lang="en">relative indication of the unit price and delivery or payment charges</skos:definition>
	</owl:Class>
	
	<owl:NamedIndividual rdf:about="&auto-vc;RentalVehicleUsage">
		<rdf:type rdf:resource="&auto-vc;CarUsageType"/>
		<rdfs:label>rental vehicle usage</rdfs:label>
		<dct:isPartOf rdf:resource="http://auto.schema.org"/>
		<dct:source rdf:resource="http://www.w3.org/wiki/WebSchemas/SchemaDotOrgSources#Automotive_Ontology_Working_Group"/>
		<skos:definition>Indicates the usage of the vehicle as a rental car.</skos:definition>
	</owl:NamedIndividual>
	
	<owl:Class rdf:about="&auto-vc;Rickshaw">
		<rdfs:subClassOf rdf:resource="&auto-vc;Pedalcycle"/>
		<rdfs:label xml:lang="en">rickshaw</rdfs:label>
		<rdfs:isDefinedBy rdf:resource="http://purl.org/vso/ns"/>
		<rdfs:seeAlso rdf:resource="http://dbpedia.org/resource/Rickshaw"/>
		<rdfs:seeAlso rdf:resource="http://en.wikipedia.org/wiki/Rickshaw"/>
		<skos:definition xml:lang="en">a two-wheeled cart which seats one or two persons and is being drawn by a runner</skos:definition>
		<fibo-fnd-utl-av:synonym xml:lang="en">ricksha</fibo-fnd-utl-av:synonym>
	</owl:Class>
	
	<owl:NamedIndividual rdf:about="&auto-vc;RightHandDriving">
		<rdf:type rdf:resource="&auto-vc;SteeringPositionValue"/>
		<rdfs:label xml:lang="en">right hand drive</rdfs:label>
		<skos:definition xml:lang="en">The steering position is on the right side of the vehicle (viewed from the main direction of driving). For cars this means that you drive on the left side of the road.</skos:definition>
	</owl:NamedIndividual>
	
	<owl:Class rdf:about="&auto-vc;RoadVehicle">
		<rdfs:subClassOf rdf:resource="&auto-vc;LandVehicle"/>
		<rdfs:label xml:lang="en">road vehicle</rdfs:label>
		<rdfs:comment xml:lang="en">A superclass of classes addopted from ANSI D.16-2017.</rdfs:comment>
		<skos:definition xml:lang="en">land vehicle other than a railway vehicle</skos:definition>
	</owl:Class>
	
	<owl:Class rdf:about="&auto-vc;Roofs">
		<rdfs:subClassOf rdf:resource="&auto-vc;ChoiceOrComponent"/>
		<rdfs:label xml:lang="en">roofs choice or component</rdfs:label>
		<rdfs:isDefinedBy rdf:resource="http://purl.org/vvo/ns#"/>
		<skos:definition xml:lang="en">The class of roof choices or components (a &quot;MonoSelectGroup&quot; in automotive terminology), VW ID: 5</skos:definition>
	</owl:Class>
	
	<owl:Class rdf:about="&auto-vc;SailingBoat">
		<rdfs:subClassOf rdf:resource="&auto-vc;Boat"/>
		<rdfs:label xml:lang="en">sailing boat</rdfs:label>
		<rdfs:isDefinedBy rdf:resource="http://purl.org/vso/ns"/>
		<rdfs:seeAlso rdf:resource="http://dbpedia.org/resource/Sailboat"/>
		<rdfs:seeAlso rdf:resource="http://en.wikipedia.org/wiki/Sailboat"/>
		<skos:definition xml:lang="en">a boat propelled partly or entirely by sails</skos:definition>
		<fibo-fnd-utl-av:synonym xml:lang="en">sailboat</fibo-fnd-utl-av:synonym>
	</owl:Class>
	
	<owl:Class rdf:about="&auto-vc;SchoolBus">
		<rdfs:subClassOf rdf:resource="&auto-vc;Bus"/>
		<rdfs:label xml:lang="en">school bus</rdfs:label>
		<rdfs:comment xml:lang="en">A motor vehicle is not a school bus while on trips which involve the transportation exclusively of other passengers or exclusively for other purposes. A motor vehicle is a school bus only if it is externally identifiable by the following characteristics : 1.) Its color is yellow, 2.) The words “ school bus &apos;&apos; appear on the front and rear, 3.) Flashing red lights are located on the front and rear, 4.) Lettering on both sides identifies the school or school district served, or the company operating the bus.</rdfs:comment>
		<skos:definition xml:lang="en">A motor vehicle used for the transportation of any school pupil at or below the 12th-grade level to or from a public or private school or school-related activity.</skos:definition>
		<fibo-fnd-utl-av:adaptedFrom>ANSI D.16-2017, section 2.8.1</fibo-fnd-utl-av:adaptedFrom>
	</owl:Class>
	
	<owl:Class rdf:about="&auto-vc;Seats">
		<rdfs:subClassOf rdf:resource="&auto-vc;ChoiceOrComponent"/>
		<rdfs:label xml:lang="en">seats choice or component</rdfs:label>
		<rdfs:isDefinedBy rdf:resource="http://purl.org/vvo/ns#"/>
		<skos:definition xml:lang="en">The class of seat-related choices or components (a &quot;MonoSelectGroup&quot; in automotive terminology), VW ID: 9</skos:definition>
	</owl:Class>
	
	<owl:Class rdf:about="&auto-vc;Semitrailer">
		<rdfs:subClassOf rdf:resource="&auto-vc;Trailer"/>
		<rdfs:label xml:lang="en">semitrailer</rdfs:label>
		<skos:definition xml:lang="en">A trailer, other than a pole trailer, designed for carrying property and so constructed that part of its weight rests upon or is carried by the towing road vehicle.</skos:definition>
		<fibo-fnd-utl-av:adaptedFrom>ANSI D.16-2017, section 2.2.17</fibo-fnd-utl-av:adaptedFrom>
	</owl:Class>
	
	<owl:Class rdf:about="&auto-vc;Ship">
		<rdfs:subClassOf rdf:resource="&auto-vc;Watercraft"/>
		<rdfs:label xml:lang="en">ship</rdfs:label>
		<rdfs:isDefinedBy rdf:resource="http://purl.org/vso/ns"/>
		<rdfs:seeAlso rdf:resource="http://dbpedia.org/resource/Ship"/>
		<rdfs:seeAlso rdf:resource="http://en.wikipedia.org/wiki/Ship"/>
		<skos:definition xml:lang="en">a large watercraft that floats on water</skos:definition>
	</owl:Class>
	
	<owl:Class rdf:about="&auto-vc;SingleUnitTruck">
		<rdfs:subClassOf rdf:resource="&auto-vc;Truck"/>
		<rdfs:label xml:lang="en">single unit truck</rdfs:label>
		<rdfs:comment xml:lang="en">When connected to a trailer, such a device may be part of a truck combination.</rdfs:comment>
		<skos:definition xml:lang="en">A truck consisting primarily of a single motorized transport device designed for carrying property.</skos:definition>
		<fibo-fnd-utl-av:adaptedFrom>ANSI D.16-2017, section 2.2.19</fibo-fnd-utl-av:adaptedFrom>
	</owl:Class>
	
	<owl:Class rdf:about="&auto-vc;SmallBus">
		<rdfs:subClassOf rdf:resource="&auto-vc;Bus"/>
		<rdfs:label xml:lang="en">small bus</rdfs:label>
		<skos:definition xml:lang="en">A bus with seating for nine to fifteen persons, including the driver.</skos:definition>
	</owl:Class>
	
	<owl:Class rdf:about="&auto-vc;SmallSpecialVehicle">
		<rdfs:subClassOf rdf:resource="&auto-vc;SpecialVehicle"/>
		<rdfs:label xml:lang="pl">mały pojazd specjalny</rdfs:label>
		<rdfs:label xml:lang="en">small special vehicle</rdfs:label>
		<rdfs:seeAlso>source: https://www.toyota-ti.ac.jp/Lab/Denshi/COIN/Ontology/TTICore-0.03/TTICarOnto.owl</rdfs:seeAlso>
		<skos:definition xml:lang="en">special vehicle which is considered small</skos:definition>
	</owl:Class>
	
	<owl:Class rdf:about="&auto-vc;SpecItemCollection">
		<rdfs:subClassOf rdf:resource="&auto-mo;GenericallyDependentContinuant"/>
		<rdfs:subClassOf>
			<owl:Class>
				<owl:intersectionOf rdf:parseType="Collection">
					<owl:Restriction>
						<owl:onProperty rdf:resource="&auto-vc;default"/>
						<owl:onClass rdf:resource="&auto-vc;ChoiceOrComponent"/>
						<owl:minQualifiedCardinality rdf:datatype="&xsd;nonNegativeInteger">0</owl:minQualifiedCardinality>
					</owl:Restriction>
					<owl:Restriction>
						<owl:onProperty rdf:resource="&auto-vc;default"/>
						<owl:onClass rdf:resource="&auto-vc;ChoiceOrComponent"/>
						<owl:maxQualifiedCardinality rdf:datatype="&xsd;nonNegativeInteger">1</owl:maxQualifiedCardinality>
					</owl:Restriction>
				</owl:intersectionOf>
			</owl:Class>
		</rdfs:subClassOf>
		<rdfs:subClassOf>
			<owl:Class>
				<owl:intersectionOf rdf:parseType="Collection">
					<owl:Restriction>
						<owl:onProperty rdf:resource="&auto-vc;displayPos"/>
						<owl:minQualifiedCardinality rdf:datatype="&xsd;nonNegativeInteger">0</owl:minQualifiedCardinality>
						<owl:onDataRange rdf:resource="&xsd;int"/>
					</owl:Restriction>
					<owl:Restriction>
						<owl:onProperty rdf:resource="&auto-vc;displayPos"/>
						<owl:maxQualifiedCardinality rdf:datatype="&xsd;nonNegativeInteger">1</owl:maxQualifiedCardinality>
						<owl:onDataRange rdf:resource="&xsd;int"/>
					</owl:Restriction>
				</owl:intersectionOf>
			</owl:Class>
		</rdfs:subClassOf>
		<rdfs:subClassOf>
			<owl:Class>
				<owl:intersectionOf rdf:parseType="Collection">
					<owl:Restriction>
						<owl:onProperty rdf:resource="&auto-vc;max"/>
						<owl:minQualifiedCardinality rdf:datatype="&xsd;nonNegativeInteger">0</owl:minQualifiedCardinality>
						<owl:onDataRange rdf:resource="&xsd;int"/>
					</owl:Restriction>
					<owl:Restriction>
						<owl:onProperty rdf:resource="&auto-vc;max"/>
						<owl:maxQualifiedCardinality rdf:datatype="&xsd;nonNegativeInteger">1</owl:maxQualifiedCardinality>
						<owl:onDataRange rdf:resource="&xsd;int"/>
					</owl:Restriction>
				</owl:intersectionOf>
			</owl:Class>
		</rdfs:subClassOf>
		<rdfs:subClassOf>
			<owl:Class>
				<owl:intersectionOf rdf:parseType="Collection">
					<owl:Restriction>
						<owl:onProperty rdf:resource="&auto-vc;min"/>
						<owl:minQualifiedCardinality rdf:datatype="&xsd;nonNegativeInteger">0</owl:minQualifiedCardinality>
						<owl:onDataRange rdf:resource="&xsd;int"/>
					</owl:Restriction>
					<owl:Restriction>
						<owl:onProperty rdf:resource="&auto-vc;min"/>
						<owl:maxQualifiedCardinality rdf:datatype="&xsd;nonNegativeInteger">1</owl:maxQualifiedCardinality>
						<owl:onDataRange rdf:resource="&xsd;int"/>
					</owl:Restriction>
				</owl:intersectionOf>
			</owl:Class>
		</rdfs:subClassOf>
		<rdfs:subClassOf>
			<owl:Restriction>
				<owl:onProperty rdf:resource="&auto-vc;availableChoice"/>
				<owl:someValuesFrom rdf:resource="&auto-vc;ChoiceOrComponent"/>
			</owl:Restriction>
		</rdfs:subClassOf>
		<rdfs:label xml:lang="en">spec item collection</rdfs:label>
		<rdfs:isDefinedBy rdf:resource="http://purl.org/coo/ns#"/>
		<owl:disjointWith rdf:resource="&auto-vc;Trim"/>
		<skos:definition xml:lang="en">A Spec Item Collection is an entity collating multiple coo:ChoiceOrComponent options for a given coo:Derivative, i.e. the available configurational choices. 
The default choice can be indicated using a coo:default link. All other choices are attached using coo:availableChoice. The number of coo:ChoiceOrComponent items that can / must be selected for a valid configuration are indicated via coo:min and coo:max.</skos:definition>
	</owl:Class>
	
	<owl:Class rdf:about="&auto-vc;SpecialVehicle">
		<rdfs:subClassOf rdf:resource="&auto-vc;Car"/>
		<rdfs:label xml:lang="pl">pojazd specjalny</rdfs:label>
		<rdfs:label xml:lang="en">special vehicle</rdfs:label>
		<rdfs:seeAlso xml:lang="en">source: https://www.toyota-ti.ac.jp/Lab/Denshi/COIN/Ontology/TTICore-0.03/TTICarOnto.owl</rdfs:seeAlso>
		<skos:definition xml:lang="en">a vehicle or trailer intended to perform a special function requiring body adjustments or special equipment; this vehicle is capable of carrying persons and objects associated with the performance of this function</skos:definition>
		<skos:definition xml:lang="pl">pojazd samochodowy lub przyczepa przeznaczone do wykonywania specjalnej funkcji, która powoduje konieczność dostosowania nadwozia lub posiadania specjalnego wyposażenia; w pojeździe tym mogą być przewożone osoby i rzeczy związane z wykonywaniem tej funkcji</skos:definition>
	</owl:Class>
	
	<owl:Class rdf:about="&auto-vc;Species">
		<rdfs:subClassOf rdf:resource="&auto-mo;QualitativeValue"/>
		<rdfs:label xml:lang="en">species</rdfs:label>
		<rdfs:comment xml:lang="en">If possible, use DBPedia URIs, e.g. http://dbpedia.org/resource/Dog.</rdfs:comment>
		<rdfs:isDefinedBy rdf:resource="http://purl.org/uco/ns#"/>
		<skos:definition xml:lang="en">typically a pet, for indicating the type of animals that were regularly transported in the vehicle</skos:definition>
	</owl:Class>
	
	<owl:Class rdf:about="&auto-vc;Speed-limitedMotor-drivenCycle">
		<rdfs:subClassOf rdf:resource="&auto-vc;Motorcycle"/>
		<rdfs:label xml:lang="en">speed-limited motor-driven cycle</rdfs:label>
		<skos:definition xml:lang="en">Any motor- driven cycle which : 1.) will not attain a speed of more than 30 miles per hour (48 kilometers per hour) in one mile (1.609 kilometers) from a standing start, 2.) has an engine with not more than 50 cubic centimeters displacement or with 2-brake horsepower or less, and 3.) has a power drive system which does not require its operator to shift gears.</skos:definition>
		<fibo-fnd-utl-av:adaptedFrom>ANSI D.16-2017, section 2.2.9.3</fibo-fnd-utl-av:adaptedFrom>
	</owl:Class>
	
	<owl:Class rdf:about="&auto-vc;SpeedInterval">
		<rdfs:subClassOf rdf:resource="&auto-mo;QuantitativeValueFloat"/>
		<rdfs:label xml:lang="en">speed interval</rdfs:label>
		<rdfs:isDefinedBy rdf:resource="http://purl.org/vso/ns"/>
		<skos:definition xml:lang="en">a value indicating a speed interval, mostly for explaining acceleration data</skos:definition>
	</owl:Class>
	
	<owl:Class rdf:about="&auto-vc;SteeringPositionValue">
		<rdfs:subClassOf rdf:resource="&auto-mo;QualitativeValue"/>
		<rdfs:label xml:lang="en">steering position value</rdfs:label>
		<dct:isPartOf rdf:resource="http://auto.schema.org"/>
		<dct:source rdf:resource="http://www.w3.org/wiki/WebSchemas/SchemaDotOrgSources#Automotive_Ontology_Working_Group"/>
		<sm:directSource rdf:resource="https://schema.org/SteeringPositionValue"/>
		<rdfs:isDefinedBy rdf:resource="http://purl.org/vso/ns"/>
		<skos:definition xml:lang="en">a value indicating a steering position</skos:definition>
	</owl:Class>
	
	<owl:Class rdf:about="&auto-vc;SteeringWheels">
		<rdfs:subClassOf rdf:resource="&auto-vc;ChoiceOrComponent"/>
		<rdfs:label xml:lang="en">steering wheels choice or component</rdfs:label>
		<rdfs:isDefinedBy rdf:resource="http://purl.org/vvo/ns#"/>
		<skos:definition xml:lang="en">The class of steering wheels choices or components (a &quot;MonoSelectGroup&quot; in automotive terminology), VW ID: 6</skos:definition>
	</owl:Class>
	
	<owl:Class rdf:about="&auto-vc;StraddleTrailer">
		<rdfs:subClassOf rdf:resource="&auto-vc;FullTrailer"/>
		<rdfs:label xml:lang="en">straddle trailer</rdfs:label>
		<skos:definition xml:lang="en">trailer that is designed to transport bulk agricultural commodities from the harvesting location, as evidenced by a framework that is driven over the cargo and lifting arms that suspend the cargo for transit</skos:definition>
	</owl:Class>
	
	<owl:NamedIndividual rdf:about="&auto-vc;Street">
		<rdf:type rdf:resource="&auto-vc;ParkingType"/>
		<rdfs:label xml:lang="en">street</rdfs:label>
		<rdfs:isDefinedBy rdf:resource="http://purl.org/uco/ns#"/>
		<skos:definition xml:lang="en">The parking of a vehicle on a public or private street</skos:definition>
	</owl:NamedIndividual>
	
	<owl:NamedIndividual rdf:about="&auto-vc;TT4SpeedAuto">
		<rdf:type rdf:resource="&auto-vc;TransmissionTypeValueAutomatic"/>
		<rdfs:label xml:lang="en">4 speed auto</rdfs:label>
		<dct:source>vvo:TransmissionTypeValueAutomatic</dct:source>
		<rdfs:isDefinedBy rdf:resource="http://purl.org/vvo/ns#"/>
		<skos:definition xml:lang="en">4 Speed auto. VW ID: 1</skos:definition>
		<auto-vc:gearboxTypeId>1</auto-vc:gearboxTypeId>
		<auto-vc:hasID>1</auto-vc:hasID>
	</owl:NamedIndividual>
	
	<owl:NamedIndividual rdf:about="&auto-vc;TT5SpeedAutoDSG">
		<rdf:type rdf:resource="&auto-vc;TransmissionTypeValueAutomatic"/>
		<rdfs:label xml:lang="en">5 speed auto DSG</rdfs:label>
		<dct:source>vvo:TransmissionTypeValueAutomatic</dct:source>
		<rdfs:isDefinedBy rdf:resource="http://purl.org/vvo/ns#"/>
		<skos:definition xml:lang="en">5 Speed auto DSG, VW ID: 8</skos:definition>
		<auto-vc:gearboxTypeId>3</auto-vc:gearboxTypeId>
		<auto-vc:hasID>8</auto-vc:hasID>
	</owl:NamedIndividual>
	
	<owl:NamedIndividual rdf:about="&auto-vc;TT5SpeedAutoTiptronic">
		<rdf:type rdf:resource="&auto-vc;TransmissionTypeValueAutomatic"/>
		<rdfs:label xml:lang="en">5 speed auto tiptronic</rdfs:label>
		<dct:source>vvo:TransmissionTypeValueAutomatic</dct:source>
		<rdfs:isDefinedBy rdf:resource="http://purl.org/vvo/ns#"/>
		<skos:definition xml:lang="en">5 Speed auto tiptronic, VW ID: 3</skos:definition>
		<auto-vc:gearboxTypeId>2</auto-vc:gearboxTypeId>
		<auto-vc:hasID>3</auto-vc:hasID>
	</owl:NamedIndividual>
	
	<owl:NamedIndividual rdf:about="&auto-vc;TT5SpeedManual">
		<rdf:type rdf:resource="&auto-vc;TransmissionTypeValueManual"/>
		<rdfs:label xml:lang="en">5 speed manual</rdfs:label>
		<dct:source>vvo:TransmissionTypeValueManual</dct:source>
		<rdfs:isDefinedBy rdf:resource="http://purl.org/vvo/ns#"/>
		<skos:definition xml:lang="en">5 Speed manual, VW ID: 2</skos:definition>
		<auto-vc:gearboxTypeId>1</auto-vc:gearboxTypeId>
		<auto-vc:hasID>2</auto-vc:hasID>
	</owl:NamedIndividual>
	
	<owl:NamedIndividual rdf:about="&auto-vc;TT6SpeedAuto">
		<rdf:type rdf:resource="&auto-vc;TransmissionTypeValueAutomatic"/>
		<rdfs:label xml:lang="en">6 speed auto</rdfs:label>
		<dct:source>vvo:TransmissionTypeValueAutomatic</dct:source>
		<rdfs:isDefinedBy rdf:resource="http://purl.org/vvo/ns#"/>
		<skos:definition xml:lang="en">6 Speed auto, VW ID: 5</skos:definition>
		<auto-vc:gearboxTypeId>2</auto-vc:gearboxTypeId>
		<auto-vc:hasID>5</auto-vc:hasID>
	</owl:NamedIndividual>
	
	<owl:NamedIndividual rdf:about="&auto-vc;TT6SpeedAutoDSG">
		<rdf:type rdf:resource="&auto-vc;TransmissionTypeValueAutomatic"/>
		<rdfs:label xml:lang="en">6 speed auto DSG</rdfs:label>
		<dct:source>vvo:TransmissionTypeValueAutomatic</dct:source>
		<rdfs:isDefinedBy rdf:resource="http://purl.org/vvo/ns#"/>
		<skos:definition xml:lang="en">6 Speed auto DSG, VW ID: 6</skos:definition>
		<auto-vc:gearboxTypeId>3</auto-vc:gearboxTypeId>
		<auto-vc:hasID>6</auto-vc:hasID>
	</owl:NamedIndividual>
	
	<owl:NamedIndividual rdf:about="&auto-vc;TT6SpeedAutoTiptronic">
		<rdf:type rdf:resource="&auto-vc;TransmissionTypeValueAutomatic"/>
		<rdfs:label xml:lang="en">6 speed auto tiptronic</rdfs:label>
		<dct:source>vvo:TransmissionTypeValueAutomatic</dct:source>
		<rdfs:isDefinedBy rdf:resource="http://purl.org/vvo/ns#"/>
		<skos:definition xml:lang="en">6 Speed auto tiptronic, VW ID: 7</skos:definition>
		<auto-vc:gearboxTypeId>2</auto-vc:gearboxTypeId>
		<auto-vc:hasID>7</auto-vc:hasID>
	</owl:NamedIndividual>
	
	<owl:NamedIndividual rdf:about="&auto-vc;TT6SpeedManual">
		<rdf:type rdf:resource="&auto-vc;TransmissionTypeValueManual"/>
		<rdfs:label xml:lang="en">6 speed manual</rdfs:label>
		<dct:source>vvo:TransmissionTypeValueManual</dct:source>
		<rdfs:isDefinedBy rdf:resource="http://purl.org/vvo/ns#"/>
		<skos:definition xml:lang="en">6 Speed manual, VW ID: 4</skos:definition>
		<auto-vc:gearboxTypeId>1</auto-vc:gearboxTypeId>
		<auto-vc:hasID>4</auto-vc:hasID>
	</owl:NamedIndividual>
	
	<owl:NamedIndividual rdf:about="&auto-vc;TT7SpeedAutoDSG">
		<rdf:type rdf:resource="&auto-vc;TransmissionTypeValueAutomatic"/>
		<rdfs:label xml:lang="en">7 speed auto DSG</rdfs:label>
		<dct:source>vvo:TransmissionTypeValueAutomatic</dct:source>
		<rdfs:isDefinedBy rdf:resource="http://purl.org/vvo/ns#"/>
		<skos:definition xml:lang="en">7 Speed auto DSG, VW ID: 9</skos:definition>
		<auto-vc:gearboxTypeId>3</auto-vc:gearboxTypeId>
		<auto-vc:hasID>9</auto-vc:hasID>
	</owl:NamedIndividual>
	
	<owl:NamedIndividual rdf:about="&auto-vc;TT8SpeedAuto">
		<rdf:type rdf:resource="&auto-vc;TransmissionTypeValueAutomatic"/>
		<rdfs:label xml:lang="en">8 speed auto</rdfs:label>
		<dct:source>vvo:TransmissionTypeValueAutomatic</dct:source>
		<rdfs:isDefinedBy rdf:resource="http://purl.org/vvo/ns#"/>
		<skos:definition xml:lang="en">8 Speed auto, VW ID: 10</skos:definition>
		<auto-vc:gearboxTypeId>2</auto-vc:gearboxTypeId>
		<auto-vc:hasID>10</auto-vc:hasID>
	</owl:NamedIndividual>
	
	<owl:NamedIndividual rdf:about="&auto-vc;TTUnspecified">
		<rdf:type rdf:resource="&auto-vc;TransmissionTypeValue"/>
		<rdfs:label xml:lang="en">unspecified</rdfs:label>
		<dct:source>vso:TransmissionTypeValue</dct:source>
		<rdfs:isDefinedBy rdf:resource="http://purl.org/vvo/ns#"/>
		<skos:definition xml:lang="en">Unspecified, VW ID: 0</skos:definition>
		<auto-vc:gearboxTypeId>1</auto-vc:gearboxTypeId>
		<auto-vc:hasID>0</auto-vc:hasID>
	</owl:NamedIndividual>
	
	<owl:NamedIndividual rdf:about="&auto-vc;TaxiVehicleUsage">
		<rdf:type rdf:resource="&auto-vc;CarUsageType"/>
		<rdfs:label>taxi vehicle usage</rdfs:label>
		<dct:isPartOf rdf:resource="http://auto.schema.org"/>
		<dct:source rdf:resource="http://www.w3.org/wiki/WebSchemas/SchemaDotOrgSources#Automotive_Ontology_Working_Group"/>
		<skos:definition>Indicates the usage of the car as a taxi.</skos:definition>
	</owl:NamedIndividual>
	
	<owl:Class rdf:about="&auto-vc;Three-wheeledMotorcycle">
		<rdfs:subClassOf rdf:resource="&auto-vc;Motorcycle"/>
		<rdfs:label xml:lang="en">three-wheeled motorcycle</rdfs:label>
		<skos:definition xml:lang="en">Any motor vehicle having a seat or saddle for the use of its operator, and having three wheels in contact with the ground.</skos:definition>
		<fibo-fnd-utl-av:adaptedFrom>ANSI D.16-2017, section 2.2.9.6</fibo-fnd-utl-av:adaptedFrom>
	</owl:Class>
	
	<owl:Class rdf:about="&auto-vc;TractorPoleTrailer">
		<rdfs:subClassOf rdf:resource="&auto-vc;PoleTrailer"/>
		<rdfs:label xml:lang="en">tractor pole trailer</rdfs:label>
		<skos:definition xml:lang="en">combination vehicle that carries logs lengthwise so that they form the body of the vehicle</skos:definition>
	</owl:Class>
	
	<owl:Class rdf:about="&auto-vc;TrafficPattern">
		<rdfs:subClassOf rdf:resource="&auto-mo;QualitativeValue"/>
		<rdfs:label xml:lang="en">traffic pattern value</rdfs:label>
		<rdfs:isDefinedBy rdf:resource="http://purl.org/vvo/ns#"/>
		<skos:definition xml:lang="en">A value indicating a traffic pattern, to be used as a reference for vso:fuelConsumption or vso:fuelEconomy</skos:definition>
	</owl:Class>
	
	<owl:Class rdf:about="&auto-vc;Trailer">
		<rdfs:subClassOf rdf:resource="&auto-vc;RoadVehicle"/>
		<rdfs:label xml:lang="en">trailer</rdfs:label>
		<skos:definition xml:lang="en">A road vehicle designed to be drawn by another road vehicle.</skos:definition>
		<fibo-fnd-utl-av:adaptedFrom>ANSI D.16-2017, section 2.2.15</fibo-fnd-utl-av:adaptedFrom>
	</owl:Class>
	
	<owl:Class rdf:about="&auto-vc;TransitBus">
		<rdfs:subClassOf rdf:resource="&auto-vc;Bus"/>
		<rdfs:label xml:lang="en">transit bus</rdfs:label>
		<skos:definition xml:lang="en">A bus used for passenger transportation over fixed, scheduled routes within primarily urban geographical areas.</skos:definition>
		<fibo-fnd-utl-av:adaptedFrom>ANSI D.16-2017, section 2.2.10.3</fibo-fnd-utl-av:adaptedFrom>
	</owl:Class>
	
	<owl:Class rdf:about="&auto-vc;TransmissionTypeValue">
		<rdfs:subClassOf rdf:resource="&auto-mo;QualitativeValue"/>
		<rdfs:subClassOf>
			<owl:Class>
				<owl:intersectionOf rdf:parseType="Collection">
					<owl:Restriction>
						<owl:onProperty rdf:resource="&auto-vc;gearboxTypeId"/>
						<owl:minQualifiedCardinality rdf:datatype="&xsd;nonNegativeInteger">0</owl:minQualifiedCardinality>
						<owl:onDataRange rdf:resource="&xsd;string"/>
					</owl:Restriction>
					<owl:Restriction>
						<owl:onProperty rdf:resource="&auto-vc;gearboxTypeId"/>
						<owl:maxQualifiedCardinality rdf:datatype="&xsd;nonNegativeInteger">1</owl:maxQualifiedCardinality>
						<owl:onDataRange rdf:resource="&xsd;string"/>
					</owl:Restriction>
				</owl:intersectionOf>
			</owl:Class>
		</rdfs:subClassOf>
		<rdfs:label xml:lang="en">transmission type value</rdfs:label>
		<rdfs:comment xml:lang="en">You can safely use any reasonable DBPedia URI, e.g. 
  http://dbpedia.org/resource/Manual_transmission
  http://dbpedia.org/resource/Automatic_transmission</rdfs:comment>
		<rdfs:isDefinedBy rdf:resource="http://purl.org/vso/ns"/>
		<skos:definition xml:lang="en">a value indicating a type of transmission</skos:definition>
	</owl:Class>
	
	<owl:Class rdf:about="&auto-vc;TransmissionTypeValueAutomatic">
		<rdfs:subClassOf rdf:resource="&auto-vc;TransmissionTypeValue"/>
		<rdfs:label xml:lang="en">transmission type value automatic</rdfs:label>
		<rdfs:isDefinedBy rdf:resource="http://purl.org/vvo/ns#"/>
		<skos:definition xml:lang="en">The class of all automatic transmission types</skos:definition>
	</owl:Class>
	
	<owl:Class rdf:about="&auto-vc;TransmissionTypeValueManual">
		<rdfs:subClassOf rdf:resource="&auto-vc;TransmissionTypeValue"/>
		<rdfs:label xml:lang="en">transmission type value manual</rdfs:label>
		<rdfs:isDefinedBy rdf:resource="http://purl.org/vvo/ns#"/>
		<skos:definition xml:lang="en">The class of all manual transmission types</skos:definition>
	</owl:Class>
	
	<owl:Class rdf:about="&auto-vc;TransportVehicle">
		<rdfs:subClassOf rdf:resource="&auto-vc;SpecialVehicle"/>
		<rdfs:label xml:lang="en">transport vehicle</rdfs:label>
		<rdfs:comment xml:lang="en">Such devices or animals shall include at least one of the following : 1.) A transport device, or a unit, made up of connected transport devices, while idle or in use, for moving persons or property from one place to another, 2.) An animal or team of animals while in use for moving person or property other than the animal or team itself from one place to another, or 3.) A movable device such as construction, farm or industrial machinery outside the confines of a building and its premises while in use for moving persons, the device itself, or other property from one place to another.</rdfs:comment>
		<skos:definition xml:lang="en">Consists of one or more devices or animals and their load.</skos:definition>
		<fibo-fnd-utl-av:adaptedFrom>ANSI D.16-2017, section 2.1.4</fibo-fnd-utl-av:adaptedFrom>
	</owl:Class>
	
	<owl:Class rdf:about="&auto-vc;Trim">
		<rdfs:subClassOf rdf:resource="&auto-mo;Model"/>
		<rdfs:subClassOf>
			<owl:Restriction>
				<owl:onProperty rdf:resource="&auto-vc;hasDerivative"/>
				<owl:onClass rdf:resource="&auto-vc;Derivative"/>
				<owl:minQualifiedCardinality rdf:datatype="&xsd;nonNegativeInteger">0</owl:minQualifiedCardinality>
			</owl:Restriction>
		</rdfs:subClassOf>
		<rdfs:label xml:lang="en">trim</rdfs:label>
		<rdfs:isDefinedBy rdf:resource="http://purl.org/coo/ns#"/>
		<skos:definition xml:lang="en">A Trim is an abstract entity specifying (1) the basic features plus (2) a set of configuration choices (mostly non-functional) of a group of vehicles. 
A Trim should be linked to its Base Model via gr:isVariantOf, if available.

Examples: VW Golf S, VW Polo Match, VW Passat SE</skos:definition>
	</owl:Class>
	
	<owl:Class rdf:about="&auto-vc;Truck">
		<rdfs:subClassOf rdf:resource="&auto-vc;LargeSpecialVehicle"/>
		<rdfs:subClassOf rdf:resource="&auto-vc;TransportVehicle"/>
		<rdfs:label xml:lang="pl">samochód ciężarowy</rdfs:label>
		<rdfs:label xml:lang="en">truck</rdfs:label>
		<rdfs:comment>QName: auto-vc-vc:Truck</rdfs:comment>
		<rdfs:comment xml:lang="pl">pojazd samochodowy przeznaczony konstrukcyjnie do przewozu ładunków</rdfs:comment>
		<rdfs:isDefinedBy rdf:resource="http://purl.org/vso/ns"/>
		<rdfs:isDefinedBy rdf:resource="https://spec.edmcouncil.org/auto/ontology/VC/VehicleCore/"/>
		<rdfs:seeAlso rdf:resource="http://dbpedia.org/resource/Truck"/>
		<rdfs:seeAlso rdf:resource="http://en.wikipedia.org/wiki/Truck"/>
		<skos:definition xml:lang="en">A motor vehicle designed primarily for carrying property.</skos:definition>
		<skos:definition xml:lang="en">a motor vehicle designed to transport cargo</skos:definition>
		<fibo-fnd-utl-av:adaptedFrom>ANSI D.16-2017, section 2.2.13</fibo-fnd-utl-av:adaptedFrom>
		<fibo-fnd-utl-av:synonym xml:lang="en">lorry</fibo-fnd-utl-av:synonym>
	</owl:Class>
	
	<owl:Class rdf:about="&auto-vc;TruckCombination">
		<rdfs:subClassOf rdf:resource="&auto-vc;Truck"/>
		<rdfs:label xml:lang="en">truck combination</rdfs:label>
		<skos:definition xml:lang="en">A truck consisting primarily of a transport device which is a single- unit truck or truck tractor together with one or more attached trailers.</skos:definition>
		<fibo-fnd-utl-av:adaptedFrom>ANSI D.16-2017, section 2.2.21</fibo-fnd-utl-av:adaptedFrom>
	</owl:Class>
	
	<owl:Class rdf:about="&auto-vc;TruckTractor">
		<rdfs:subClassOf rdf:resource="&auto-vc;Truck"/>
		<rdfs:label xml:lang="en">truck tractor</rdfs:label>
		<skos:definition xml:lang="en">A motor vehicle consisting of a single motorized transport device designed primarily for drawing trailers.</skos:definition>
		<fibo-fnd-utl-av:adaptedFrom>ANSI D.16-2017, section 2.2.20</fibo-fnd-utl-av:adaptedFrom>
	</owl:Class>
	
	<owl:NamedIndividual rdf:about="&auto-vc;TwoStrokeMixture">
		<rdf:type rdf:resource="&auto-vc;FuelTypeValue"/>
		<rdfs:label xml:lang="en">two-stroke mixture</rdfs:label>
		<rdfs:isDefinedBy rdf:resource="http://purl.org/vso/ns"/>
		<skos:definition xml:lang="en">A pre-mixed fuel-oil mixture</skos:definition>
	</owl:NamedIndividual>
	
	<owl:Class rdf:about="&auto-vc;Upholstery">
		<rdfs:subClassOf rdf:resource="&auto-vc;ChoiceOrComponent"/>
		<rdfs:label xml:lang="en">upholstery choice or component</rdfs:label>
		<rdfs:isDefinedBy rdf:resource="http://purl.org/vvo/ns#"/>
		<skos:definition xml:lang="en">The class of upholstery choices or components (a &quot;MonoSelectGroup&quot; in automotive terminology), VW ID: 4</skos:definition>
	</owl:Class>
	
	<owl:NamedIndividual rdf:about="&auto-vc;Urban">
		<rdf:type rdf:resource="&auto-vc;TrafficPattern"/>
		<rdfs:label xml:lang="en">urban</rdfs:label>
		<dct:source>vvo:TrafficPattern</dct:source>
		<rdfs:isDefinedBy rdf:resource="http://purl.org/vvo/ns#"/>
		<skos:definition xml:lang="en">Urban usage as a traffic pattern</skos:definition>
	</owl:NamedIndividual>
	
	<owl:Class rdf:about="&auto-vc;UtilityVehicle">
		<rdfs:subClassOf rdf:resource="&auto-vc;SpecialVehicle"/>
		<rdfs:label xml:lang="en">utility vehicle</rdfs:label>
		<rdfs:comment xml:lang="en">These vehicles are generally four wheel-drive (4 x 4) and have increased ground clearance. A utility vehicle typically has a gross vehicle weight rating (GVWR) of 10,000 pounds or less. Utility vehicles with wheelbases greater than 88 inches are classified by overall width. The wheelbase and overall width should be rounded to the nearest inch.</rdfs:comment>
		<skos:definition xml:lang="en">A motor vehicle other than a motorcycle or large bus consisting primarily of a transport device designed for carrying persons, and generally considered a multi-purpose vehicle that is designed to have off-road capabilities.</skos:definition>
	</owl:Class>
	
	<owl:Class rdf:about="&auto-vc;Van">
		<rdfs:subClassOf rdf:resource="&auto-vc;SmallSpecialVehicle"/>
		<rdfs:label xml:lang="en">van</rdfs:label>
		<rdfs:comment xml:lang="en">Vans are classified by size based on frame type and overall vehicle body width. Before classification, vehicle width should be rounded to the nearest inch.</rdfs:comment>
		<rdfs:isDefinedBy rdf:resource="http://purl.org/vso/ns"/>
		<rdfs:seeAlso rdf:resource="http://dbpedia.org/resource/Van"/>
		<rdfs:seeAlso rdf:resource="http://en.wikipedia.org/wiki/Van"/>
		<skos:definition xml:lang="en">A gross vehicle weight rating (GVWR) of 10,000 pounds or less and is basically a “ box on wheels ” that is identifiable by its enclosed passenger and/or cargo area, step-up floor, and relatively short (or nonexistent) hood.</skos:definition>
		<skos:definition xml:lang="en">a kind of vehicle used for transporting  goods or groups of people. It is usually a box-shaped vehicle on four wheels, about the same width and length as a large automobile, but taller and usually higher off the ground, also referred to as a light commercial vehicle or LCV.</skos:definition>
		<fibo-fnd-utl-av:adaptedFrom>ANSI D.16-2017, section 2.2.14</fibo-fnd-utl-av:adaptedFrom>
	</owl:Class>
	
	<owl:Class rdf:about="&auto-vc;Van-basedBus">
		<rdfs:subClassOf rdf:resource="&auto-vc;Van"/>
		<rdfs:label xml:lang="en">van-based bus</rdfs:label>
		<skos:definition xml:lang="en">Any passenger van designed for carrying nine or more persons, including the driver.</skos:definition>
		<fibo-fnd-utl-av:adaptedFrom>ANSI D.16-2017, section 2.2.14.4</fibo-fnd-utl-av:adaptedFrom>
	</owl:Class>
	
	<owl:Class rdf:about="&auto-vc;Van-basedMotorhome">
		<rdfs:subClassOf rdf:resource="&auto-vc;Van"/>
		<rdfs:label xml:lang="en">van-based motorhome</rdfs:label>
		<skos:definition xml:lang="en">Any van where a frame-mounted recreational unit is added behind the driver or cab area.</skos:definition>
		<fibo-fnd-utl-av:adaptedFrom>ANSI D.16-2017, section 2.2.14.3</fibo-fnd-utl-av:adaptedFrom>
	</owl:Class>
	
	<owl:Class rdf:about="&auto-vc;Vehicle">
		<rdfs:subClassOf rdf:resource="&auto-mo;Object"/>
		<rdfs:subClassOf>
			<owl:Restriction>
				<owl:onProperty rdf:resource="&auto-vc;condition"/>
				<owl:minCardinality rdf:datatype="&xsd;nonNegativeInteger">0</owl:minCardinality>
			</owl:Restriction>
		</rdfs:subClassOf>
		<rdfs:subClassOf>
			<owl:Restriction>
				<owl:onProperty rdf:resource="&auto-vc;knownVehicleDamages"/>
				<owl:minCardinality rdf:datatype="&xsd;nonNegativeInteger">0</owl:minCardinality>
			</owl:Restriction>
		</rdfs:subClassOf>
		<rdfs:subClassOf>
			<owl:Restriction>
				<owl:onProperty rdf:resource="&auto-vc;cargoVolume"/>
				<owl:onClass rdf:resource="&auto-mo;QuantitativeValue"/>
				<owl:minQualifiedCardinality rdf:datatype="&xsd;nonNegativeInteger">0</owl:minQualifiedCardinality>
			</owl:Restriction>
		</rdfs:subClassOf>
		<rdfs:subClassOf>
			<owl:Restriction>
				<owl:onProperty rdf:resource="&auto-vc;accelerationTime"/>
				<owl:onClass rdf:resource="&auto-mo;QuantitativeValueFloat"/>
				<owl:minQualifiedCardinality rdf:datatype="&xsd;nonNegativeInteger">0</owl:minQualifiedCardinality>
			</owl:Restriction>
		</rdfs:subClassOf>
		<rdfs:subClassOf>
			<owl:Restriction>
				<owl:onProperty rdf:resource="&auto-vc;usage"/>
				<owl:onClass rdf:resource="&auto-vc;CarUsageType"/>
				<owl:minQualifiedCardinality rdf:datatype="&xsd;nonNegativeInteger">0</owl:minQualifiedCardinality>
			</owl:Restriction>
		</rdfs:subClassOf>
		<rdfs:subClassOf>
			<owl:Restriction>
				<owl:onProperty rdf:resource="&auto-vc;hasOwnershipInfo"/>
				<owl:onClass rdf:resource="&auto-vc;OwnershipInfo"/>
				<owl:minQualifiedCardinality rdf:datatype="&xsd;nonNegativeInteger">0</owl:minQualifiedCardinality>
			</owl:Restriction>
		</rdfs:subClassOf>
		<rdfs:subClassOf>
			<owl:Restriction>
				<owl:onProperty rdf:resource="&auto-vc;parking"/>
				<owl:onClass rdf:resource="&auto-vc;ParkingType"/>
				<owl:minQualifiedCardinality rdf:datatype="&xsd;nonNegativeInteger">0</owl:minQualifiedCardinality>
			</owl:Restriction>
		</rdfs:subClassOf>
		<rdfs:subClassOf>
			<owl:Restriction>
				<owl:onProperty rdf:resource="&auto-vc;listPrice"/>
				<owl:onClass rdf:resource="&auto-vc;PriceSpecification"/>
				<owl:minQualifiedCardinality rdf:datatype="&xsd;nonNegativeInteger">0</owl:minQualifiedCardinality>
			</owl:Restriction>
		</rdfs:subClassOf>
		<rdfs:subClassOf>
			<owl:Restriction>
				<owl:onProperty rdf:resource="&auto-vc;valuation"/>
				<owl:onClass rdf:resource="&auto-vc;PriceSpecification"/>
				<owl:minQualifiedCardinality rdf:datatype="&xsd;nonNegativeInteger">0</owl:minQualifiedCardinality>
			</owl:Restriction>
		</rdfs:subClassOf>
		<rdfs:subClassOf>
			<owl:Restriction>
				<owl:onProperty rdf:resource="&auto-vc;pets"/>
				<owl:onClass rdf:resource="&auto-vc;Species"/>
				<owl:minQualifiedCardinality rdf:datatype="&xsd;nonNegativeInteger">0</owl:minQualifiedCardinality>
			</owl:Restriction>
		</rdfs:subClassOf>
		<rdfs:subClassOf>
			<owl:Restriction>
				<owl:onProperty rdf:resource="&auto-vc;currentLocation"/>
				<owl:onClass>
					<owl:Class>
						<owl:unionOf rdf:parseType="Collection">
							<rdf:Description rdf:about="&auto-mo;Location">
							</rdf:Description>
							<rdf:Description rdf:about="&auto-mo;PostalAddress">
							</rdf:Description>
						</owl:unionOf>
					</owl:Class>
				</owl:onClass>
				<owl:minQualifiedCardinality rdf:datatype="&xsd;nonNegativeInteger">0</owl:minQualifiedCardinality>
			</owl:Restriction>
		</rdfs:subClassOf>
		<rdfs:subClassOf>
			<owl:Restriction>
				<owl:onProperty rdf:resource="&auto-vc;currentOwner"/>
				<owl:onClass>
					<owl:Class>
						<owl:unionOf rdf:parseType="Collection">
							<rdf:Description rdf:about="&auto-mo;Organization">
							</rdf:Description>
							<rdf:Description rdf:about="&auto-mo;Person">
							</rdf:Description>
						</owl:unionOf>
					</owl:Class>
				</owl:onClass>
				<owl:minQualifiedCardinality rdf:datatype="&xsd;nonNegativeInteger">0</owl:minQualifiedCardinality>
			</owl:Restriction>
		</rdfs:subClassOf>
		<rdfs:subClassOf>
			<owl:Restriction>
				<owl:onProperty rdf:resource="&auto-vc;owner"/>
				<owl:onClass>
					<owl:Class>
						<owl:unionOf rdf:parseType="Collection">
							<rdf:Description rdf:about="&auto-mo;Organization">
							</rdf:Description>
							<rdf:Description rdf:about="&auto-mo;Person">
							</rdf:Description>
						</owl:unionOf>
					</owl:Class>
				</owl:onClass>
				<owl:minQualifiedCardinality rdf:datatype="&xsd;nonNegativeInteger">0</owl:minQualifiedCardinality>
			</owl:Restriction>
		</rdfs:subClassOf>
		<rdfs:subClassOf>
			<owl:Restriction>
				<owl:onProperty rdf:resource="&auto-vc;shortSubtitle"/>
				<owl:minQualifiedCardinality rdf:datatype="&xsd;nonNegativeInteger">0</owl:minQualifiedCardinality>
				<owl:onDataRange rdf:resource="&rdf;PlainLiteral"/>
			</owl:Restriction>
		</rdfs:subClassOf>
		<rdfs:subClassOf>
			<owl:Restriction>
				<owl:onProperty rdf:resource="&auto-vc;shortTitle"/>
				<owl:minQualifiedCardinality rdf:datatype="&xsd;nonNegativeInteger">0</owl:minQualifiedCardinality>
				<owl:onDataRange rdf:resource="&rdf;PlainLiteral"/>
			</owl:Restriction>
		</rdfs:subClassOf>
		<rdfs:subClassOf>
			<owl:Restriction>
				<owl:onProperty rdf:resource="&auto-vc;subtitle"/>
				<owl:minQualifiedCardinality rdf:datatype="&xsd;nonNegativeInteger">0</owl:minQualifiedCardinality>
				<owl:onDataRange rdf:resource="&rdf;PlainLiteral"/>
			</owl:Restriction>
		</rdfs:subClassOf>
		<rdfs:subClassOf>
			<owl:Restriction>
				<owl:onProperty rdf:resource="&auto-vc;termsAndConditions"/>
				<owl:minQualifiedCardinality rdf:datatype="&xsd;nonNegativeInteger">0</owl:minQualifiedCardinality>
				<owl:onDataRange rdf:resource="&rdf;PlainLiteral"/>
			</owl:Restriction>
		</rdfs:subClassOf>
		<rdfs:subClassOf>
			<owl:Restriction>
				<owl:onProperty rdf:resource="&auto-vc;indicationOfOdometerRollback"/>
				<owl:minQualifiedCardinality rdf:datatype="&xsd;nonNegativeInteger">0</owl:minQualifiedCardinality>
				<owl:onDataRange rdf:resource="&xsd;boolean"/>
			</owl:Restriction>
		</rdfs:subClassOf>
		<rdfs:subClassOf>
			<owl:Restriction>
				<owl:onProperty rdf:resource="&auto-vc;rentalUsage"/>
				<owl:minQualifiedCardinality rdf:datatype="&xsd;nonNegativeInteger">0</owl:minQualifiedCardinality>
				<owl:onDataRange rdf:resource="&xsd;boolean"/>
			</owl:Restriction>
		</rdfs:subClassOf>
		<rdfs:subClassOf>
			<owl:Restriction>
				<owl:onProperty rdf:resource="&auto-vc;repaired"/>
				<owl:minQualifiedCardinality rdf:datatype="&xsd;nonNegativeInteger">0</owl:minQualifiedCardinality>
				<owl:onDataRange rdf:resource="&xsd;boolean"/>
			</owl:Restriction>
		</rdfs:subClassOf>
		<rdfs:subClassOf>
			<owl:Restriction>
				<owl:onProperty rdf:resource="&auto-vc;smoking"/>
				<owl:minQualifiedCardinality rdf:datatype="&xsd;nonNegativeInteger">0</owl:minQualifiedCardinality>
				<owl:onDataRange rdf:resource="&xsd;boolean"/>
			</owl:Restriction>
		</rdfs:subClassOf>
		<rdfs:subClassOf>
			<owl:Restriction>
				<owl:onProperty rdf:resource="&auto-vc;structuralDamage"/>
				<owl:minQualifiedCardinality rdf:datatype="&xsd;nonNegativeInteger">0</owl:minQualifiedCardinality>
				<owl:onDataRange rdf:resource="&xsd;boolean"/>
			</owl:Restriction>
		</rdfs:subClassOf>
		<rdfs:subClassOf>
			<owl:Restriction>
				<owl:onProperty rdf:resource="&auto-vc;purchaseDate"/>
				<owl:minQualifiedCardinality rdf:datatype="&xsd;nonNegativeInteger">0</owl:minQualifiedCardinality>
				<owl:onDataRange rdf:resource="&xsd;dateTime"/>
			</owl:Restriction>
		</rdfs:subClassOf>
		<rdfs:subClassOf>
			<owl:Restriction>
				<owl:onProperty rdf:resource="&auto-vc;vehicleModelDate"/>
				<owl:minQualifiedCardinality rdf:datatype="&xsd;nonNegativeInteger">0</owl:minQualifiedCardinality>
				<owl:onDataRange rdf:resource="&xsd;dateTime"/>
			</owl:Restriction>
		</rdfs:subClassOf>
		<rdfs:subClassOf>
			<owl:Restriction>
				<owl:onProperty rdf:resource="&auto-vc;numberOfDrivers"/>
				<owl:minQualifiedCardinality rdf:datatype="&xsd;nonNegativeInteger">0</owl:minQualifiedCardinality>
				<owl:onDataRange rdf:resource="&xsd;integer"/>
			</owl:Restriction>
		</rdfs:subClassOf>
		<rdfs:subClassOf>
			<owl:Restriction>
				<owl:onProperty rdf:resource="&auto-vc;numberOfOwners"/>
				<owl:minQualifiedCardinality rdf:datatype="&xsd;nonNegativeInteger">0</owl:minQualifiedCardinality>
				<owl:onDataRange rdf:resource="&xsd;integer"/>
			</owl:Restriction>
		</rdfs:subClassOf>
		<rdfs:subClassOf>
			<owl:Restriction>
				<owl:onProperty rdf:resource="&auto-vc;knownVehicleDamages"/>
				<owl:minQualifiedCardinality rdf:datatype="&xsd;nonNegativeInteger">0</owl:minQualifiedCardinality>
				<owl:onDataRange rdf:resource="&xsd;string"/>
			</owl:Restriction>
		</rdfs:subClassOf>
		<rdfs:subClassOf>
			<owl:Restriction>
				<owl:onProperty rdf:resource="&auto-vc;airbagDeployment"/>
				<owl:onDataRange rdf:resource="&xsd;boolean"/>
				<owl:qualifiedCardinality rdf:datatype="&xsd;nonNegativeInteger">1</owl:qualifiedCardinality>
			</owl:Restriction>
		</rdfs:subClassOf>
		<rdfs:subClassOf>
			<owl:Restriction>
				<owl:onProperty rdf:resource="&auto-vc;marketingName"/>
				<owl:someValuesFrom rdf:resource="&xsd;string"/>
			</owl:Restriction>
		</rdfs:subClassOf>
		<rdfs:label xml:lang="pl">pojazd</rdfs:label>
		<rdfs:label xml:lang="en">vehicle</rdfs:label>
		<dct:isPartOf rdf:resource="http://auto.schema.org"/>
		<dct:source rdf:resource="http://www.w3.org/wiki/WebSchemas/SchemaDotOrgSources#Automotive_Ontology_Working_Group"/>
		<sm:directSource rdf:resource="https://schema.org/Vehicle"/>
		<rdfs:isDefinedBy rdf:resource="http://purl.org/vso/ns"/>
		<rdfs:seeAlso rdf:resource="http://dbpedia.org/resource/Vehicle"/>
		<rdfs:seeAlso rdf:resource="http://en.wikipedia.org/wiki/Vehicle"/>
		<skos:definition xml:lang="en">a device that is designed or used to transport people or cargo over land, water, air, or through space</skos:definition>
	</owl:Class>
	
	<owl:Class rdf:about="&auto-vc;WarrantyScope">
		<rdfs:subClassOf rdf:resource="&auto-mo;GenericallyDependentContinuant"/>
		<rdfs:label>warranty scope</rdfs:label>
		<skos:definition xml:lang="en">period of time during which the warranty is valid</skos:definition>
	</owl:Class>
	
	<owl:Class rdf:about="&auto-vc;Watercraft">
		<rdfs:subClassOf rdf:resource="&auto-vc;Vehicle"/>
		<rdfs:label xml:lang="en">watercraft</rdfs:label>
		<rdfs:isDefinedBy rdf:resource="http://purl.org/vso/ns"/>
		<rdfs:seeAlso rdf:resource="http://dbpedia.org/resource/Watercraft"/>
		<rdfs:seeAlso rdf:resource="http://en.wikipedia.org/wiki/Watercraft"/>
		<skos:definition xml:lang="en">A transport vehicle designed primarily for, or in use for, moving persons or property on or through, and supported by, water from one place to another.</skos:definition>
		<skos:definition xml:lang="en">a vehicle, vessel or craft designed to move across or through water</skos:definition>
		<fibo-fnd-utl-av:adaptedFrom>ANSI D.16-2017, section 2.1.6</fibo-fnd-utl-av:adaptedFrom>
	</owl:Class>
	
	<owl:Class rdf:about="&auto-vc;Wheels">
		<rdfs:subClassOf rdf:resource="&auto-vc;ChoiceOrComponent"/>
		<rdfs:label xml:lang="en">wheels choice or component</rdfs:label>
		<rdfs:isDefinedBy rdf:resource="http://purl.org/vvo/ns#"/>
		<skos:definition xml:lang="en">The class of wheels-related choices or components (a &quot;MonoSelectGroup&quot; in automotive terminology), VW ID: 2</skos:definition>
	</owl:Class>
	
	<owl:Class rdf:about="&auto-vc;WorkingMotorVehicle">
		<rdfs:subClassOf rdf:resource="&auto-mo;Role"/>
		<rdfs:label xml:lang="en">working motor vehicle</rdfs:label>
		<rdfs:comment xml:lang="en">This &quot;work&quot; may be located within open or closed portions of the trafficway and motor vehicles performing these activities can be within or outside of the trafficway boundaries.</rdfs:comment>
		<skos:definition xml:lang="en">A motor vehicle in the act of performing construction, maintenance or utility work related to the trafficway.</skos:definition>
		<fibo-fnd-utl-av:adaptedFrom>ANSI D.16-2017, section 2.2.7.2.</fibo-fnd-utl-av:adaptedFrom>
	</owl:Class>
	
	<owl:ObjectProperty rdf:about="&auto-vc;accelerationTime">
		<rdfs:label xml:lang="en">acceleration time</rdfs:label>
		<dct:isPartOf rdf:resource="http://auto.schema.org"/>
		<dct:source rdf:resource="http://www.w3.org/wiki/WebSchemas/SchemaDotOrgSources#Automotive_Ontology_Working_Group"/>
		<rdfs:domain rdf:resource="&auto-vc;Vehicle"/>
		<rdfs:range rdf:resource="&auto-mo;QuantitativeValueFloat"/>
		<skos:definition>The time needed to accelerate the vehicle from a given start velocity to a given target velocity.&lt;br/&gt;&lt;br/&gt;

Typical unit code(s): SEC for seconds&lt;br/&gt;&lt;br/&gt;

&lt;ul&gt;
&lt;li&gt;Note: There are unfortunately no standard unit codes for seconds/0..100 km/h or seconds/0..60 mph. Simply use &quot;SEC&quot; for seconds and indicate the velocities in the &lt;a class=&quot;localLink&quot; href=&quot;http://schema.org/name&quot;&gt;name&lt;/a&gt; of the &lt;a class=&quot;localLink&quot; href=&quot;http://schema.org/QuantitativeValue&quot;&gt;QuantitativeValue&lt;/a&gt;, or use &lt;a class=&quot;localLink&quot; href=&quot;http://schema.org/valueReference&quot;&gt;valueReference&lt;/a&gt; with a &lt;a class=&quot;localLink&quot; href=&quot;http://schema.org/QuantitativeValue&quot;&gt;QuantitativeValue&lt;/a&gt; of 0..60 mph or 0..100 km/h to specify the reference speeds.&lt;/li&gt;
&lt;/ul&gt;</skos:definition>
	</owl:ObjectProperty>
	
	<owl:DatatypeProperty rdf:about="&auto-vc;acrissCode">
		<rdfs:label xml:lang="en">acriss code</rdfs:label>
		<dct:isPartOf rdf:resource="http://auto.schema.org"/>
		<dct:source rdf:resource="http://www.w3.org/wiki/WebSchemas/SchemaDotOrgSources#Automotive_Ontology_Working_Group"/>
		<rdfs:domain rdf:resource="&auto-vc;MotorizedRoadVehicle"/>
		<rdfs:domain>
			<owl:Class>
				<owl:unionOf rdf:parseType="Collection">
					<rdf:Description rdf:about="&auto-vc;Bus">
					</rdf:Description>
					<rdf:Description rdf:about="&auto-vc;Car">
					</rdf:Description>
				</owl:unionOf>
			</owl:Class>
		</rdfs:domain>
		<rdfs:isDefinedBy rdf:resource="http://purl.org/vso/ns"/>
		<rdfs:range rdf:resource="&xsd;string"/>
		<rdfs:seeAlso rdf:resource="http://dbpedia.org/resource/ACRISS_Car_Classification_Code"/>
		<rdfs:seeAlso rdf:resource="http://en.wikipedia.org/wiki/ACRISS_Car_Classification_Code"/>
		<skos:definition xml:lang="en">The ACRISS Car Classification Code is a code used by many car rental companies, for classifying vehicles. ACRISS stands for Association of Car Rental Industry Systems and Standards.</skos:definition>
		<skos:definition>The ACRISS Car Classification Code is a code used by many car rental companies, for classifying vehicles. ACRISS stands for Association of Car Rental Industry Systems and Standards.</skos:definition>
	</owl:DatatypeProperty>
	
	<owl:ObjectProperty rdf:about="&auto-vc;advancedPayment">
		<rdfs:label xml:lang="en">advanced payment</rdfs:label>
		<rdfs:domain rdf:resource="&auto-vc;Financing"/>
		<rdfs:isDefinedBy rdf:resource="http://purl.org/vvo/ns#"/>
		<rdfs:range rdf:resource="&auto-vc;PriceSpecification"/>
		<skos:definition xml:lang="en">Indicates the advanced payment for the financing</skos:definition>
	</owl:ObjectProperty>
	
	<owl:DatatypeProperty rdf:about="&auto-vc;airbagDeployment">
		<rdfs:label xml:lang="en">airbag deployment</rdfs:label>
		<rdfs:domain>
			<owl:Class>
				<owl:unionOf rdf:parseType="Collection">
					<rdf:Description rdf:about="&auto-vc;DamageOrAccident">
					</rdf:Description>
					<rdf:Description rdf:about="&auto-vc;Vehicle">
					</rdf:Description>
				</owl:unionOf>
			</owl:Class>
		</rdfs:domain>
		<rdfs:isDefinedBy rdf:resource="http://purl.org/uco/ns#"/>
		<rdfs:range rdf:resource="&xsd;boolean"/>
		<skos:definition xml:lang="en">This property indicates whether at least one of the airbags of the vehicle has been deployed in the respective accident (when attached to uco:DamageOrAccident) or ever (when directly applied to a vso:Vehicle).</skos:definition>
	</owl:DatatypeProperty>
	
	<owl:DatatypeProperty rdf:about="&auto-vc;apr">
		<rdfs:label xml:lang="en">apr</rdfs:label>
		<rdfs:domain rdf:resource="&auto-vc;Financing"/>
		<rdfs:isDefinedBy rdf:resource="http://purl.org/vvo/ns#"/>
		<rdfs:range rdf:resource="&xsd;decimal"/>
		<skos:definition xml:lang="en">Annual percentage rate. Note: 7.5 % is encoded as &quot;7.5&quot;^^xsd:decimal, not &quot;0.075&quot;^^xsd:decimal.</skos:definition>
	</owl:DatatypeProperty>
	
	<owl:ObjectProperty rdf:about="&auto-vc;availableChoice">
		<rdfs:label xml:lang="en">available choice</rdfs:label>
		<rdfs:domain rdf:resource="&auto-vc;SpecItemCollection"/>
		<rdfs:isDefinedBy rdf:resource="http://purl.org/coo/ns#"/>
		<rdfs:range rdf:resource="&auto-vc;ChoiceOrComponent"/>
		<skos:definition xml:lang="en">This property links available Choices or Components to a Spec Item.</skos:definition>
	</owl:ObjectProperty>
	
	<owl:ObjectProperty rdf:about="&auto-vc;bodyStyle">
		<rdfs:subPropertyOf rdf:resource="&owl;topObjectProperty"/>
		<rdfs:comment xml:lang="en">body style</rdfs:comment>
		<rdfs:label xml:lang="en">body type</rdfs:label>
		<dct:isPartOf rdf:resource="http://auto.schema.org"/>
		<dct:source rdf:resource="http://www.w3.org/wiki/WebSchemas/SchemaDotOrgSources#Automotive_Ontology_Working_Group"/>
		<rdfs:isDefinedBy rdf:resource="http://purl.org/vso/ns"/>
		<rdfs:range rdf:resource="&auto-vc;BodyStyleValue"/>
		<rdfs:seeAlso rdf:resource="http://en.wikipedia.org/wiki/Car_body_styles"/>
		<skos:definition>Indicates the design and body style of the vehicle (e.g. station wagon, hatchback, etc.).</skos:definition>
		<skos:definition xml:lang="en">Indicates the design and body style of the vehicle. 

Use DBPedia resources to indicate the features, if possible. Popular identifiers are
  http://dbpedia.org/resource/Convertible
  http://dbpedia.org/resource/Hatchback
  http://dbpedia.org/resource/Station_wagon
  http://dbpedia.org/resource/Sport_utility_vehicle
  http://dbpedia.org/resource/Roadster

See also http://en.wikipedia.org/wiki/Car_body_styles.

If you cannot find a suitable identifier in DBPedia, define your own as an instance of vso:BodyStyleValue.</skos:definition>
	</owl:ObjectProperty>
	
	<owl:DatatypeProperty rdf:about="&auto-vc;capCode">
		<rdfs:label xml:lang="en">cap code</rdfs:label>
		<rdfs:domain rdf:resource="&auto-vc;Derivative"/>
		<rdfs:isDefinedBy rdf:resource="http://purl.org/vvo/ns#"/>
		<rdfs:range rdf:resource="&xsd;string"/>
		<skos:definition xml:lang="en">The CAP code</skos:definition>
	</owl:DatatypeProperty>
	
	<owl:ObjectProperty rdf:about="&auto-vc;cargoVolume">
		<rdfs:label xml:lang="en">cargo volume</rdfs:label>
		<dct:isPartOf rdf:resource="http://auto.schema.org"/>
		<dct:source rdf:resource="http://www.w3.org/wiki/WebSchemas/SchemaDotOrgSources#Automotive_Ontology_Working_Group"/>
		<rdfs:domain rdf:resource="&auto-vc;Vehicle"/>
		<rdfs:range rdf:resource="&auto-mo;QuantitativeValueFloat"/>
		<skos:definition>The available volume for cargo or luggage. For automobiles, this is usually the trunk volume.

Typical unit code(s): LTR for liters, FTQ for cubic foot/feet

Note: You can use minValue and maxValue to indicate ranges.</skos:definition>
	</owl:ObjectProperty>
	
	<owl:ObjectProperty rdf:about="&auto-vc;carriedOutBy">
		<rdfs:label xml:lang="en">carried out by</rdfs:label>
		<rdfs:domain>
			<owl:Class>
				<owl:unionOf rdf:parseType="Collection">
					<rdf:Description rdf:about="&auto-vc;Check">
					</rdf:Description>
					<rdf:Description rdf:about="&auto-vc;DamageOrAccident">
					</rdf:Description>
					<rdf:Description rdf:about="&auto-vc;ModificationOrMaintenance">
					</rdf:Description>
				</owl:unionOf>
			</owl:Class>
		</rdfs:domain>
		<rdfs:isDefinedBy rdf:resource="http://purl.org/uco/ns#"/>
		<rdfs:range>
			<owl:Class>
				<owl:unionOf rdf:parseType="Collection">
					<rdf:Description rdf:about="&auto-vc;BusinessEntity">
					</rdf:Description>
					<rdf:Description rdf:about="&auto-vc;BusinessEntityType">
					</rdf:Description>
				</owl:unionOf>
			</owl:Class>
		</rdfs:range>
		<skos:definition xml:lang="en">The business or type of business that carried out the check, repair, maintenance, or modification</skos:definition>
	</owl:ObjectProperty>
	
	<owl:DatatypeProperty rdf:about="&auto-vc;color">
		<rdfs:subPropertyOf rdf:resource="&owl;topDataProperty"/>
		<rdfs:label xml:lang="en">color</rdfs:label>
		<rdfs:domain rdf:resource="&auto-vc;Vehicle"/>
		<rdfs:isDefinedBy rdf:resource="http://purl.org/vso/ns"/>
		<rdfs:range rdf:resource="&rdfs;Literal"/>
		<skos:definition xml:lang="en">The color of the vehicle</skos:definition>
	</owl:DatatypeProperty>
	
	<owl:ObjectProperty rdf:about="&auto-vc;compatibility">
		<rdfs:label xml:lang="en">compatibility</rdfs:label>
		<rdfs:domain rdf:resource="&auto-vc;Derivative"/>
		<rdfs:isDefinedBy rdf:resource="http://purl.org/coo/ns#"/>
		<rdfs:range rdf:resource="&auto-vc;ConfigurationInfo"/>
		<skos:definition xml:lang="en">Links from a Derivative to information on whether a particular configuration is valid (true) or invalid (false)</skos:definition>
	</owl:ObjectProperty>
	
	<owl:ObjectProperty rdf:about="&auto-vc;compatibleWith">
		<rdf:type rdf:resource="&owl;SymmetricProperty"/>
		<rdfs:label xml:lang="en">compatible with</rdfs:label>
		<rdfs:domain rdf:resource="&auto-vc;ChoiceOrComponent"/>
		<rdfs:isDefinedBy rdf:resource="http://purl.org/coo/ns#"/>
		<rdfs:range rdf:resource="&auto-vc;ChoiceOrComponent"/>
		<skos:definition xml:lang="en">Indicates that two Choices or Components are compatible with each other.

Note: This property is symmetric, i.e., if A is compatible with B, then B is also compatible with A.</skos:definition>
	</owl:ObjectProperty>
	
	<owl:DatatypeProperty rdf:about="&auto-vc;condition">
		<rdfs:label xml:lang="en">condition</rdfs:label>
		<rdfs:domain rdf:resource="&auto-vc;Vehicle"/>
		<rdfs:isDefinedBy rdf:resource="http://purl.org/vso/ns"/>
		<rdfs:range rdf:resource="&rdfs;Literal"/>
		<skos:definition xml:lang="en">A textual description of the condition of the vehicle. This property should be mainly used with gr:ActualProductOrServiceInstance.</skos:definition>
	</owl:DatatypeProperty>
	
	<owl:ObjectProperty rdf:about="&auto-vc;contains">
		<rdfs:label xml:lang="en">contains</rdfs:label>
		<rdfs:domain rdf:resource="&auto-vc;OwnershipInfo"/>
		<rdfs:isDefinedBy rdf:resource="http://purl.org/uco/ns#"/>
		<rdfs:range rdf:resource="&auto-vc;OwnershipInfo"/>
		<skos:definition xml:lang="en">A naive part-whole relation that allows providing more granular uco:OwnershipInfo data for a part of the duration of the ownership</skos:definition>
	</owl:ObjectProperty>
	
	<owl:DatatypeProperty rdf:about="&auto-vc;countryOfOrigin">
		<rdfs:label xml:lang="en">country of origin</rdfs:label>
		<rdfs:domain rdf:resource="&auto-vc;Vehicle"/>
		<rdfs:isDefinedBy rdf:resource="http://purl.org/uco/ns#"/>
		<rdfs:range rdf:resource="&xsd;string"/>
		<skos:definition xml:lang="en">The country or geo-political region in which the vehicle was initially sold officially, indicated as the two-character version of ISO 3166-1 (ISO 3166-1 alpha-2) for regions or ISO 3166-2, which breaks down the countries from ISO 3166-1 into administrative subdivisions.</skos:definition>
	</owl:DatatypeProperty>
	
	<owl:DatatypeProperty rdf:about="&auto-vc;countryOfRegistration">
		<rdfs:label xml:lang="en">country of registration</rdfs:label>
		<rdfs:domain rdf:resource="&auto-vc;Vehicle"/>
		<rdfs:isDefinedBy rdf:resource="http://purl.org/uco/ns#"/>
		<rdfs:range rdf:resource="&xsd;string"/>
		<skos:definition xml:lang="en">The country or geo-political region in which the vehicle is currently registered, indicated as the two-character version of ISO 3166-1 (ISO 3166-1 alpha-2) for regions or ISO 3166-2, which breaks down the countries from ISO 3166-1 into administrative subdivisions.</skos:definition>
	</owl:DatatypeProperty>
	
	<owl:ObjectProperty rdf:about="&auto-vc;credit">
		<rdfs:label xml:lang="en">credit</rdfs:label>
		<rdfs:domain rdf:resource="&auto-vc;Financing"/>
		<rdfs:isDefinedBy rdf:resource="http://purl.org/vvo/ns#"/>
		<rdfs:range rdf:resource="&auto-vc;PriceSpecification"/>
		<skos:definition xml:lang="en">Indicates the credit for the financing</skos:definition>
	</owl:ObjectProperty>
	
	<owl:ObjectProperty rdf:about="&auto-vc;currentLocation">
		<rdfs:label xml:lang="en">current location</rdfs:label>
		<rdfs:domain rdf:resource="&auto-vc;Vehicle"/>
		<rdfs:isDefinedBy rdf:resource="http://purl.org/uco/ns#"/>
		<rdfs:range rdf:resource="&auto-mo;Location"/>
		<rdfs:range rdf:resource="&auto-mo;PostalAddress"/>
		<skos:definition xml:lang="en">The current location of the vehicle, i.e. where the car could be tested. For indicating alternative locations to which the seller is willing to bring the car, use gr:availableAtOrFrom attached to the gr:Offering, since those are aspects of the offer, not of the vehicle.</skos:definition>
	</owl:ObjectProperty>
	
	<owl:ObjectProperty rdf:about="&auto-vc;currentOwner">
		<rdfs:subPropertyOf rdf:resource="&auto-vc;owner"/>
		<rdfs:label xml:lang="en">current owner</rdfs:label>
		<rdfs:isDefinedBy rdf:resource="http://purl.org/uco/ns#"/>
		<skos:definition xml:lang="en">This property points to the current owner of the vehicle.</skos:definition>
	</owl:ObjectProperty>
	
	<owl:ObjectProperty rdf:about="&auto-vc;customerCashPrice">
		<rdfs:label xml:lang="en">customer cash price</rdfs:label>
		<rdfs:domain rdf:resource="&auto-vc;Financing"/>
		<rdfs:isDefinedBy rdf:resource="http://purl.org/vvo/ns#"/>
		<rdfs:range rdf:resource="&auto-vc;PriceSpecification"/>
		<skos:definition xml:lang="en">Indicates the customer cash price for the financing</skos:definition>
	</owl:ObjectProperty>
	
	<owl:ObjectProperty rdf:about="&auto-vc;customerDeposit">
		<rdfs:label xml:lang="en">customer deposit</rdfs:label>
		<rdfs:domain rdf:resource="&auto-vc;Financing"/>
		<rdfs:isDefinedBy rdf:resource="http://purl.org/vvo/ns#"/>
		<rdfs:range rdf:resource="&auto-vc;PriceSpecification"/>
		<skos:definition xml:lang="en">Indicates the customer deposit for the financing</skos:definition>
	</owl:ObjectProperty>
	
	<owl:DatatypeProperty rdf:about="&auto-vc;cylinderTypeId">
		<rdfs:label xml:lang="en">cylinder type id</rdfs:label>
		<rdfs:isDefinedBy rdf:resource="http://purl.org/vvo/ns#"/>
		<rdfs:range rdf:resource="&xsd;string"/>
		<skos:definition xml:lang="en">The Volkswagen-specific identifier for the cylinder type of a vehicle or engine</skos:definition>
	</owl:DatatypeProperty>
	
	<owl:DatatypeProperty rdf:about="&auto-vc;dateLaunched">
		<rdfs:subPropertyOf rdf:resource="&owl;topDataProperty"/>
		<rdfs:label xml:lang="en">date launched</rdfs:label>
		<rdfs:domain rdf:resource="&auto-vc;Vehicle"/>
		<rdfs:isDefinedBy rdf:resource="http://purl.org/vvo/ns#"/>
		<rdfs:range rdf:resource="&xsd;dateTime"/>
		<skos:definition xml:lang="en">The date of the official launch of the car model</skos:definition>
	</owl:DatatypeProperty>
	
	<owl:DatatypeProperty rdf:about="&auto-vc;dateVehicleFirstRegistered">
		<rdfs:subPropertyOf rdf:resource="&owl;topDataProperty"/>
		<rdfs:label xml:lang="en">date vehicle first registered</rdfs:label>
		<dct:isPartOf rdf:resource="http://auto.schema.org"/>
		<dct:source rdf:resource="http://www.w3.org/wiki/WebSchemas/SchemaDotOrgSources#Automotive_Ontology_Working_Group"/>
		<rdfs:domain rdf:resource="&auto-vc;Vehicle"/>
		<rdfs:isDefinedBy rdf:resource="http://purl.org/vso/ns"/>
		<rdfs:range rdf:resource="&xsd;dateTime"/>
		<skos:definition>The date of the first registration of the vehicle with the respective public authorities.</skos:definition>
		<skos:definition xml:lang="en">The date of the first registration of the vehicle with the respective public authorities. This property should be used mainly with gr:ActualProductOrServiceInstance.</skos:definition>
	</owl:DatatypeProperty>
	
	<owl:ObjectProperty rdf:about="&auto-vc;default">
		<rdfs:subPropertyOf rdf:resource="&auto-vc;availableChoice"/>
		<rdfs:label xml:lang="en">default</rdfs:label>
		<rdfs:isDefinedBy rdf:resource="http://purl.org/coo/ns#"/>
		<skos:definition xml:lang="en">This property links the default Choice or Component to a Spec Item. 
Since it is defined a sub-property of coo:availableChoice, the default choice is automatically part of the available choices.</skos:definition>
	</owl:ObjectProperty>
	
	<owl:ObjectProperty rdf:about="&auto-vc;dependsOn">
		<rdfs:label xml:lang="en">depends on</rdfs:label>
		<rdfs:domain rdf:resource="&auto-vc;ChoiceOrComponent"/>
		<rdfs:isDefinedBy rdf:resource="http://purl.org/coo/ns#"/>
		<rdfs:range rdf:resource="&auto-vc;ChoiceOrComponent"/>
		<skos:definition xml:lang="en">Links a Choice or Component to one or multiple other Choices Or Components required for that choice  

Note: This property is transitive, i.e., if B is required by A and C and D are required by B, then C and D are also required by A.</skos:definition>
	</owl:ObjectProperty>
	
	<owl:ObjectProperty rdf:about="&auto-vc;depositContribution">
		<rdfs:label xml:lang="en">deposit contribution</rdfs:label>
		<rdfs:domain rdf:resource="&auto-vc;Financing"/>
		<rdfs:isDefinedBy rdf:resource="http://purl.org/vvo/ns#"/>
		<rdfs:range rdf:resource="&auto-vc;PriceSpecification"/>
		<skos:definition xml:lang="en">Indicates the deposit contribution for the financing</skos:definition>
	</owl:ObjectProperty>
	
	<owl:DatatypeProperty rdf:about="&auto-vc;dhCode">
		<rdfs:label xml:lang="en">dh code</rdfs:label>
		<rdfs:domain rdf:resource="&auto-vc;Derivative"/>
		<rdfs:isDefinedBy rdf:resource="http://purl.org/vvo/ns#"/>
		<rdfs:range rdf:resource="&xsd;string"/>
		<skos:definition xml:lang="en">The DH code</skos:definition>
	</owl:DatatypeProperty>
	
	<owl:ObjectProperty rdf:about="&auto-vc;discount">
		<rdfs:label xml:lang="en">discount</rdfs:label>
		<rdfs:domain rdf:resource="&auto-vc;Financing"/>
		<rdfs:isDefinedBy rdf:resource="http://purl.org/vvo/ns#"/>
		<rdfs:range rdf:resource="&auto-vc;PriceSpecification"/>
		<skos:definition xml:lang="en">Indicates the discount for the financing</skos:definition>
	</owl:ObjectProperty>
	
	<owl:DatatypeProperty rdf:about="&auto-vc;displayPos">
		<rdfs:label xml:lang="en">display position</rdfs:label>
		<rdfs:isDefinedBy rdf:resource="http://purl.org/coo/ns#"/>
		<rdfs:range rdf:resource="&xsd;int"/>
		<skos:definition xml:lang="en">The position at which the option or element should be listed in a menu or user dialog, lower numbers come first.
The main usage of this property are coo:SpecItemCollection and coo:ChoiceOrComponent, but it is possible to apply it to any owl:Class.

Note: It is recommended to rely on this property only for data originating from a single RDF graph; otherwise, unpredictable results are possible.</skos:definition>
	</owl:DatatypeProperty>
	
	<owl:ObjectProperty rdf:about="&auto-vc;driveWheelConfiguration">
		<rdfs:subPropertyOf rdf:resource="&owl;topObjectProperty"/>
		<rdfs:label xml:lang="en">drive wheel configuration</rdfs:label>
		<dct:isPartOf rdf:resource="http://auto.schema.org"/>
		<dct:source rdf:resource="http://www.w3.org/wiki/WebSchemas/SchemaDotOrgSources#Automotive_Ontology_Working_Group"/>
		<rdfs:domain rdf:resource="&auto-vc;Vehicle"/>
		<rdfs:isDefinedBy rdf:resource="http://purl.org/vso/ns"/>
		<rdfs:range rdf:resource="&auto-vc;DriveWheelConfigurationValue"/>
		<rdfs:seeAlso rdf:resource="http://en.wikipedia.org/wiki/Drive_wheel"/>
		<skos:definition xml:lang="en">The drive wheel configuration, i.e. which roadwheels will receive torque from the vehicle&apos;s engine via the drivetrain</skos:definition>
		<skos:definition>The drive wheel configuration, i.e. which roadwheels will receive torque from the vehicle&apos;s engine via the drivetrain.</skos:definition>
	</owl:ObjectProperty>
	
	<owl:ObjectProperty rdf:about="&auto-vc;driver">
		<rdfs:label xml:lang="en">driver</rdfs:label>
		<rdfs:domain rdf:resource="&auto-vc;Vehicle"/>
		<rdfs:isDefinedBy rdf:resource="http://purl.org/uco/ns#"/>
		<rdfs:range rdf:resource="&auto-mo;Person"/>
		<skos:definition xml:lang="en">This property points to the driver or drivers that were regularly driving the vehicle during the respective period of time (when attached to uco:OwnershipInfo) or in total (when attached directly to a vso:Vehicle).</skos:definition>
	</owl:ObjectProperty>
	
	<owl:DatatypeProperty rdf:about="&auto-vc;emissionsCO2">
		<rdfs:label xml:lang="en">emissions CO2</rdfs:label>
		<dct:isPartOf rdf:resource="http://auto.schema.org"/>
		<dct:source rdf:resource="http://www.w3.org/wiki/WebSchemas/SchemaDotOrgSources#Automotive_Ontology_Working_Group"/>
		<rdfs:range rdf:resource="&xsd;float"/>
		<skos:definition>The CO2 emissions in g/km. When used in combination with a QuantitativeValue, put &quot;g/km&quot; into the unitText property of that value, since there is no UN/CEFACT Common Code for &quot;g/km&quot;.</skos:definition>
	</owl:DatatypeProperty>
	
	<owl:DatatypeProperty rdf:about="&auto-vc;emissionsPerPassenger">
		<rdfs:label xml:lang="en">emissions per passenger</rdfs:label>
		<rdfs:domain rdf:resource="&auto-vc;Vehicle"/>
		<rdfs:range rdf:resource="&rdfs;Literal"/>
		<skos:definition xml:lang="en">relates a vehicle to the amount of emissions it emits per passenger present in it during driving</skos:definition>
	</owl:DatatypeProperty>
	
	<owl:ObjectProperty rdf:about="&auto-vc;engineDisplacement">
		<rdfs:label xml:lang="en">engine displacement</rdfs:label>
		<dct:isPartOf rdf:resource="http://auto.schema.org"/>
		<dct:source rdf:resource="http://www.w3.org/wiki/WebSchemas/SchemaDotOrgSources#Automotive_Ontology_Working_Group"/>
		<rdfs:domain rdf:resource="&auto-vc;EngineSpecification"/>
		<rdfs:range rdf:resource="&auto-mo;QuantitativeValueFloat"/>
		<skos:definition>The volume swept by all of the pistons inside the cylinders of an internal combustion engine in a single movement. &lt;br/&gt;&lt;br/&gt;

Typical unit code(s): CMQ for cubic centimeter, LTR for liters, INQ for cubic inches
* Note 1: You can link to information about how the given value has been determined using the &lt;a class=&quot;localLink&quot; href=&quot;http://schema.org/valueReference&quot;&gt;valueReference&lt;/a&gt; property.
* Note 2: You can use &lt;a class=&quot;localLink&quot; href=&quot;http://schema.org/minValue&quot;&gt;minValue&lt;/a&gt; and &lt;a class=&quot;localLink&quot; href=&quot;http://schema.org/maxValue&quot;&gt;maxValue&lt;/a&gt; to indicate ranges.</skos:definition>
	</owl:ObjectProperty>
	
	<owl:DatatypeProperty rdf:about="&auto-vc;engineName">
		<rdfs:subPropertyOf rdf:resource="&owl;topDataProperty"/>
		<rdfs:label xml:lang="en">engine name</rdfs:label>
		<rdfs:domain rdf:resource="&auto-mo;Object"/>
		<rdfs:isDefinedBy rdf:resource="http://purl.org/vso/ns"/>
		<rdfs:range rdf:resource="&rdfs;Literal"/>
		<skos:definition xml:lang="en">A short text indicating the engine(s) of the vehicle</skos:definition>
	</owl:DatatypeProperty>
	
	<owl:ObjectProperty rdf:about="&auto-vc;enginePower">
		<rdfs:label xml:lang="en">engine power</rdfs:label>
		<dct:isPartOf rdf:resource="http://auto.schema.org"/>
		<dct:source rdf:resource="http://www.w3.org/wiki/WebSchemas/SchemaDotOrgSources#Automotive_Ontology_Working_Group"/>
		<rdfs:domain rdf:resource="&auto-vc;EngineSpecification"/>
		<rdfs:range rdf:resource="&auto-mo;QuantitativeValueFloat"/>
		<skos:definition>The power of the vehicle&apos;s engine.
    Typical unit code(s): KWT for kilowatt, BHP for brake horsepower, N12 for metric horsepower (PS, with 1 PS = 735,49875 W)&lt;br/&gt;&lt;br/&gt;

&lt;ul&gt;
&lt;li&gt;Note 1: There are many different ways of measuring an engine&apos;s power. For an overview, see  &lt;a href=&quot;http://en.wikipedia.org/wiki/Horsepower#Engine_power_test_codes&quot;&gt;http://en.wikipedia.org/wiki/Horsepower#Engine&lt;em&gt;power&lt;/em&gt;test_codes&lt;/a&gt;.&lt;/li&gt;
&lt;li&gt;Note 2: You can link to information about how the given value has been determined using the &lt;a class=&quot;localLink&quot; href=&quot;http://schema.org/valueReference&quot;&gt;valueReference&lt;/a&gt; property.&lt;/li&gt;
&lt;li&gt;Note 3: You can use &lt;a class=&quot;localLink&quot; href=&quot;http://schema.org/minValue&quot;&gt;minValue&lt;/a&gt; and &lt;a class=&quot;localLink&quot; href=&quot;http://schema.org/maxValue&quot;&gt;maxValue&lt;/a&gt; to indicate ranges.&lt;/li&gt;
&lt;/ul&gt;</skos:definition>
	</owl:ObjectProperty>
	
	<owl:ObjectProperty rdf:about="&auto-vc;engineType">
		<rdfs:subPropertyOf rdf:resource="&owl;topObjectProperty"/>
		<rdfs:label xml:lang="en">engine type</rdfs:label>
		<rdfs:label>engine type</rdfs:label>
		<dct:isPartOf rdf:resource="http://auto.schema.org"/>
		<dct:source rdf:resource="http://www.w3.org/wiki/WebSchemas/SchemaDotOrgSources#Automotive_Ontology_Working_Group"/>
		<rdfs:domain rdf:resource="&auto-vc;EngineSpecification"/>
		<rdfs:isDefinedBy rdf:resource="http://purl.org/vso/ns"/>
		<rdfs:range rdf:resource="&auto-vc;EngineTypeValue"/>
		<skos:definition>The type of engine or engines powering the vehicle.</skos:definition>
		<skos:definition xml:lang="en">The type of engine or engines powering the vehicle. If there are multiple engines, simply attach this property multiple times.

Use DBPedia resources to indicate the engine type. Popular identifiers are
  http://dbpedia.org/resource/Two-stroke_engine
  http://dbpedia.org/resource/Four-stroke_engine
  http://dbpedia.org/resource/Wankel_engine
  http://dbpedia.org/resource/Electric_motor

If you cannot find a suitable identifier in DBPedia, define your own as an instance of vso:EngineTypeValue.</skos:definition>
	</owl:ObjectProperty>
	
	<owl:ObjectProperty rdf:about="&auto-vc;eventInformation">
		<rdfs:label xml:lang="en">event information</rdfs:label>
		<rdfs:domain rdf:resource="&auto-vc;Vehicle"/>
		<rdfs:isDefinedBy rdf:resource="http://purl.org/uco/ns#"/>
		<skos:definition xml:lang="en">This property points to events related to the vehicle, like accidents and damages or major modifications or maintenance.</skos:definition>
	</owl:ObjectProperty>
	
	<owl:ObjectProperty rdf:about="&auto-vc;excessMileage">
		<rdfs:label xml:lang="en">excess mileage</rdfs:label>
		<rdfs:domain rdf:resource="&auto-vc;Financing"/>
		<rdfs:isDefinedBy rdf:resource="http://purl.org/vvo/ns#"/>
		<rdfs:range rdf:resource="&auto-vc;PriceSpecification"/>
		<skos:definition xml:lang="en">Indicates the rate for excess mileage</skos:definition>
	</owl:ObjectProperty>
	
	<owl:ObjectProperty rdf:about="&auto-vc;feature">
		<rdfs:subPropertyOf rdf:resource="&owl;topObjectProperty"/>
		<rdfs:label xml:lang="en">feature</rdfs:label>
		<rdfs:domain rdf:resource="&auto-vc;Vehicle"/>
		<rdfs:isDefinedBy rdf:resource="http://purl.org/uco/ns#"/>
		<rdfs:isDefinedBy rdf:resource="http://purl.org/vso/ns"/>
		<rdfs:range rdf:resource="&auto-mo;PropertyValue"/>
		<rdfs:seeAlso rdf:resource="http://dbpedia.org/resource/Category:Automotive_accessories"/>
		<rdfs:seeAlso rdf:resource="http://en.wikipedia.org/wiki/Category:Automotive_accessories"/>
		<skos:definition xml:lang="en">Indicates a built-in feature, accessory, or component of the vehicle.

Use DBPedia resources to indicate the features, if possible. Popular identifiers are
  http://dbpedia.org/resource/Anti-lock_braking_system
  http://dbpedia.org/resource/Electronic_stability_control
  http://dbpedia.org/resource/Armrest
  http://dbpedia.org/resource/Spoiler_%28automotive%29
  http://dbpedia.org/resource/CD_Changer
  http://dbpedia.org/resource/Cup_holder
  http://dbpedia.org/resource/Tow_hitch
  http://dbpedia.org/resource/Power_window
  http://dbpedia.org/resource/Power_steering
  http://dbpedia.org/resource/Air_conditioner
  http://dbpedia.org/resource/Child_safety_lock
  http://dbpedia.org/resource/Parking_sensors

See also http://en.wikipedia.org/wiki/Category:Automotive_accessories.

If you cannot find a suitable identifier in DBPedia, define your own as an instance of vso:FeatureValue.</skos:definition>
		<skos:definition xml:lang="en">This property points to vehicle features in a semi-structured property-value form.</skos:definition>
	</owl:ObjectProperty>
	
	<owl:ObjectProperty rdf:about="&auto-vc;featureOverride">
		<rdfs:label xml:lang="en">feature override</rdfs:label>
		<rdfs:domain>
			<owl:Class>
				<owl:unionOf rdf:parseType="Collection">
					<rdf:Description rdf:about="&auto-vc;ChoiceOrComponent">
					</rdf:Description>
					<rdf:Description rdf:about="&auto-vc;ConfigurationInfo">
					</rdf:Description>
				</owl:unionOf>
			</owl:Class>
		</rdfs:domain>
		<rdfs:isDefinedBy rdf:resource="http://purl.org/coo/ns#"/>
		<rdfs:range rdf:resource="&auto-vc;PropertySpecification"/>
		<skos:definition xml:lang="en">Links a coo:ConfigurationInfo node to information on how a choice or component or the combination of multiple choices will override the regular properties of the resulting vehicle</skos:definition>
	</owl:ObjectProperty>
	
	<owl:DatatypeProperty rdf:about="&auto-vc;finalPayment">
		<rdfs:label xml:lang="en">final payment</rdfs:label>
		<rdfs:domain rdf:resource="&auto-vc;Financing"/>
		<rdfs:isDefinedBy rdf:resource="http://purl.org/vvo/ns#"/>
		<rdfs:range rdf:resource="&xsd;decimal"/>
		<skos:definition xml:lang="en">Indicates the final payment for the financing</skos:definition>
	</owl:DatatypeProperty>
	
	<owl:ObjectProperty rdf:about="&auto-vc;finalPaymentFee">
		<rdfs:label xml:lang="en">final payment fee</rdfs:label>
		<rdfs:domain rdf:resource="&auto-vc;Financing"/>
		<rdfs:isDefinedBy rdf:resource="http://purl.org/vvo/ns#"/>
		<rdfs:range rdf:resource="&auto-vc;PriceSpecification"/>
		<skos:definition xml:lang="en">Indicates the final payment fee for the financing</skos:definition>
	</owl:ObjectProperty>
	
	<owl:ObjectProperty rdf:about="&auto-vc;firstMonthlyPaymentFee">
		<rdfs:label xml:lang="en">first monthly payment fee</rdfs:label>
		<rdfs:domain rdf:resource="&auto-vc;Financing"/>
		<rdfs:isDefinedBy rdf:resource="http://purl.org/vvo/ns#"/>
		<rdfs:range rdf:resource="&auto-vc;PriceSpecification"/>
		<skos:definition xml:lang="en">Indicates the first monthly payment fee for the financing</skos:definition>
	</owl:ObjectProperty>
	
	<owl:DatatypeProperty rdf:about="&auto-vc;from">
		<rdfs:label xml:lang="en">from</rdfs:label>
		<rdfs:domain rdf:resource="&auto-vc;OwnershipInfo"/>
		<rdfs:isDefinedBy rdf:resource="http://purl.org/uco/ns#"/>
		<rdfs:range rdf:resource="&xsd;dateTime"/>
		<skos:definition xml:lang="en">This property indicates the beginning of the period of ownership represented by this uco:OwnershipInfo node.</skos:definition>
	</owl:DatatypeProperty>
	
	<owl:ObjectProperty rdf:about="&auto-vc;fuelCapacity">
		<rdfs:label xml:lang="en">fuel capacity</rdfs:label>
		<dct:isPartOf rdf:resource="http://auto.schema.org"/>
		<dct:source rdf:resource="http://www.w3.org/wiki/WebSchemas/SchemaDotOrgSources#Automotive_Ontology_Working_Group"/>
		<rdfs:domain rdf:resource="&auto-vc;Vehicle"/>
		<rdfs:range rdf:resource="&auto-mo;QuantitativeValueFloat"/>
		<skos:definition>The capacity of the fuel tank or in the case of electric cars, the battery. If there are multiple components for storage, this should indicate the total of all storage of the same type.&lt;br/&gt;&lt;br/&gt;

Typical unit code(s): LTR for liters, GLL of US gallons, GLI for UK / imperial gallons, AMH for ampere-hours (for electrical vehicles).</skos:definition>
	</owl:ObjectProperty>
	
	<owl:ObjectProperty rdf:about="&auto-vc;fuelConsumption">
		<rdfs:label xml:lang="en">fuel consumption</rdfs:label>
		<rdfs:label xml:lang="en">fuel efficiency</rdfs:label>
		<dct:isPartOf rdf:resource="http://auto.schema.org"/>
		<dct:source rdf:resource="http://www.w3.org/wiki/WebSchemas/SchemaDotOrgSources#Automotive_Ontology_Working_Group"/>
		<rdfs:domain rdf:resource="&auto-vc;Vehicle"/>
		<rdfs:range rdf:resource="&auto-mo;QuantitativeValueFloat"/>
		<skos:definition>The amount of fuel consumed for traveling a particular distance or temporal duration with the given vehicle (e.g. liters per 100 km).

Note 1: There are unfortunately no standard unit codes for liters per 100 km. Use unitText to indicate the unit of measurement, e.g. L/100 km.
Note 2: There are two ways of indicating the fuel consumption, fuelConsumption (e.g. 8 liters per 100 km) and fuelEfficiency (e.g. 30 miles per gallon). They are reciprocal.
Note 3: Often, the absolute value is useful only when related to driving speed (&quot;at 80 km/h&quot;) or usage pattern (&quot;city traffic&quot;). You can use valueReference to link the value for the fuel consumption to another value.</skos:definition>
		<skos:definition>The distance traveled per unit of fuel used; most commonly miles per gallon (mpg) or kilometers per liter (km/L).

Note 1: There are unfortunately no standard unit codes for miles per gallon or kilometers per liter. Use unitText to indicate the unit of measurement, e.g. mpg or km/L.
Note 2: There are two ways of indicating the fuel consumption, fuelConsumption (e.g. 8 liters per 100 km) and fuelEfficiency (e.g. 30 miles per gallon). They are reciprocal.
Note 3: Often, the absolute value is useful only when related to driving speed (&quot;at 80 km/h&quot;) or usage pattern (&quot;city traffic&quot;). You can use valueReference to link the value for the fuel economy to another value.</skos:definition>
	</owl:ObjectProperty>
	
	<owl:DatatypeProperty rdf:about="&auto-vc;fuelInjectionTypeId">
		<rdfs:label xml:lang="en">fuel injection type id</rdfs:label>
		<rdfs:isDefinedBy rdf:resource="http://purl.org/vvo/ns#"/>
		<rdfs:range rdf:resource="&xsd;string"/>
		<skos:definition xml:lang="en">The Volkswagen-specific identifier for the fuel injection type of a vehicle or engine</skos:definition>
	</owl:DatatypeProperty>
	
	<owl:ObjectProperty rdf:about="&auto-vc;fuelType">
		<rdfs:subPropertyOf rdf:resource="&owl;topObjectProperty"/>
		<rdfs:label xml:lang="en">fuel type</rdfs:label>
		<dct:isPartOf rdf:resource="http://auto.schema.org"/>
		<dct:source rdf:resource="http://www.w3.org/wiki/WebSchemas/SchemaDotOrgSources#Automotive_Ontology_Working_Group"/>
		<rdfs:domain rdf:resource="&auto-vc;Vehicle"/>
		<rdfs:isDefinedBy rdf:resource="http://purl.org/vso/ns"/>
		<rdfs:range rdf:resource="&auto-vc;FuelTypeValue"/>
		<skos:definition xml:lang="en">The type of fuel suitable for the engine or engines of the vehicle.

Use DBPedia resources to indicate the fuel type. Popular identifiers are
  http://dbpedia.org/resource/Gasoline
  http://dbpedia.org/resource/Diesel
  http://dbpedia.org/resource/Biodiesel
  http://dbpedia.org/resource/Kerosene

For two-stroke mixtures, use vso:TwoStrokeMixture.</skos:definition>
		<skos:definition>The type of fuel suitable for the engine or engines of the vehicle. If the vehicle has only one engine, this property can be attached directly to the vehicle.</skos:definition>
	</owl:ObjectProperty>
	
	<owl:ObjectProperty rdf:about="&auto-vc;gearbox">
		<rdfs:subPropertyOf rdf:resource="&owl;topObjectProperty"/>
		<rdfs:label xml:lang="en">gearbox</rdfs:label>
		<rdfs:domain rdf:resource="&auto-vc;Vehicle"/>
		<rdfs:isDefinedBy rdf:resource="http://purl.org/vvo/ns#"/>
		<rdfs:range rdf:resource="&auto-vc;GearboxTypeValue"/>
		<rdfs:seeAlso rdf:resource="http://dbpedia.org/page/Transmission_%28mechanics%29"/>
		<rdfs:seeAlso rdf:resource="http://en.wikipedia.org/wiki/Transmission_%28mechanics%29"/>
		<skos:definition xml:lang="en">The gearbox type of the vehicle or vehicle model</skos:definition>
	</owl:ObjectProperty>
	
	<owl:DatatypeProperty rdf:about="&auto-vc;gearboxTypeId">
		<rdfs:label xml:lang="en">gearbox type id</rdfs:label>
		<rdfs:isDefinedBy rdf:resource="http://purl.org/vvo/ns#"/>
		<rdfs:range rdf:resource="&xsd;string"/>
		<skos:definition xml:lang="en">The Volkswagen-specific gearbox type ID</skos:definition>
	</owl:DatatypeProperty>
	
	<owl:ObjectProperty rdf:about="&auto-vc;hasCompleteCarModel">
		<rdfs:label xml:lang="en">has complete car model</rdfs:label>
		<rdfs:domain rdf:resource="&auto-vc;Derivative"/>
		<rdfs:isDefinedBy rdf:resource="http://purl.org/coo/ns#"/>
		<rdfs:range rdf:resource="&auto-vc;CompleteCarModel"/>
		<skos:definition xml:lang="en">Links one or multiple Complete Car Models to the underlying Derivative</skos:definition>
	</owl:ObjectProperty>
	
	<owl:ObjectProperty rdf:about="&auto-vc;hasDerivative">
		<rdfs:label xml:lang="en">has derivative</rdfs:label>
		<rdfs:domain rdf:resource="&auto-vc;Trim"/>
		<rdfs:isDefinedBy rdf:resource="http://purl.org/coo/ns#"/>
		<rdfs:range rdf:resource="&auto-vc;Derivative"/>
		<skos:definition xml:lang="en">Links a Derivative to a Trim</skos:definition>
	</owl:ObjectProperty>
	
	<owl:DatatypeProperty rdf:about="&auto-vc;hasElectricEnergyConsumtion">
		<rdfs:label xml:lang="en">has electric energy consumtion</rdfs:label>
		<rdfs:range rdf:resource="&rdfs;Literal"/>
		<skos:definition>This property represents the electric energy consumption of a vehicle measured in Wh/km.</skos:definition>
	</owl:DatatypeProperty>
	
	<owl:DatatypeProperty rdf:about="&auto-vc;hasEmissionsReduction">
		<rdfs:label xml:lang="en">has emissions reduction</rdfs:label>
		<rdfs:range rdf:resource="&rdfs;Literal"/>
		<skos:definition>This property represents emissions reduction measured in g/km that a vehicle has, through the implemented innovative technologies.</skos:definition>
	</owl:DatatypeProperty>
	
	<owl:DatatypeProperty rdf:about="&auto-vc;hasEngineCapacity">
		<rdfs:label xml:lang="en">has engine capacity</rdfs:label>
		<rdfs:range rdf:resource="&rdfs;Literal"/>
		<skos:definition>This property shows the capacity of the engine of a vehicle measured in cm3</skos:definition>
	</owl:DatatypeProperty>
	
	<owl:DatatypeProperty rdf:about="&auto-vc;hasFuelMode">
		<rdfs:label xml:lang="en">has fuel mode</rdfs:label>
		<rdfs:range rdf:resource="&rdfs;Literal"/>
		<skos:definition>This property represents the fuel mode of a vehicle</skos:definition>
	</owl:DatatypeProperty>
	
	<owl:DatatypeProperty rdf:about="&auto-vc;hasID">
		<rdfs:label xml:lang="en">has ID</rdfs:label>
		<rdfs:isDefinedBy rdf:resource="http://purl.org/coo/ns#"/>
		<rdfs:isDefinedBy rdf:resource="http://purl.org/vvo/ns#"/>
		<rdfs:range rdf:resource="&xsd;string"/>
		<skos:definition xml:lang="en">An annotation property that can be used to attach element identifiers from XML schemas for the corresponding XML data or schema</skos:definition>
		<skos:definition xml:lang="en">An annotation property that can be used to attach element identifiers from XML schemas for the corresponding XML data or schema.</skos:definition>
	</owl:DatatypeProperty>
	
	<owl:DatatypeProperty rdf:about="&auto-vc;hasInnovativeTechnology">
		<rdfs:label xml:lang="en">has innovative technology</rdfs:label>
		<rdfs:range rdf:resource="&rdfs;Literal"/>
		<skos:definition>This property represents an innovation technology that a vehicle has implemented.</skos:definition>
	</owl:DatatypeProperty>
	
	<owl:DatatypeProperty rdf:about="&auto-vc;hasMSRegManufacturerName">
		<rdfs:label xml:lang="en">has MSReg manufacturer name</rdfs:label>
		<rdfs:range rdf:resource="&rdfs;Literal"/>
		<skos:definition>This property represents a manufacturer name as in the registry of Member States of the European Environment Agency.</skos:definition>
	</owl:DatatypeProperty>
	
	<owl:DatatypeProperty rdf:about="&auto-vc;hasManufacturerHarmonisedName">
		<rdfs:label xml:lang="en">has manufacturer harmonised name</rdfs:label>
		<rdfs:range rdf:resource="&rdfs;Literal"/>
		<skos:definition>This property represents a manufacturer harmonised name.</skos:definition>
	</owl:DatatypeProperty>
	
	<owl:DatatypeProperty rdf:about="&auto-vc;hasManufacturerPooling">
		<rdfs:label xml:lang="en">has manufacturer pooling</rdfs:label>
		<rdfs:range rdf:resource="&rdfs;Literal"/>
		<skos:definition>This property represents a manufacturers pooling.</skos:definition>
	</owl:DatatypeProperty>
	
	<owl:DatatypeProperty rdf:about="&auto-vc;hasOtherAxleWidth">
		<rdfs:label xml:lang="en">has other axle width</rdfs:label>
		<rdfs:domain rdf:resource="&auto-vc;Vehicle"/>
		<rdfs:range rdf:resource="&rdfs;Literal"/>
		<skos:definition>This property represents the width of the other steering axle of a vehicle measured in mm.</skos:definition>
	</owl:DatatypeProperty>
	
	<owl:ObjectProperty rdf:about="&auto-vc;hasOwnershipInfo">
		<rdfs:label xml:lang="en">has ownership info</rdfs:label>
		<rdfs:domain rdf:resource="&auto-vc;Vehicle"/>
		<rdfs:isDefinedBy rdf:resource="http://purl.org/uco/ns#"/>
		<rdfs:range rdf:resource="&auto-vc;OwnershipInfo"/>
		<skos:definition xml:lang="en">This property points to information about the current and previous owners of the vehicle.</skos:definition>
	</owl:ObjectProperty>
	
	<owl:ObjectProperty rdf:about="&auto-vc;hasSpecItemChoice">
		<rdfs:label xml:lang="en">has spec item choice</rdfs:label>
		<rdfs:domain rdf:resource="&auto-vc;CompleteCarModel"/>
		<rdfs:isDefinedBy rdf:resource="http://purl.org/coo/ns#"/>
		<rdfs:range rdf:resource="&auto-vc;ChoiceOrComponent"/>
		<skos:definition xml:lang="en">Links a Complete Car Model to the choices for configurational options</skos:definition>
	</owl:ObjectProperty>
	
	<owl:ObjectProperty rdf:about="&auto-vc;hasSpecItems">
		<rdfs:label xml:lang="en">has spec items</rdfs:label>
		<rdfs:domain rdf:resource="&auto-vc;Derivative"/>
		<rdfs:isDefinedBy rdf:resource="http://purl.org/coo/ns#"/>
		<rdfs:range rdf:resource="&auto-vc;SpecItemCollection"/>
		<skos:definition xml:lang="en">This property links available Spec Items to a Derivative.</skos:definition>
	</owl:ObjectProperty>
	
	<owl:DatatypeProperty rdf:about="&auto-vc;hasSteeringAxleWidth">
		<rdfs:label xml:lang="en">has steering axle width</rdfs:label>
		<rdfs:domain rdf:resource="&auto-vc;Vehicle"/>
		<rdfs:range rdf:resource="&rdfs;Literal"/>
		<skos:definition>This property represents the width of the steering axle of a vehicle measured in mm.</skos:definition>
	</owl:DatatypeProperty>
	
	<owl:DatatypeProperty rdf:about="&auto-vc;hasTotalNewRegistrations">
		<rdfs:label xml:lang="en">has total new registrations</rdfs:label>
		<rdfs:domain rdf:resource="&auto-vc;Vehicle"/>
		<rdfs:range rdf:resource="&xsd;int"/>
		<skos:definition>This property represents the nubmer of total new registration of a vehicle.</skos:definition>
	</owl:DatatypeProperty>
	
	<owl:ObjectProperty rdf:about="&auto-vc;hasTrim">
		<rdfs:label xml:lang="en">has trim</rdfs:label>
		<rdfs:domain rdf:resource="&auto-vc;BaseModel"/>
		<rdfs:isDefinedBy rdf:resource="http://purl.org/coo/ns#"/>
		<rdfs:range rdf:resource="&auto-vc;Trim"/>
		<skos:definition xml:lang="en">Links a Trim to Base Model</skos:definition>
	</owl:ObjectProperty>
	
	<owl:DatatypeProperty rdf:about="&auto-vc;hasTypeApprovalNumber">
		<rdfs:label xml:lang="en">has type approval number</rdfs:label>
		<rdfs:range rdf:resource="&rdfs;Literal"/>
		<skos:definition>This property represents an internal type approval number.</skos:definition>
	</owl:DatatypeProperty>
	
	<owl:ObjectProperty rdf:about="&auto-vc;height">
		<rdfs:label xml:lang="en">height</rdfs:label>
		<rdfs:domain rdf:resource="&auto-vc;Vehicle"/>
		<rdfs:isDefinedBy rdf:resource="http://purl.org/vso/ns"/>
		<rdfs:range rdf:resource="&auto-mo;QuantitativeValueFloat"/>
		<skos:definition xml:lang="en">The outer height of the vehicle. Note that you can use gr:hasMinValueFloat and gr:hasMaxValueFloat to indicate ranges.
Typical unit code(s): CMT for centimeters, MTR for meters, INH for inches, FOT for foot/feet</skos:definition>
	</owl:ObjectProperty>
	
	<owl:ObjectProperty rdf:about="&auto-vc;heightOpenTailgate">
		<rdfs:label xml:lang="en">height open bonnet</rdfs:label>
		<rdfs:label xml:lang="en">height open tailgate</rdfs:label>
		<rdfs:domain rdf:resource="&auto-vc;Vehicle"/>
		<rdfs:isDefinedBy rdf:resource="http://purl.org/vvo/ns#"/>
		<rdfs:range rdf:resource="&auto-mo;QuantitativeValue"/>
		<skos:definition xml:lang="en">The outer height of the vehicle with the tailgate open. Note that you can use gr:hasMinValueFloat and gr:hasMaxValueFloat to indicate ranges.
Typical unit code(s): CMT for centimeters, MTR for meters, INH for inches, FOT for foot/feet</skos:definition>
	</owl:ObjectProperty>
	
	<owl:ObjectProperty rdf:about="&auto-vc;includes">
		<rdfs:label xml:lang="en">includes</rdfs:label>
		<rdfs:domain rdf:resource="&auto-vc;ChoiceOrComponent"/>
		<rdfs:isDefinedBy rdf:resource="http://purl.org/coo/ns#"/>
		<rdfs:range rdf:resource="&auto-vc;ChoiceOrComponent"/>
		<skos:definition xml:lang="en">Links a Choice or Component to one or multiple other Choices Or Components implicity contained

Note: This property is transitive, i.e., if B is included in A and C and D are included in B, then C and D are also included in A.</skos:definition>
	</owl:ObjectProperty>
	
	<owl:ObjectProperty rdf:about="&auto-vc;includesChoices">
		<rdfs:label xml:lang="en">includes choices</rdfs:label>
		<rdfs:domain rdf:resource="&auto-vc;ConfigurationInfo"/>
		<rdfs:isDefinedBy rdf:resource="http://purl.org/coo/ns#"/>
		<rdfs:range rdf:resource="&auto-vc;ChoiceOrComponent"/>
		<skos:definition xml:lang="en">Indicates the set of Choices Or Components to which the Configuration Info node refers

Note 1: Complementing compatibility information can be attached to the components directly via coo:compatibleWith, coo:incompatibleWith, coo:dependsOn, and coo:includes.
Note 2: The coo:ConfigurationInfo node makes only a valid statement for a configuration that includes ALL of the Choices or Components attached via this property. 
Note 3: If you want to know whether further components can be added, check that there are no coo:incompatibleWith relationships with any Choice or Component. This check must also be extended to all Choices or Components implicitly included via coo:includes.
Note 4: If you want to know whether some components may be omitted without invalidating the configuration, check that there are no coo:dependsOn relationships with any Choice or Component. This check must also be extended to all Choices Or Components implicitly included via coo:includes.
Note 5: Under an Open World Assumption (OWA), only an explicit compatibility statement for your configuration is really reliable. A weaker guarantee may be sufficient for your application, though.</skos:definition>
	</owl:ObjectProperty>
	
	<owl:ObjectProperty rdf:about="&auto-vc;incompatibleWith">
		<rdf:type rdf:resource="&owl;SymmetricProperty"/>
		<rdfs:label xml:lang="en">incompatible with</rdfs:label>
		<rdfs:domain rdf:resource="&auto-vc;ChoiceOrComponent"/>
		<rdfs:isDefinedBy rdf:resource="http://purl.org/coo/ns#"/>
		<rdfs:range rdf:resource="&auto-vc;ChoiceOrComponent"/>
		<skos:definition xml:lang="en">Indicates that two Choices or Components are incompatible with each other, independent from other choices.

Note: This property is symmetric, i.e., if A is incompatible with B, then B is also incompatible with A.</skos:definition>
	</owl:ObjectProperty>
	
	<owl:DatatypeProperty rdf:about="&auto-vc;indicationOfOdometerRollback">
		<rdfs:label xml:lang="en">indication of odometer rollback</rdfs:label>
		<rdfs:domain rdf:resource="&auto-vc;Vehicle"/>
		<rdfs:isDefinedBy rdf:resource="http://purl.org/uco/ns#"/>
		<rdfs:range rdf:resource="&xsd;boolean"/>
		<skos:definition xml:lang="en">This property indicates whether it is likely or known that the odometer of the vehicle does not properly reflect the total mileage of the vehicle, e.g. because the odometer has been replaced, reset, or tampered with</skos:definition>
	</owl:DatatypeProperty>
	
	<owl:ObjectProperty rdf:about="&auto-vc;inspected">
		<rdfs:label xml:lang="en">inspected</rdfs:label>
		<rdfs:domain rdf:resource="&auto-vc;Vehicle"/>
		<rdfs:isDefinedBy rdf:resource="http://purl.org/uco/ns#"/>
		<skos:definition xml:lang="en">This property points to inspections and certifications that the vehicle has undergone.</skos:definition>
	</owl:ObjectProperty>
	
	<owl:DatatypeProperty rdf:about="&auto-vc;insuranceGroup">
		<rdfs:label xml:lang="en">insurance group</rdfs:label>
		<rdfs:domain rdf:resource="&auto-vc;MotorizedRoadVehicle"/>
		<rdfs:isDefinedBy rdf:resource="http://purl.org/vvo/ns#"/>
		<rdfs:range rdf:resource="&xsd;string"/>
		<skos:definition xml:lang="en">The insurance group code</skos:definition>
	</owl:DatatypeProperty>
	
	<owl:DatatypeProperty rdf:about="&auto-vc;insuranceGroup50">
		<rdfs:label xml:lang="en">insurance group 50</rdfs:label>
		<rdfs:domain rdf:resource="&auto-vc;MotorizedRoadVehicle"/>
		<rdfs:isDefinedBy rdf:resource="http://purl.org/vvo/ns#"/>
		<rdfs:range rdf:resource="&xsd;string"/>
		<skos:definition xml:lang="en">The insurance group 50 code</skos:definition>
	</owl:DatatypeProperty>
	
	<owl:DatatypeProperty rdf:about="&auto-vc;knownVehicleDamages">
		<rdfs:label xml:lang="en">known vehicle damages</rdfs:label>
		<dct:isPartOf rdf:resource="http://auto.schema.org"/>
		<dct:source rdf:resource="http://www.w3.org/wiki/WebSchemas/SchemaDotOrgSources#Automotive_Ontology_Working_Group"/>
		<rdfs:domain rdf:resource="&auto-vc;Vehicle"/>
		<rdfs:isDefinedBy rdf:resource="http://purl.org/vso/ns"/>
		<rdfs:range rdf:resource="&xsd;string"/>
		<skos:definition>A textual description of known damages, both repaired and unrepaired.</skos:definition>
		<skos:definition xml:lang="en">A textual description of known damages, both repaired and unrepaired.

Note: This property should be used with gr:ActualProductOrServiceInstance (when offering a vehicle) or gr:ProductOrServicesSomeInstancesPlaceholder (when seeking a vehicle using gr:seeks) only.</skos:definition>
	</owl:DatatypeProperty>
	
	<owl:ObjectProperty rdf:about="&auto-vc;length">
		<rdfs:label xml:lang="en">length</rdfs:label>
		<rdfs:domain rdf:resource="&auto-vc;Vehicle"/>
		<rdfs:isDefinedBy rdf:resource="http://purl.org/vso/ns"/>
		<rdfs:range rdf:resource="&auto-mo;QuantitativeValueFloat"/>
		<skos:definition xml:lang="en">The outer length of the vehicle. Note that you can use gr:hasMinValueFloat and gr:hasMaxValueFloat to indicate ranges.
Typical unit code(s): CMT for centimeters, MTR for meters, INH for inches, FOT for foot/feet</skos:definition>
	</owl:ObjectProperty>
	
	<owl:DatatypeProperty rdf:about="&auto-vc;licensePlate">
		<rdfs:label xml:lang="en">license plate</rdfs:label>
		<rdfs:domain rdf:resource="&auto-vc;OwnershipInfo"/>
		<rdfs:isDefinedBy rdf:resource="http://purl.org/uco/ns#"/>
		<rdfs:range rdf:resource="&xsd;string"/>
		<skos:definition xml:lang="en">The license plate string(s) assigned to the vehicle during the period of ownership</skos:definition>
	</owl:DatatypeProperty>
	
	<owl:ObjectProperty rdf:about="&auto-vc;listPrice">
		<rdfs:label xml:lang="en">list price</rdfs:label>
		<rdfs:domain rdf:resource="&auto-vc;Vehicle"/>
		<rdfs:isDefinedBy rdf:resource="http://purl.org/uco/ns#"/>
		<rdfs:range rdf:resource="&auto-vc;PriceSpecification"/>
		<skos:definition xml:lang="en">The original list price of the new car at the time of production</skos:definition>
	</owl:ObjectProperty>
	
	<owl:ObjectProperty rdf:about="&auto-vc;luggageCapacitySeatsFolded">
		<rdfs:subPropertyOf rdf:resource="&auto-vc;cargoVolume"/>
		<rdfs:label xml:lang="en">luggage capacity seats folded</rdfs:label>
		<rdfs:isDefinedBy rdf:resource="http://purl.org/vvo/ns#"/>
		<skos:definition xml:lang="en">The available volume for cargo or luggage with the seats folded
Typical unit code(s): LTR for liters, FTQ for cubic foot/feet
  
Note: You can use gr:hasMinValueFloat and gr:hasMaxValueFloat to indicate ranges.</skos:definition>
	</owl:ObjectProperty>
	
	<owl:ObjectProperty rdf:about="&auto-vc;luggageCapacitySeatsUpright">
		<rdfs:subPropertyOf rdf:resource="&auto-vc;cargoVolume"/>
		<rdfs:label xml:lang="en">luggage capacity seats upright</rdfs:label>
		<rdfs:isDefinedBy rdf:resource="http://purl.org/vvo/ns#"/>
		<skos:definition xml:lang="en">The available volume for cargo or luggage with the seats upright
Typical unit code(s): LTR for liters, FTQ for cubic foot/feet
  
Note: You can use gr:hasMinValueFloat and gr:hasMaxValueFloat to indicate ranges.</skos:definition>
	</owl:ObjectProperty>
	
	<owl:ObjectProperty rdf:about="&auto-vc;mainLocation">
		<rdfs:label xml:lang="en">main location</rdfs:label>
		<rdfs:domain rdf:resource="&auto-vc;OwnershipInfo"/>
		<rdfs:isDefinedBy rdf:resource="http://purl.org/uco/ns#"/>
		<rdfs:range rdf:resource="&auto-mo;Location"/>
		<rdfs:range rdf:resource="&auto-mo;PostalAddress"/>
		<skos:definition xml:lang="en">The main location(s) of the vehicle during the period of ownership</skos:definition>
	</owl:ObjectProperty>
	
	<owl:DatatypeProperty rdf:about="&auto-vc;manufacturerCode">
		<rdfs:label xml:lang="en">manufacturer code</rdfs:label>
		<rdfs:domain rdf:resource="&auto-vc;Vehicle"/>
		<rdfs:isDefinedBy rdf:resource="http://purl.org/vvo/ns#"/>
		<rdfs:range rdf:resource="&xsd;string"/>
		<skos:definition xml:lang="en">The manufacturer code</skos:definition>
	</owl:DatatypeProperty>
	
	<owl:DatatypeProperty rdf:about="&auto-vc;marketingName">
		<rdfs:label xml:lang="en">marketing name</rdfs:label>
		<rdfs:isDefinedBy rdf:resource="http://purl.org/vvo/ns#"/>
		<rdfs:range rdf:resource="&xsd;string"/>
		<skos:definition xml:lang="en">The name of the object for marketing purposes</skos:definition>
	</owl:DatatypeProperty>
	
	<owl:DatatypeProperty rdf:about="&auto-vc;max">
		<rdfs:label xml:lang="en">max</rdfs:label>
		<rdfs:domain rdf:resource="&auto-vc;SpecItemCollection"/>
		<rdfs:isDefinedBy rdf:resource="http://purl.org/coo/ns#"/>
		<rdfs:range rdf:resource="&xsd;int"/>
		<skos:definition xml:lang="en">The maximum number of coo:ChoiceOrComponent entities that can be selected for a valid configuration</skos:definition>
	</owl:DatatypeProperty>
	
	<owl:ObjectProperty rdf:about="&auto-vc;meetsEmissionStandard">
		<rdfs:subPropertyOf rdf:resource="&owl;topObjectProperty"/>
		<rdfs:label xml:lang="en">meets emission standard</rdfs:label>
		<dct:isPartOf rdf:resource="http://auto.schema.org"/>
		<dct:source rdf:resource="http://www.w3.org/wiki/WebSchemas/SchemaDotOrgSources#Automotive_Ontology_Working_Group"/>
		<rdfs:domain rdf:resource="&auto-vc;Vehicle"/>
		<rdfs:isDefinedBy rdf:resource="http://purl.org/vso/ns"/>
		<rdfs:range rdf:resource="&auto-vc;EmissionStandardValue"/>
		<rdfs:seeAlso rdf:resource="http://en.wikipedia.org/wiki/Emissions_standard"/>
		<skos:definition>Indicates that the vehicle meets the respective emission standard.</skos:definition>
		<skos:definition xml:lang="en">Indicates that the vehicle meets the respective emission standard. 

Use DBPedia resources to indicate the standard, if possible. Popular identifiers are
  http://dbpedia.org/resource/Super_Ultra_Low_Emission_Vehicle
  http://dbpedia.org/resource/Partial_zero-emissions_vehicle

See also http://en.wikipedia.org/wiki/Emissions_standard.

Unfortunately, there are no DBPedia identifiers for the popular Euro 1 - Euro 5 standards available.
If you cannot find a suitable identifier in DBPedia, define your own as an instance of vso:EmissionStandardValue.</skos:definition>
	</owl:ObjectProperty>
	
	<owl:ObjectProperty rdf:about="&auto-vc;mileage">
		<rdfs:label xml:lang="en">mileage</rdfs:label>
		<rdfs:isDefinedBy rdf:resource="http://purl.org/uco/ns#"/>
		<rdfs:range rdf:resource="&auto-mo;QuantitativeValue"/>
		<skos:definition xml:lang="en">The mileage of the vehicle at the event, e.g. at the accident, maintenance, check, or modification. 

Typical unit code(s): KMT for kilometers, SMI for statute miles</skos:definition>
	</owl:ObjectProperty>
	
	<owl:ObjectProperty rdf:about="&auto-vc;mileageEnd">
		<rdfs:label xml:lang="en">mileage end</rdfs:label>
		<rdfs:domain rdf:resource="&auto-vc;OwnershipInfo"/>
		<rdfs:isDefinedBy rdf:resource="http://purl.org/uco/ns#"/>
		<rdfs:range rdf:resource="&auto-mo;QuantitativeValue"/>
		<skos:definition xml:lang="en">The mileage of the vehicle at the end of the period of ownership. 

Typical unit code(s): KMT for kilometers, SMI for statute miles</skos:definition>
	</owl:ObjectProperty>
	
	<owl:ObjectProperty rdf:about="&auto-vc;mileageFromOdometer">
		<rdfs:label xml:lang="en">mileage from odometer</rdfs:label>
		<dct:isPartOf rdf:resource="http://auto.schema.org"/>
		<dct:source rdf:resource="http://www.w3.org/wiki/WebSchemas/SchemaDotOrgSources#Automotive_Ontology_Working_Group"/>
		<rdfs:domain rdf:resource="&auto-vc;Vehicle"/>
		<rdfs:range rdf:resource="&auto-mo;QuantitativeValueFloat"/>
		<skos:definition>The total distance travelled by the particular vehicle since its initial production, as read from its odometer.

Typical unit code(s): KMT for kilometers, SMI for statute miles</skos:definition>
	</owl:ObjectProperty>
	
	<owl:ObjectProperty rdf:about="&auto-vc;mileageInitial">
		<rdfs:label xml:lang="en">mileage initial</rdfs:label>
		<rdfs:domain rdf:resource="&auto-vc;OwnershipInfo"/>
		<rdfs:isDefinedBy rdf:resource="http://purl.org/uco/ns#"/>
		<rdfs:range rdf:resource="&auto-mo;QuantitativeValue"/>
		<skos:definition xml:lang="en">The mileage of the vehicle at the beginning of the period of ownership. 

Typical unit code(s): KMT for kilometers, SMI for statute miles</skos:definition>
	</owl:ObjectProperty>
	
	<owl:DatatypeProperty rdf:about="&auto-vc;min">
		<rdfs:label xml:lang="en">min</rdfs:label>
		<rdfs:domain rdf:resource="&auto-vc;SpecItemCollection"/>
		<rdfs:isDefinedBy rdf:resource="http://purl.org/coo/ns#"/>
		<rdfs:range rdf:resource="&xsd;int"/>
		<skos:definition xml:lang="en">The minimum number of coo:ChoiceOrComponent entities that must be selected for a valid configuration</skos:definition>
	</owl:DatatypeProperty>
	
	<owl:ObjectProperty rdf:about="&auto-vc;monthlyPayment">
		<rdfs:label xml:lang="en">monthly payment</rdfs:label>
		<rdfs:domain rdf:resource="&auto-vc;Financing"/>
		<rdfs:isDefinedBy rdf:resource="http://purl.org/vvo/ns#"/>
		<rdfs:range rdf:resource="&auto-vc;PriceSpecification"/>
		<skos:definition xml:lang="en">Indicates the monthly payment for the financing</skos:definition>
	</owl:ObjectProperty>
	
	<owl:DatatypeProperty rdf:about="&auto-vc;noOfMonthlyPayments">
		<rdfs:label xml:lang="en">number of monthly payments</rdfs:label>
		<rdfs:domain rdf:resource="&auto-vc;Financing"/>
		<rdfs:isDefinedBy rdf:resource="http://purl.org/vvo/ns#"/>
		<rdfs:range rdf:resource="&xsd;decimal"/>
		<skos:definition xml:lang="en">The number of monthly payments</skos:definition>
	</owl:DatatypeProperty>
	
	<owl:DatatypeProperty rdf:about="&auto-vc;notAtFaultAccident">
		<rdfs:label xml:lang="en">not-at-fault accident</rdfs:label>
		<rdfs:domain rdf:resource="&auto-vc;DamageOrAccident"/>
		<rdfs:isDefinedBy rdf:resource="http://purl.org/uco/ns#"/>
		<rdfs:range rdf:resource="&xsd;boolean"/>
		<skos:definition xml:lang="en">This property indicates whether the accident leading to the damage was a not-at-fault accident from the perspective of the owner.</skos:definition>
	</owl:DatatypeProperty>
	
	<owl:DatatypeProperty rdf:about="&auto-vc;numberOfAirbags">
		<rdfs:label xml:lang="en">number of airbags</rdfs:label>
		<dct:isPartOf rdf:resource="http://auto.schema.org"/>
		<dct:source rdf:resource="http://www.w3.org/wiki/WebSchemas/SchemaDotOrgSources#Automotive_Ontology_Working_Group"/>
		<rdfs:domain rdf:resource="&auto-vc;Vehicle"/>
		<rdfs:range>
			<rdfs:Datatype>
				<owl:unionOf rdf:parseType="Collection">
					<rdf:Description rdf:about="&xsd;decimal">
					</rdf:Description>
					<rdf:Description rdf:about="&xsd;string">
					</rdf:Description>
				</owl:unionOf>
			</rdfs:Datatype>
		</rdfs:range>
		<skos:definition>The number or type of airbags in the vehicle.</skos:definition>
	</owl:DatatypeProperty>
	
	<owl:ObjectProperty rdf:about="&auto-vc;numberOfAxles">
		<rdfs:label xml:lang="en">number of axles</rdfs:label>
		<dct:isPartOf rdf:resource="http://auto.schema.org"/>
		<dct:source rdf:resource="http://www.w3.org/wiki/WebSchemas/SchemaDotOrgSources#Automotive_Ontology_Working_Group"/>
		<rdfs:domain rdf:resource="&auto-vc;Vehicle"/>
		<rdfs:range rdf:resource="&auto-mo;QuantitativeValueInteger"/>
		<skos:definition>The number of axles.

Typical unit code(s): C62</skos:definition>
	</owl:ObjectProperty>
	
	<owl:DatatypeProperty rdf:about="&auto-vc;numberOfDoors">
		<rdfs:label xml:lang="en">number of doors</rdfs:label>
		<dct:isPartOf rdf:resource="http://auto.schema.org"/>
		<dct:source rdf:resource="http://www.w3.org/wiki/WebSchemas/SchemaDotOrgSources#Automotive_Ontology_Working_Group"/>
		<rdfs:domain rdf:resource="&auto-vc;Vehicle"/>
		<rdfs:range rdf:resource="&xsd;decimal"/>
		<skos:definition>The number of doors.

Typical unit code(s): C62</skos:definition>
	</owl:DatatypeProperty>
	
	<owl:DatatypeProperty rdf:about="&auto-vc;numberOfDrivers">
		<rdfs:label xml:lang="en">number of drivers</rdfs:label>
		<rdfs:domain>
			<owl:Class>
				<owl:unionOf rdf:parseType="Collection">
					<rdf:Description rdf:about="&auto-vc;OwnershipInfo">
					</rdf:Description>
					<rdf:Description rdf:about="&auto-vc;Vehicle">
					</rdf:Description>
				</owl:unionOf>
			</owl:Class>
		</rdfs:domain>
		<rdfs:isDefinedBy rdf:resource="http://purl.org/uco/ns#"/>
		<rdfs:range rdf:resource="&xsd;integer"/>
		<skos:definition xml:lang="en">The number of people who were/are regularly driving the vehicle in the respective period of time (when attached to uco:OwnershipInfo) or in total (when directly applied to a vso:Vehicle)</skos:definition>
	</owl:DatatypeProperty>
	
	<owl:ObjectProperty rdf:about="&auto-vc;numberOfForwardGears">
		<rdfs:label xml:lang="en">number of forward gears</rdfs:label>
		<dct:isPartOf rdf:resource="http://auto.schema.org"/>
		<dct:source rdf:resource="http://www.w3.org/wiki/WebSchemas/SchemaDotOrgSources#Automotive_Ontology_Working_Group"/>
		<rdfs:domain rdf:resource="&auto-vc;Vehicle"/>
		<rdfs:range rdf:resource="&auto-mo;QuantitativeValueInteger"/>
		<skos:definition>The total number of forward gears available for the transmission system of the vehicle.

Typical unit code(s): C62</skos:definition>
	</owl:ObjectProperty>
	
	<owl:DatatypeProperty rdf:about="&auto-vc;numberOfOwners">
		<rdfs:label xml:lang="en">number of owners</rdfs:label>
		<rdfs:domain rdf:resource="&auto-vc;Vehicle"/>
		<rdfs:isDefinedBy rdf:resource="http://purl.org/uco/ns#"/>
		<rdfs:range rdf:resource="&xsd;integer"/>
		<skos:definition xml:lang="en">The total number of people or organizations who owned the vehicle, including the current owner.

Note that this value can be higher (but not lower) than the number of uco:OwnershipInfo nodes, since those records may be incomplete.</skos:definition>
	</owl:DatatypeProperty>
	
	<owl:DatatypeProperty rdf:about="&auto-vc;numberOfPassengers">
		<rdfs:label xml:lang="en">has number of passengers</rdfs:label>
		<rdfs:domain rdf:resource="&auto-vc;Vehicle"/>
		<rdfs:range rdf:resource="&xsd;int"/>
		<skos:definition xml:lang="en">relates a vehicle to the number of passengers it contains</skos:definition>
	</owl:DatatypeProperty>
	
	<owl:DatatypeProperty rdf:about="&auto-vc;offerPromoCode">
		<rdfs:label xml:lang="en">offer promo code</rdfs:label>
		<rdfs:domain rdf:resource="&auto-vc;Offering"/>
		<rdfs:isDefinedBy rdf:resource="http://purl.org/vvo/ns#"/>
		<rdfs:range rdf:resource="&xsd;string"/>
		<skos:definition xml:lang="en">The code for a promotional offer</skos:definition>
	</owl:DatatypeProperty>
	
	<owl:DatatypeProperty rdf:about="&auto-vc;originalPartsOnly">
		<rdfs:label xml:lang="en">original parts only</rdfs:label>
		<rdfs:domain>
			<owl:Class>
				<owl:unionOf rdf:parseType="Collection">
					<rdf:Description rdf:about="&auto-vc;DamageOrAccident">
					</rdf:Description>
					<rdf:Description rdf:about="&auto-vc;ModificationOrMaintenance">
					</rdf:Description>
				</owl:unionOf>
			</owl:Class>
		</rdfs:domain>
		<rdfs:isDefinedBy rdf:resource="http://purl.org/uco/ns#"/>
		<rdfs:range rdf:resource="&xsd;boolean"/>
		<skos:definition xml:lang="en">This indicates whether the parts used for repairing a damage, for a maintenance task, or a modification were all original.</skos:definition>
	</owl:DatatypeProperty>
	
	<owl:ObjectProperty rdf:about="&auto-vc;otrRetailPrice">
		<rdfs:label xml:lang="en">otr retail price</rdfs:label>
		<rdfs:domain rdf:resource="&auto-vc;Financing"/>
		<rdfs:isDefinedBy rdf:resource="http://purl.org/vvo/ns#"/>
		<rdfs:range rdf:resource="&auto-vc;PriceSpecification"/>
		<skos:definition xml:lang="en">Indicates the OTR retail price for the financing</skos:definition>
	</owl:ObjectProperty>
	
	<owl:ObjectProperty rdf:about="&auto-vc;owner">
		<rdfs:label xml:lang="en">owner</rdfs:label>
		<rdfs:domain rdf:resource="&auto-vc;OwnershipInfo"/>
		<rdfs:domain rdf:resource="&auto-vc;Vehicle"/>
		<rdfs:isDefinedBy rdf:resource="http://purl.org/uco/ns#"/>
		<rdfs:range rdf:resource="&auto-vc;BusinessEntity"/>
		<skos:definition xml:lang="en">This property points to the owner of the vehicle for the respective period of time, as indicated by the uco:OwnershipInfo node.</skos:definition>
	</owl:ObjectProperty>
	
	<owl:ObjectProperty rdf:about="&auto-vc;parking">
		<rdfs:label xml:lang="en">parking</rdfs:label>
		<rdfs:domain rdf:resource="&auto-vc;OwnershipInfo"/>
		<rdfs:domain rdf:resource="&auto-vc;Vehicle"/>
		<rdfs:isDefinedBy rdf:resource="http://purl.org/uco/ns#"/>
		<rdfs:range rdf:resource="&auto-vc;ParkingType"/>
		<skos:definition xml:lang="en">The main type(s) of parking that have been used for the vehicle during the period of ownership (if attached to uco:OwnershipInfo) or in general (if attached to the vso:Vehicle directly)</skos:definition>
	</owl:ObjectProperty>
	
	<owl:DatatypeProperty rdf:about="&auto-vc;partAdded">
		<rdfs:label xml:lang="en">part added</rdfs:label>
		<rdfs:domain rdf:resource="&auto-vc;ModificationOrMaintenance"/>
		<rdfs:isDefinedBy rdf:resource="http://purl.org/uco/ns#"/>
		<rdfs:range rdf:resource="&rdfs;Literal"/>
		<skos:definition xml:lang="en">A textual description of the part or parts added in the modification (e.g. tuning) or maintenance task</skos:definition>
	</owl:DatatypeProperty>
	
	<owl:DatatypeProperty rdf:about="&auto-vc;partRemoved">
		<rdfs:label xml:lang="en">part removed</rdfs:label>
		<rdfs:domain rdf:resource="&auto-vc;ModificationOrMaintenance"/>
		<rdfs:isDefinedBy rdf:resource="http://purl.org/uco/ns#"/>
		<rdfs:range rdf:resource="&rdfs;Literal"/>
		<skos:definition xml:lang="en">A textual description of the part or parts removed in the modification (e.g. tuning) or maintenance task</skos:definition>
	</owl:DatatypeProperty>
	
	<owl:DatatypeProperty rdf:about="&auto-vc;partReplaced">
		<rdfs:label xml:lang="en">part replaced</rdfs:label>
		<rdfs:domain rdf:resource="&auto-vc;ModificationOrMaintenance"/>
		<rdfs:isDefinedBy rdf:resource="http://purl.org/uco/ns#"/>
		<rdfs:range rdf:resource="&rdfs;Literal"/>
		<skos:definition xml:lang="en">A textual description of the part or parts replaced in the modification (e.g. tuning) or maintenance (e.g. new engine) task</skos:definition>
	</owl:DatatypeProperty>
	
	<owl:ObjectProperty rdf:about="&auto-vc;payload">
		<rdfs:label xml:lang="en">payload</rdfs:label>
		<dct:isPartOf rdf:resource="http://auto.schema.org"/>
		<dct:source rdf:resource="http://www.w3.org/wiki/WebSchemas/SchemaDotOrgSources#Automotive_Ontology_Working_Group"/>
		<rdfs:domain rdf:resource="&auto-vc;Vehicle"/>
		<rdfs:range rdf:resource="&auto-mo;QuantitativeValueFloat"/>
		<skos:definition>The permitted weight of passengers and cargo, EXCLUDING the weight of the empty vehicle.&lt;br/&gt;&lt;br/&gt;

Typical unit code(s): KGM for kilogram, LBR for pound&lt;br/&gt;&lt;br/&gt;

&lt;ul&gt;
&lt;li&gt;Note 1: Many databases specify the permitted TOTAL weight instead, which is the sum of &lt;a class=&quot;localLink&quot; href=&quot;http://schema.org/weight&quot;&gt;weight&lt;/a&gt; and &lt;a class=&quot;localLink&quot; href=&quot;http://schema.org/payload&quot;&gt;payload&lt;/a&gt;&lt;/li&gt;
&lt;li&gt;Note 2: You can indicate additional information in the &lt;a class=&quot;localLink&quot; href=&quot;http://schema.org/name&quot;&gt;name&lt;/a&gt; of the &lt;a class=&quot;localLink&quot; href=&quot;http://schema.org/QuantitativeValue&quot;&gt;QuantitativeValue&lt;/a&gt; node.&lt;/li&gt;
&lt;li&gt;Note 3: You may also link to a &lt;a class=&quot;localLink&quot; href=&quot;http://schema.org/QualitativeValue&quot;&gt;QualitativeValue&lt;/a&gt; node that provides additional information using &lt;a class=&quot;localLink&quot; href=&quot;http://schema.org/valueReference&quot;&gt;valueReference&lt;/a&gt;.&lt;/li&gt;
&lt;li&gt;Note 4: Note that you can use &lt;a class=&quot;localLink&quot; href=&quot;http://schema.org/minValue&quot;&gt;minValue&lt;/a&gt; and &lt;a class=&quot;localLink&quot; href=&quot;http://schema.org/maxValue&quot;&gt;maxValue&lt;/a&gt; to indicate ranges.&lt;/li&gt;
&lt;/ul&gt;</skos:definition>
	</owl:ObjectProperty>
	
	<owl:ObjectProperty rdf:about="&auto-vc;pets">
		<rdfs:label xml:lang="en">pets</rdfs:label>
		<rdfs:domain rdf:resource="&auto-vc;OwnershipInfo"/>
		<rdfs:domain rdf:resource="&auto-vc;Vehicle"/>
		<rdfs:isDefinedBy rdf:resource="http://purl.org/uco/ns#"/>
		<rdfs:range rdf:resource="&auto-vc;Species"/>
		<skos:definition xml:lang="en">The type(s) of animals that have been transported in the vehicle during the period of ownership (if attached to uco:OwnershipInfo) or in general (if attached to the vso:Vehicle directly). 
  
If possible, use DBPedia URIs, e.g. http://dbpedia.org/resource/Dog.</skos:definition>
	</owl:ObjectProperty>
	
	<owl:ObjectProperty rdf:about="&auto-vc;priceModifier">
		<rdfs:label xml:lang="en">price modiﬁer</rdfs:label>
		<rdfs:isDefinedBy rdf:resource="http://purl.org/coo/ns#"/>
		<rdfs:range rdf:resource="&auto-vc;RelativePriceSpecification"/>
		<skos:definition xml:lang="en">Links a coo:ConfigurationInfo node to information on a choice or component or the combination of multiple choices will affect the regular pricing of the resulting vehicle

Note: The use of gr:addOn is in general a better way of modeling surcharges</skos:definition>
	</owl:ObjectProperty>
	
	<owl:DatatypeProperty rdf:about="&auto-vc;productCode">
		<rdfs:label xml:lang="en">product code</rdfs:label>
		<rdfs:isDefinedBy rdf:resource="http://purl.org/vvo/ns#"/>
		<rdfs:range rdf:resource="&xsd;string"/>
		<skos:definition xml:lang="en">The Volkswagen-specific product code for the vehicle model, choice, component, spare part, or service</skos:definition>
	</owl:DatatypeProperty>
	
	<owl:DatatypeProperty rdf:about="&auto-vc;productionDate">
		<rdfs:label xml:lang="en">production date</rdfs:label>
		<dct:isPartOf rdf:resource="http://auto.schema.org"/>
		<dct:source rdf:resource="http://www.w3.org/wiki/WebSchemas/SchemaDotOrgSources#Automotive_Ontology_Working_Group"/>
		<rdfs:domain rdf:resource="&auto-vc;Vehicle"/>
		<rdfs:isDefinedBy rdf:resource="http://purl.org/vso/ns"/>
		<rdfs:range rdf:resource="&xsd;dateTime"/>
		<skos:definition>The date of production of the item, e.g. vehicle.</skos:definition>
		<skos:definition xml:lang="en">The date of production of the vehicle. This property should be used mainly with gr:ActualProductOrServiceInstance.</skos:definition>
	</owl:DatatypeProperty>
	
	<owl:DatatypeProperty rdf:about="&auto-vc;propertyID">
		<rdfs:label xml:lang="en">property ID</rdfs:label>
		<rdfs:domain rdf:resource="&auto-mo;PropertyValue"/>
		<rdfs:isDefinedBy rdf:resource="http://purl.org/uco/ns#"/>
		<rdfs:range rdf:resource="&rdfs;Literal"/>
		<skos:definition xml:lang="en">A global identifier, e.g. a URI, a prefixed string, or any other identifier that can be used to refer to a standardized property type</skos:definition>
	</owl:DatatypeProperty>
	
	<owl:DatatypeProperty rdf:about="&auto-vc;propertyName">
		<rdfs:label xml:lang="en">property name</rdfs:label>
		<rdfs:domain rdf:resource="&auto-mo;PropertyValue"/>
		<rdfs:isDefinedBy rdf:resource="http://purl.org/uco/ns#"/>
		<rdfs:range rdf:resource="&rdfs;Literal"/>
		<skos:definition xml:lang="en">The name of the property</skos:definition>
	</owl:DatatypeProperty>
	
	<owl:DatatypeProperty rdf:about="&auto-vc;propertyValue">
		<rdfs:label xml:lang="en">property value</rdfs:label>
		<rdfs:domain rdf:resource="&auto-mo;PropertyValue"/>
		<rdfs:isDefinedBy rdf:resource="http://purl.org/uco/ns#"/>
		<rdfs:range rdf:resource="&rdfs;Literal"/>
		<skos:definition xml:lang="en">The value of of the property</skos:definition>
	</owl:DatatypeProperty>
	
	<owl:DatatypeProperty rdf:about="&auto-vc;purchaseDate">
		<rdfs:label xml:lang="en">purchase date</rdfs:label>
		<dct:isPartOf rdf:resource="http://auto.schema.org"/>
		<dct:source rdf:resource="http://www.w3.org/wiki/WebSchemas/SchemaDotOrgSources#Automotive_Ontology_Working_Group"/>
		<rdfs:domain rdf:resource="&auto-vc;Vehicle"/>
		<rdfs:range rdf:resource="&xsd;dateTime"/>
		<skos:definition>The date the item e.g. vehicle was purchased by the current owner.</skos:definition>
	</owl:DatatypeProperty>
	
	<owl:ObjectProperty rdf:about="&auto-vc;referenceDistance">
		<rdfs:subPropertyOf rdf:resource="&auto-mo;valueReference"/>
		<rdfs:label xml:lang="en">reference distance</rdfs:label>
		<rdfs:domain rdf:resource="&auto-mo;QuantitativeValueFloat"/>
		<rdfs:isDefinedBy rdf:resource="http://purl.org/vso/ns"/>
		<rdfs:range rdf:resource="&auto-mo;QuantitativeValue"/>
		<skos:definition xml:lang="en">The distance to which a vso:fuelConsumption value refers</skos:definition>
	</owl:ObjectProperty>
	
	<owl:ObjectProperty rdf:about="&auto-vc;referenceFuelQuantity">
		<rdfs:subPropertyOf rdf:resource="&auto-mo;valueReference"/>
		<rdfs:label xml:lang="en">reference fuel quantity</rdfs:label>
		<rdfs:domain rdf:resource="&auto-mo;QuantitativeValueFloat"/>
		<rdfs:isDefinedBy rdf:resource="http://purl.org/vso/ns"/>
		<rdfs:range rdf:resource="&auto-vc;FuelQuantity"/>
		<skos:definition xml:lang="en">The quantity of fuel to which a vso:fuelEconomy value refers</skos:definition>
	</owl:ObjectProperty>
	
	<owl:ObjectProperty rdf:about="&auto-vc;referenceSpeeds">
		<rdfs:subPropertyOf rdf:resource="&auto-mo;valueReference"/>
		<rdfs:label xml:lang="en">reference speeds</rdfs:label>
		<rdfs:domain rdf:resource="&auto-mo;QuantitativeValueFloat"/>
		<rdfs:isDefinedBy rdf:resource="http://purl.org/vso/ns"/>
		<rdfs:range rdf:resource="&auto-vc;SpeedInterval"/>
		<skos:definition xml:lang="en">The interval of initial and target speed to which a vso:acceleration value refers</skos:definition>
	</owl:ObjectProperty>
	
	<owl:ObjectProperty rdf:about="&auto-vc;refersToTrafficPattern">
		<rdfs:subPropertyOf rdf:resource="&auto-mo;valueReference"/>
		<rdfs:label xml:lang="en">refers to traffic pattern</rdfs:label>
		<rdfs:domain rdf:resource="&auto-mo;QuantitativeValue"/>
		<rdfs:isDefinedBy rdf:resource="http://purl.org/vvo/ns#"/>
		<rdfs:range rdf:resource="&auto-vc;TrafficPattern"/>
		<skos:definition xml:lang="en">Indicates the traffic pattern to which the vso:fuelEconomy or vso:fuelConsumption value refers</skos:definition>
	</owl:ObjectProperty>
	
	<owl:DatatypeProperty rdf:about="&auto-vc;rentalUsage">
		<rdfs:label xml:lang="en">rental usage</rdfs:label>
		<rdfs:domain rdf:resource="&auto-vc;Vehicle"/>
		<rdfs:isDefinedBy rdf:resource="http://purl.org/vso/ns"/>
		<rdfs:range rdf:resource="&xsd;boolean"/>
		<skos:definition xml:lang="en">Indicates whether the vehicle has been used for commercial rental. The legislation in many countries requires this information to be revealed when offering a car for sale. 

Note 1: This property should be used with gr:ActualProductOrServiceInstance (when offering a vehicle) or gr:ProductOrServicesSomeInstancesPlaceholder (when seeking a vehicle using gr:seeks) only.
Note 2: This property is relevant mainly for offers to SELL the vehicle (gr:hasBusinessFunction gr:Sell).</skos:definition>
	</owl:DatatypeProperty>
	
	<owl:DatatypeProperty rdf:about="&auto-vc;repaired">
		<rdfs:label xml:lang="en">repaired</rdfs:label>
		<rdfs:domain>
			<owl:Class>
				<owl:unionOf rdf:parseType="Collection">
					<rdf:Description rdf:about="&auto-vc;DamageOrAccident">
					</rdf:Description>
					<rdf:Description rdf:about="&auto-vc;Vehicle">
					</rdf:Description>
				</owl:unionOf>
			</owl:Class>
		</rdfs:domain>
		<rdfs:isDefinedBy rdf:resource="http://purl.org/uco/ns#"/>
		<rdfs:range rdf:resource="&xsd;boolean"/>
		<skos:definition xml:lang="en">This indicates whether damages resulting from a certain uco:DamageOrAccident (when attached to this type) or all damages (when directly attached to a vso:Vehicle) have been properly repaired. Do not use this propery on a vso:Vehicle if it never had a damage.</skos:definition>
	</owl:DatatypeProperty>
	
	<owl:ObjectProperty rdf:about="&auto-vc;roofLoad">
		<rdfs:label xml:lang="en">roof load</rdfs:label>
		<dct:isPartOf rdf:resource="http://auto.schema.org"/>
		<dct:source rdf:resource="http://www.w3.org/wiki/WebSchemas/SchemaDotOrgSources#Automotive_Ontology_Working_Group"/>
		<rdfs:range rdf:resource="&auto-mo;QuantitativeValueFloat"/>
		<skos:definition>The permitted total weight of cargo and installations (e.g. a roof rack) on top of the vehicle.&lt;br/&gt;&lt;br/&gt;

Typical unit code(s): KGM for kilogram, LBR for pound&lt;br/&gt;&lt;br/&gt;

&lt;ul&gt;
&lt;li&gt;Note 1: You can indicate additional information in the &lt;a class=&quot;localLink&quot; href=&quot;http://schema.org/name&quot;&gt;name&lt;/a&gt; of the &lt;a class=&quot;localLink&quot; href=&quot;http://schema.org/QuantitativeValue&quot;&gt;QuantitativeValue&lt;/a&gt; node.&lt;/li&gt;
&lt;li&gt;Note 2: You may also link to a &lt;a class=&quot;localLink&quot; href=&quot;http://schema.org/QualitativeValue&quot;&gt;QualitativeValue&lt;/a&gt; node that provides additional information using &lt;a class=&quot;localLink&quot; href=&quot;http://schema.org/valueReference&quot;&gt;valueReference&lt;/a&gt;&lt;/li&gt;
&lt;li&gt;Note 3: Note that you can use &lt;a class=&quot;localLink&quot; href=&quot;http://schema.org/minValue&quot;&gt;minValue&lt;/a&gt; and &lt;a class=&quot;localLink&quot; href=&quot;http://schema.org/maxValue&quot;&gt;maxValue&lt;/a&gt; to indicate ranges.&lt;/li&gt;
&lt;/ul&gt;</skos:definition>
	</owl:ObjectProperty>
	
	<owl:ObjectProperty rdf:about="&auto-vc;rotationalSpeedReference">
		<rdfs:subPropertyOf rdf:resource="&auto-mo;valueReference"/>
		<rdfs:label xml:lang="en">rotational speed reference</rdfs:label>
		<rdfs:domain rdf:resource="&auto-mo;QuantitativeValue"/>
		<rdfs:isDefinedBy rdf:resource="http://purl.org/vvo/ns#"/>
		<rdfs:range rdf:resource="&auto-mo;QuantitativeValue"/>
		<skos:definition xml:lang="en">The rotational speed to which a vvo:torque or vso:enginePower value refers
Typical unit code(s): RPM for revolutions per minute or RPS for revolutions per second</skos:definition>
	</owl:ObjectProperty>
	
	<owl:ObjectProperty rdf:about="&auto-vc;scrappageContribution">
		<rdfs:label xml:lang="en">scrappage contribution</rdfs:label>
		<rdfs:domain rdf:resource="&auto-vc;Financing"/>
		<rdfs:isDefinedBy rdf:resource="http://purl.org/vvo/ns#"/>
		<rdfs:range rdf:resource="&auto-vc;PriceSpecification"/>
		<skos:definition xml:lang="en">Indicates the scrappage contribution for the financing</skos:definition>
	</owl:ObjectProperty>
	
	<owl:ObjectProperty rdf:about="&auto-vc;seatingCapacity">
		<rdfs:label xml:lang="en">seating capacity</rdfs:label>
		<rdfs:label xml:lang="en">vehicle seating capacity</rdfs:label>
		<dct:isPartOf rdf:resource="http://auto.schema.org"/>
		<dct:source rdf:resource="http://www.w3.org/wiki/WebSchemas/SchemaDotOrgSources#Automotive_Ontology_Working_Group"/>
		<rdfs:domain rdf:resource="&auto-vc;Vehicle"/>
		<rdfs:range rdf:resource="&auto-mo;QuantitativeValueInteger"/>
		<skos:definition>The number of passengers that can be seated in the vehicle, both in terms of the physical space available, and in terms of limitations set by law.

Typical unit code(s): C62 for persons.</skos:definition>
		<skos:definition>The number of persons that can be seated (e.g. in a vehicle), both in terms of the physical space available, and in terms of limitations set by law.&lt;br/&gt;&lt;br/&gt;

Typical unit code(s): C62 for persons</skos:definition>
	</owl:ObjectProperty>
	
	<owl:DatatypeProperty rdf:about="&auto-vc;serialNumber">
		<rdfs:label>serial number</rdfs:label>
		<skos:definition xml:lang="en">relates a vehicle to its serial number</skos:definition>
	</owl:DatatypeProperty>
	
	<owl:DatatypeProperty rdf:about="&auto-vc;shortSubtitle">
		<rdfs:label xml:lang="en">short subtitle</rdfs:label>
		<rdfs:domain>
			<owl:Class>
				<owl:unionOf rdf:parseType="Collection">
					<rdf:Description rdf:about="&auto-vc;Financing">
					</rdf:Description>
					<rdf:Description rdf:about="&auto-vc;Offering">
					</rdf:Description>
					<rdf:Description rdf:about="&auto-vc;Vehicle">
					</rdf:Description>
				</owl:unionOf>
			</owl:Class>
		</rdfs:domain>
		<rdfs:isDefinedBy rdf:resource="http://purl.org/vvo/ns#"/>
		<rdfs:range rdf:resource="&rdf;PlainLiteral"/>
		<skos:definition xml:lang="en">The short subtitle for a vehicle, component, offer, or financing option</skos:definition>
	</owl:DatatypeProperty>
	
	<owl:DatatypeProperty rdf:about="&auto-vc;shortTitle">
		<rdfs:label xml:lang="en">short title</rdfs:label>
		<rdfs:domain>
			<owl:Class>
				<owl:unionOf rdf:parseType="Collection">
					<rdf:Description rdf:about="&auto-vc;Financing">
					</rdf:Description>
					<rdf:Description rdf:about="&auto-vc;Offering">
					</rdf:Description>
					<rdf:Description rdf:about="&auto-vc;Vehicle">
					</rdf:Description>
				</owl:unionOf>
			</owl:Class>
		</rdfs:domain>
		<rdfs:isDefinedBy rdf:resource="http://purl.org/vvo/ns#"/>
		<rdfs:range rdf:resource="&rdf;PlainLiteral"/>
		<skos:definition xml:lang="en">The short title for a vehicle, component, offer, or financing option</skos:definition>
	</owl:DatatypeProperty>
	
	<owl:DatatypeProperty rdf:about="&auto-vc;smoking">
		<rdfs:label xml:lang="en">smoking</rdfs:label>
		<rdfs:domain>
			<owl:Class>
				<owl:unionOf rdf:parseType="Collection">
					<rdf:Description rdf:about="&auto-vc;OwnershipInfo">
					</rdf:Description>
					<rdf:Description rdf:about="&auto-vc;Vehicle">
					</rdf:Description>
				</owl:unionOf>
			</owl:Class>
		</rdfs:domain>
		<rdfs:isDefinedBy rdf:resource="http://purl.org/uco/ns#"/>
		<rdfs:range rdf:resource="&xsd;boolean"/>
		<skos:definition xml:lang="en">This property indicates whether it has been smoked inside the car in the respective period of time (when attached to uco:OwnershipInfo) or ever (when directly applied to a vso:Vehicle).</skos:definition>
	</owl:DatatypeProperty>
	
	<owl:ObjectProperty rdf:about="&auto-vc;speed">
		<rdfs:label xml:lang="en">speed</rdfs:label>
		<dct:isPartOf rdf:resource="http://auto.schema.org"/>
		<dct:source rdf:resource="http://www.w3.org/wiki/WebSchemas/SchemaDotOrgSources#Automotive_Ontology_Working_Group"/>
		<rdfs:domain rdf:resource="&auto-vc;Vehicle"/>
		<rdfs:range rdf:resource="&auto-mo;QuantitativeValueFloat"/>
		<skos:definition>The speed range of the vehicle. If the vehicle is powered by an engine, the upper limit of the speed range (indicated by &lt;a class=&quot;localLink&quot; href=&quot;http://schema.org/maxValue&quot;&gt;maxValue&lt;/a&gt; should be the maximum speed achievable under regular conditions.&lt;br/&gt;&lt;br/&gt;

Typical unit code(s): KMH for km/h, HM for mile per hour (0.447 04 m/s), KNT for knot&lt;br/&gt;&lt;br/&gt;

*Note 1: Use &lt;a class=&quot;localLink&quot; href=&quot;http://schema.org/minValue&quot;&gt;minValue&lt;/a&gt; and &lt;a class=&quot;localLink&quot; href=&quot;http://schema.org/maxValue&quot;&gt;maxValue&lt;/a&gt; to indicate the range. Typically, the minimal value is zero.
* Note 2: There are many different ways of measuring the speed range. You can link to information about how the given value has been determined using the &lt;a class=&quot;localLink&quot; href=&quot;http://schema.org/valueReference&quot;&gt;valueReference&lt;/a&gt; property.</skos:definition>
	</owl:ObjectProperty>
	
	<owl:ObjectProperty rdf:about="&auto-vc;steeringPosition">
		<rdfs:subPropertyOf rdf:resource="&owl;topObjectProperty"/>
		<rdfs:label xml:lang="en">steering position</rdfs:label>
		<dct:isPartOf rdf:resource="http://auto.schema.org"/>
		<dct:source rdf:resource="http://www.w3.org/wiki/WebSchemas/SchemaDotOrgSources#Automotive_Ontology_Working_Group"/>
		<rdfs:domain rdf:resource="&auto-vc;Vehicle"/>
		<rdfs:isDefinedBy rdf:resource="http://purl.org/vso/ns"/>
		<rdfs:range rdf:resource="&auto-vc;SteeringPositionValue"/>
		<skos:definition xml:lang="en">The position of the steering wheel or similar device (mostly for cars)</skos:definition>
		<skos:definition>The position of the steering wheel or similar device (mostly for cars).</skos:definition>
	</owl:ObjectProperty>
	
	<owl:DatatypeProperty rdf:about="&auto-vc;structuralDamage">
		<rdfs:label xml:lang="en">structural damage</rdfs:label>
		<rdfs:domain>
			<owl:Class>
				<owl:unionOf rdf:parseType="Collection">
					<rdf:Description rdf:about="&auto-vc;DamageOrAccident">
					</rdf:Description>
					<rdf:Description rdf:about="&auto-vc;Vehicle">
					</rdf:Description>
				</owl:unionOf>
			</owl:Class>
		</rdfs:domain>
		<rdfs:isDefinedBy rdf:resource="http://purl.org/uco/ns#"/>
		<rdfs:range rdf:resource="&xsd;boolean"/>
		<skos:definition xml:lang="en">This property indicates whether the vehicle has suffered from structural damage in the respective accident (when attached to uco:DamageOrAccident) or ever (when directly applied to a vso:Vehicle).</skos:definition>
	</owl:DatatypeProperty>
	
	<owl:DatatypeProperty rdf:about="&auto-vc;subtitle">
		<rdfs:label xml:lang="en">subtitle</rdfs:label>
		<rdfs:domain>
			<owl:Class>
				<owl:unionOf rdf:parseType="Collection">
					<rdf:Description rdf:about="&auto-vc;Financing">
					</rdf:Description>
					<rdf:Description rdf:about="&auto-vc;Offering">
					</rdf:Description>
					<rdf:Description rdf:about="&auto-vc;Vehicle">
					</rdf:Description>
				</owl:unionOf>
			</owl:Class>
		</rdfs:domain>
		<rdfs:isDefinedBy rdf:resource="http://purl.org/vvo/ns#"/>
		<rdfs:range rdf:resource="&rdf;PlainLiteral"/>
		<skos:definition xml:lang="en">The subtitle for a vehicle, component, offer, or financing option</skos:definition>
	</owl:DatatypeProperty>
	
	<owl:DatatypeProperty rdf:about="&auto-vc;termsAndConditions">
		<rdfs:label xml:lang="en">terms and conditions</rdfs:label>
		<rdfs:domain>
			<owl:Class>
				<owl:unionOf rdf:parseType="Collection">
					<rdf:Description rdf:about="&auto-vc;Financing">
					</rdf:Description>
					<rdf:Description rdf:about="&auto-vc;Offering">
					</rdf:Description>
					<rdf:Description rdf:about="&auto-vc;Vehicle">
					</rdf:Description>
				</owl:unionOf>
			</owl:Class>
		</rdfs:domain>
		<rdfs:isDefinedBy rdf:resource="http://purl.org/vvo/ns#"/>
		<rdfs:range rdf:resource="&rdf;PlainLiteral"/>
		<skos:definition xml:lang="en">Terms and conditions of the service, offer, or financing option</skos:definition>
	</owl:DatatypeProperty>
	
	<owl:DatatypeProperty rdf:about="&auto-vc;to">
		<rdfs:label xml:lang="en">to</rdfs:label>
		<rdfs:domain rdf:resource="&auto-vc;OwnershipInfo"/>
		<rdfs:isDefinedBy rdf:resource="http://purl.org/uco/ns#"/>
		<rdfs:range rdf:resource="&xsd;dateTime"/>
		<skos:definition xml:lang="en">This property indicates the end of the period of ownership represented by this uco:OwnershipInfo node.</skos:definition>
	</owl:DatatypeProperty>
	
	<owl:ObjectProperty rdf:about="&auto-vc;torque">
		<rdfs:label xml:lang="en">torque</rdfs:label>
		<dct:isPartOf rdf:resource="http://auto.schema.org"/>
		<dct:source rdf:resource="http://www.w3.org/wiki/WebSchemas/SchemaDotOrgSources#Automotive_Ontology_Working_Group"/>
		<rdfs:domain rdf:resource="&auto-vc;EngineSpecification"/>
		<rdfs:isDefinedBy rdf:resource="http://purl.org/vvo/ns#"/>
		<rdfs:range rdf:resource="&auto-mo;QuantitativeValue"/>
		<skos:definition xml:lang="en">The torque (turning force) of an engine
Typical unit code(s): NU for newton metre (N m), F17 for pound-force per foot, or F48 for pound-force per inch</skos:definition>
		<skos:definition>The torque (turning force) of the vehicle&apos;s engine.&lt;br/&gt;&lt;br/&gt;

Typical unit code(s): NU for newton metre (N m), F17 for pound-force per foot, or F48 for pound-force per inch&lt;br/&gt;&lt;br/&gt;

&lt;ul&gt;
&lt;li&gt;Note 1: You can link to information about how the given value has been determined (e.g. reference RPM) using the &lt;a class=&quot;localLink&quot; href=&quot;http://schema.org/valueReference&quot;&gt;valueReference&lt;/a&gt; property.&lt;/li&gt;
&lt;li&gt;Note 2: You can use &lt;a class=&quot;localLink&quot; href=&quot;http://schema.org/minValue&quot;&gt;minValue&lt;/a&gt; and &lt;a class=&quot;localLink&quot; href=&quot;http://schema.org/maxValue&quot;&gt;maxValue&lt;/a&gt; to indicate ranges.&lt;/li&gt;
&lt;/ul&gt;</skos:definition>
	</owl:ObjectProperty>
	
	<owl:ObjectProperty rdf:about="&auto-vc;totalPayable">
		<rdfs:label xml:lang="en">total payable</rdfs:label>
		<rdfs:domain rdf:resource="&auto-vc;Financing"/>
		<rdfs:isDefinedBy rdf:resource="http://purl.org/vvo/ns#"/>
		<rdfs:range rdf:resource="&auto-vc;PriceSpecification"/>
		<skos:definition xml:lang="en">Indicates the total payable for the financing</skos:definition>
	</owl:ObjectProperty>
	
	<owl:ObjectProperty rdf:about="&auto-vc;trailerWeight">
		<rdfs:label xml:lang="en">tongue weight</rdfs:label>
		<rdfs:label xml:lang="en">trailer weight</rdfs:label>
		<dct:isPartOf rdf:resource="http://auto.schema.org"/>
		<dct:source rdf:resource="http://www.w3.org/wiki/WebSchemas/SchemaDotOrgSources#Automotive_Ontology_Working_Group"/>
		<rdfs:domain rdf:resource="&auto-vc;Vehicle"/>
		<rdfs:range rdf:resource="&auto-mo;QuantitativeValueFloat"/>
		<skos:definition>The permitted vertical load (TWR) of a trailer attached to the vehicle. Also referred to as Tongue Load Rating (TLR) or Vertical Load Rating (VLR)&lt;br/&gt;&lt;br/&gt;

Typical unit code(s): KGM for kilogram, LBR for pound&lt;br/&gt;&lt;br/&gt;

&lt;ul&gt;
&lt;li&gt;Note 1: You can indicate additional information in the &lt;a class=&quot;localLink&quot; href=&quot;http://schema.org/name&quot;&gt;name&lt;/a&gt; of the &lt;a class=&quot;localLink&quot; href=&quot;http://schema.org/QuantitativeValue&quot;&gt;QuantitativeValue&lt;/a&gt; node.&lt;/li&gt;
&lt;li&gt;Note 2: You may also link to a &lt;a class=&quot;localLink&quot; href=&quot;http://schema.org/QualitativeValue&quot;&gt;QualitativeValue&lt;/a&gt; node that provides additional information using &lt;a class=&quot;localLink&quot; href=&quot;http://schema.org/valueReference&quot;&gt;valueReference&lt;/a&gt;.&lt;/li&gt;
&lt;li&gt;Note 3: Note that you can use &lt;a class=&quot;localLink&quot; href=&quot;http://schema.org/minValue&quot;&gt;minValue&lt;/a&gt; and &lt;a class=&quot;localLink&quot; href=&quot;http://schema.org/maxValue&quot;&gt;maxValue&lt;/a&gt; to indicate ranges.&lt;/li&gt;
&lt;/ul&gt;</skos:definition>
		<skos:definition>The permitted weight of a trailer attached to the vehicle.

Typical unit code(s): KGM for kilogram, LBR for pound

Note 1: You can indicate additional information in the name of the QuantitativeValue node. 

Note 2: You may also link to a QualitativeValue node that provides additional information using valueReference. 

Note 3: Note that you can use minValue and maxValue to indicate ranges.</skos:definition>
	</owl:ObjectProperty>
	
	<owl:ObjectProperty rdf:about="&auto-vc;transmission">
		<rdfs:subPropertyOf rdf:resource="&owl;topObjectProperty"/>
		<rdfs:label xml:lang="en">transmission</rdfs:label>
		<rdfs:isDefinedBy rdf:resource="http://purl.org/vso/ns"/>
		<rdfs:range rdf:resource="&auto-vc;TransmissionTypeValue"/>
		<rdfs:seeAlso rdf:resource="http://dbpedia.org/page/Transmission_%28mechanics%29"/>
		<rdfs:seeAlso rdf:resource="http://en.wikipedia.org/wiki/Transmission_%28mechanics%29"/>
		<skos:definition xml:lang="en">The type of component used for transmitting the power from a rotating power source to the wheels or propeller(s) (&quot;gearbox&quot; for cars).

Use DBPedia resources to indicate the transmission type, if possible. Popular identifiers are
  http://dbpedia.org/resource/Manual_transmission
  http://dbpedia.org/resource/Automatic_transmission

If you cannot find a suitable identifier in DBPedia, define your own as an instance of vso:TransmissionTypeValue.</skos:definition>
	</owl:ObjectProperty>
	
	<owl:DatatypeProperty rdf:about="&auto-vc;type">
		<rdfs:label>type</rdfs:label>
		<rdfs:domain rdf:resource="&auto-vc;Car"/>
		<rdfs:range rdf:resource="&rdfs;Literal"/>
		<skos:definition>This property represents an internal type of vehicle.</skos:definition>
	</owl:DatatypeProperty>
	
	<owl:DatatypeProperty rdf:about="&auto-vc;unitCode">
		<rdfs:label xml:lang="en">unit code</rdfs:label>
		<rdfs:domain rdf:resource="&auto-mo;PropertyValue"/>
		<rdfs:isDefinedBy rdf:resource="http://purl.org/uco/ns#"/>
		<rdfs:range rdf:resource="&xsd;string"/>
		<skos:definition xml:lang="en">A UN/CEFACT Common Code for indicating the unit of measurement of the value, if available</skos:definition>
	</owl:DatatypeProperty>
	
	<owl:DatatypeProperty rdf:about="&auto-vc;unitText">
		<rdfs:label xml:lang="en">unit text</rdfs:label>
		<rdfs:domain rdf:resource="&auto-mo;PropertyValue"/>
		<rdfs:isDefinedBy rdf:resource="http://purl.org/uco/ns#"/>
		<rdfs:range rdf:resource="&rdfs;Literal"/>
		<skos:definition xml:lang="en">A string or text indicating the unit of measurement. Useful if you cannot provide a standard unit code for uco:unitCode.</skos:definition>
	</owl:DatatypeProperty>
	
	<owl:ObjectProperty rdf:about="&auto-vc;usage">
		<rdfs:label xml:lang="en">usage</rdfs:label>
		<rdfs:domain rdf:resource="&auto-vc;OwnershipInfo"/>
		<rdfs:domain rdf:resource="&auto-vc;Vehicle"/>
		<rdfs:isDefinedBy rdf:resource="http://purl.org/uco/ns#"/>
		<rdfs:range rdf:resource="&auto-vc;CarUsageType"/>
		<skos:definition xml:lang="en">The type(s) of usage during the period of ownership (if attached to uco:OwnershipInfo) or in general (if attached to the vso:Vehicle directly)</skos:definition>
	</owl:ObjectProperty>
	
	<owl:DatatypeProperty rdf:about="&auto-vc;valid">
		<rdfs:label xml:lang="en">valid</rdfs:label>
		<rdfs:domain rdf:resource="&auto-vc;ConfigurationInfo"/>
		<rdfs:isDefinedBy rdf:resource="http://purl.org/coo/ns#"/>
		<rdfs:range rdf:resource="&xsd;boolean"/>
		<skos:definition xml:lang="en">Indicates whether the attached set of choices is a valid (true) or invalid (false) configuration for the Derivative</skos:definition>
	</owl:DatatypeProperty>
	
	<owl:DatatypeProperty rdf:about="&auto-vc;validFrom">
		<rdfs:label xml:lang="en">valid from</rdfs:label>
		<rdfs:domain rdf:resource="&auto-vc;Check"/>
		<rdfs:isDefinedBy rdf:resource="http://purl.org/uco/ns#"/>
		<rdfs:range rdf:resource="&xsd;dateTime"/>
		<skos:definition xml:lang="en">This property indicates the beginning of the validity of the inspection represented by the uco:Check node. This is typically the day of the inspection.</skos:definition>
	</owl:DatatypeProperty>
	
	<owl:DatatypeProperty rdf:about="&auto-vc;validThrough">
		<rdfs:label xml:lang="en">valid to</rdfs:label>
		<rdfs:domain rdf:resource="&auto-vc;Check"/>
		<rdfs:isDefinedBy rdf:resource="http://purl.org/uco/ns#"/>
		<rdfs:range rdf:resource="&xsd;dateTime"/>
		<skos:definition xml:lang="en">This property indicates the end of the validity of the inspection represented by the uco:Check node. This is typically the day of the inspection plus one (UK MOT) or two years (e.g. German TÜV).</skos:definition>
	</owl:DatatypeProperty>
	
	<owl:ObjectProperty rdf:about="&auto-vc;valuation">
		<rdfs:label xml:lang="en">valuation</rdfs:label>
		<rdfs:domain rdf:resource="&auto-vc;Vehicle"/>
		<rdfs:isDefinedBy rdf:resource="http://purl.org/uco/ns#"/>
		<rdfs:range rdf:resource="&auto-vc;PriceSpecification"/>
		<skos:definition xml:lang="en">The market price assessment gained by the respective valuation. Use gr:name to indicate the name of the valuation service.</skos:definition>
	</owl:ObjectProperty>
	
	<owl:DatatypeProperty rdf:about="&auto-vc;variant">
		<rdfs:label>variant</rdfs:label>
		<rdfs:range rdf:resource="&rdfs;Literal"/>
		<skos:definition>This property represents an internal variant code.</skos:definition>
	</owl:DatatypeProperty>
	
	<owl:DatatypeProperty rdf:about="&auto-vc;vehicleConfiguration">
		<rdfs:label xml:lang="en">vehicle configuration</rdfs:label>
		<dct:isPartOf rdf:resource="http://auto.schema.org"/>
		<dct:source rdf:resource="http://www.w3.org/wiki/WebSchemas/SchemaDotOrgSources#Automotive_Ontology_Working_Group"/>
		<rdfs:domain rdf:resource="&auto-vc;Vehicle"/>
		<rdfs:range rdf:resource="&xsd;string"/>
		<skos:definition>A short text indicating the configuration of the vehicle, e.g. &apos;5dr hatchback ST 2.5 MT 225 hp&apos; or &apos;limited edition&apos;.</skos:definition>
	</owl:DatatypeProperty>
	
	<owl:ObjectProperty rdf:about="&auto-vc;vehicleEngine">
		<rdfs:label xml:lang="en">vehicle engine</rdfs:label>
		<dct:isPartOf rdf:resource="http://auto.schema.org"/>
		<dct:source rdf:resource="http://www.w3.org/wiki/WebSchemas/SchemaDotOrgSources#Automotive_Ontology_Working_Group"/>
		<rdfs:domain rdf:resource="&auto-vc;Vehicle"/>
		<rdfs:range rdf:resource="&auto-vc;EngineSpecification"/>
		<skos:definition>Information about the engine or engines of the vehicle.</skos:definition>
	</owl:ObjectProperty>
	
	<owl:DatatypeProperty rdf:about="&auto-vc;vehicleIdentificationNumber">
		<rdfs:subPropertyOf rdf:resource="&auto-vc;serialNumber"/>
		<rdfs:label xml:lang="en">VIN</rdfs:label>
		<rdfs:label xml:lang="en">vehicle identification number</rdfs:label>
		<dct:isPartOf rdf:resource="http://auto.schema.org"/>
		<dct:source rdf:resource="http://www.w3.org/wiki/WebSchemas/SchemaDotOrgSources#Automotive_Ontology_Working_Group"/>
		<rdfs:domain rdf:resource="&auto-vc;Vehicle"/>
		<rdfs:isDefinedBy rdf:resource="http://purl.org/vso/ns"/>
		<rdfs:range rdf:resource="&xsd;string"/>
		<rdfs:seeAlso rdf:resource="http://dbpedia.org/resource/Vehicle_Identification_Number"/>
		<rdfs:seeAlso rdf:resource="http://en.wikipedia.org/wiki/Vehicle_Identification_Number"/>
		<skos:definition xml:lang="en">A unique serial number used by the automotive industry to identify individual motor vehicles</skos:definition>
		<skos:definition>The Vehicle Identification Number (VIN) is a unique serial number used by the automotive industry to identify individual motor vehicles.</skos:definition>
		<fibo-fnd-utl-av:abbreviation>VIN</fibo-fnd-utl-av:abbreviation>
		<fibo-fnd-utl-av:synonym xml:lang="en">Vehicle Identification Number</fibo-fnd-utl-av:synonym>
	</owl:DatatypeProperty>
	
	<owl:DatatypeProperty rdf:about="&auto-vc;vehicleInteriorColor">
		<rdfs:label xml:lang="en">vehicle interior color</rdfs:label>
		<dct:isPartOf rdf:resource="http://auto.schema.org"/>
		<dct:source rdf:resource="http://www.w3.org/wiki/WebSchemas/SchemaDotOrgSources#Automotive_Ontology_Working_Group"/>
		<rdfs:domain rdf:resource="&auto-vc;Vehicle"/>
		<rdfs:range rdf:resource="&xsd;string"/>
		<skos:definition>The color or color combination of the interior of the vehicle.</skos:definition>
	</owl:DatatypeProperty>
	
	<owl:DatatypeProperty rdf:about="&auto-vc;vehicleInteriorType">
		<rdfs:label xml:lang="en">vehicle interior type</rdfs:label>
		<dct:isPartOf rdf:resource="http://auto.schema.org"/>
		<dct:source rdf:resource="http://www.w3.org/wiki/WebSchemas/SchemaDotOrgSources#Automotive_Ontology_Working_Group"/>
		<rdfs:domain rdf:resource="&auto-vc;Vehicle"/>
		<rdfs:range rdf:resource="&xsd;string"/>
		<skos:definition>The type or material of the interior of the vehicle (e.g. synthetic fabric, leather, wood, etc.). While most interior types are characterized by the material used, an interior type can also be based on vehicle usage or target audience.</skos:definition>
	</owl:DatatypeProperty>
	
	<owl:DatatypeProperty rdf:about="&auto-vc;vehicleModelDate">
		<rdfs:label xml:lang="en">vehicle model date</rdfs:label>
		<dct:isPartOf rdf:resource="http://auto.schema.org"/>
		<dct:source rdf:resource="http://www.w3.org/wiki/WebSchemas/SchemaDotOrgSources#Automotive_Ontology_Working_Group"/>
		<rdfs:domain rdf:resource="&auto-vc;Vehicle"/>
		<rdfs:isDefinedBy rdf:resource="http://purl.org/vso/ns"/>
		<rdfs:range rdf:resource="&xsd;dateTime"/>
		<skos:definition xml:lang="en">The release date of a vehicle model (often used to differentiate versions of the same make and model)</skos:definition>
		<skos:definition>The release date of a vehicle model (often used to differentiate versions of the same make and model).</skos:definition>
	</owl:DatatypeProperty>
	
	<owl:ObjectProperty rdf:about="&auto-vc;vehicleSpecialUsage">
		<rdfs:label xml:lang="en">vehicle special usage</rdfs:label>
		<dct:isPartOf rdf:resource="http://auto.schema.org"/>
		<dct:source rdf:resource="http://www.w3.org/wiki/WebSchemas/SchemaDotOrgSources#Automotive_Ontology_Working_Group"/>
		<rdfs:domain rdf:resource="&auto-vc;Vehicle"/>
		<skos:definition>Indicates whether the vehicle has been used for special purposes, like commercial rental, driving school, or as a taxi. The legislation in many countries requires this information to be revealed when offering a car for sale.</skos:definition>
	</owl:ObjectProperty>
	
	<owl:ObjectProperty rdf:about="&auto-vc;vehicleTransmission">
		<rdfs:label xml:lang="en">vehicle transmission</rdfs:label>
		<dct:isPartOf rdf:resource="http://auto.schema.org"/>
		<dct:source rdf:resource="http://www.w3.org/wiki/WebSchemas/SchemaDotOrgSources#Automotive_Ontology_Working_Group"/>
		<rdfs:domain rdf:resource="&auto-vc;Vehicle"/>
		<rdfs:range>
			<owl:Class>
				<owl:unionOf rdf:parseType="Collection">
					<rdf:Description rdf:about="&auto-mo;QualitativeValue">
					</rdf:Description>
					<rdf:Description rdf:about="&auto-mo;TextValue">
					</rdf:Description>
				</owl:unionOf>
			</owl:Class>
		</rdfs:range>
		<skos:definition>The type of component used for transmitting the power from a rotating power source to the wheels or other relevant component(s) (&quot;gearbox&quot; for cars).</skos:definition>
	</owl:ObjectProperty>
	
	<owl:DatatypeProperty rdf:about="&auto-vc;vehicleTypeApprovedCategory">
		<rdfs:label>vehicle type approved category</rdfs:label>
		<rdfs:range rdf:resource="&rdfs;Literal"/>
		<skos:definition>This property represents a category of the approved vehicle type.</skos:definition>
	</owl:DatatypeProperty>
	
	<owl:DatatypeProperty rdf:about="&auto-vc;version">
		<rdfs:label>version</rdfs:label>
		<rdfs:domain rdf:resource="&auto-vc;Vehicle"/>
		<rdfs:range rdf:resource="&rdfs;Literal"/>
		<skos:definition>This property represents an internal version code of a vehicle.</skos:definition>
	</owl:DatatypeProperty>
	
	<owl:ObjectProperty rdf:about="&auto-vc;weightTotal">
		<rdfs:label xml:lang="en">weight total</rdfs:label>
		<dct:isPartOf rdf:resource="http://auto.schema.org"/>
		<dct:source rdf:resource="http://www.w3.org/wiki/WebSchemas/SchemaDotOrgSources#Automotive_Ontology_Working_Group"/>
		<rdfs:domain rdf:resource="&auto-vc;Vehicle"/>
		<rdfs:range rdf:resource="&auto-mo;QuantitativeValueFloat"/>
		<skos:definition>The permitted total weight of the loaded vehicle, including passengers and cargo and the weight of the empty vehicle.&lt;br/&gt;&lt;br/&gt;

Typical unit code(s): KGM for kilogram, LBR for pound&lt;br/&gt;&lt;br/&gt;

&lt;ul&gt;
&lt;li&gt;Note 1: You can indicate additional information in the &lt;a class=&quot;localLink&quot; href=&quot;http://schema.org/name&quot;&gt;name&lt;/a&gt; of the &lt;a class=&quot;localLink&quot; href=&quot;http://schema.org/QuantitativeValue&quot;&gt;QuantitativeValue&lt;/a&gt; node.&lt;/li&gt;
&lt;li&gt;Note 2: You may also link to a &lt;a class=&quot;localLink&quot; href=&quot;http://schema.org/QualitativeValue&quot;&gt;QualitativeValue&lt;/a&gt; node that provides additional information using &lt;a class=&quot;localLink&quot; href=&quot;http://schema.org/valueReference&quot;&gt;valueReference&lt;/a&gt;.&lt;/li&gt;
&lt;li&gt;Note 3: Note that you can use &lt;a class=&quot;localLink&quot; href=&quot;http://schema.org/minValue&quot;&gt;minValue&lt;/a&gt; and &lt;a class=&quot;localLink&quot; href=&quot;http://schema.org/maxValue&quot;&gt;maxValue&lt;/a&gt; to indicate ranges.&lt;/li&gt;
&lt;/ul&gt;</skos:definition>
	</owl:ObjectProperty>
	
	<owl:ObjectProperty rdf:about="&auto-vc;wheelbase">
		<rdfs:label xml:lang="en">wheelbase</rdfs:label>
		<dct:isPartOf rdf:resource="http://auto.schema.org"/>
		<dct:source rdf:resource="http://www.w3.org/wiki/WebSchemas/SchemaDotOrgSources#Automotive_Ontology_Working_Group"/>
		<rdfs:domain rdf:resource="&auto-vc;Vehicle"/>
		<rdfs:range rdf:resource="&auto-mo;QuantitativeValueFloat"/>
		<skos:definition>The distance between the centers of the front and rear wheels.&lt;br/&gt;&lt;br/&gt;

Typical unit code(s): CMT for centimeters, MTR for meters, INH for inches, FOT for foot/feet</skos:definition>
	</owl:ObjectProperty>
	
	<owl:ObjectProperty rdf:about="&auto-vc;width">
		<rdfs:label xml:lang="en">width</rdfs:label>
		<rdfs:domain rdf:resource="&auto-vc;Vehicle"/>
		<rdfs:isDefinedBy rdf:resource="http://purl.org/vso/ns"/>
		<rdfs:range rdf:resource="&auto-mo;QuantitativeValueFloat"/>
		<skos:definition xml:lang="en">The outer width of the vehicle. Note that you can use gr:hasMinValueFloat and gr:hasMaxValueFloat to indicate ranges.
Typical unit code(s): CMT for centimeters, MTR for meters, INH for inches, FOT for foot/feet</skos:definition>
	</owl:ObjectProperty>
	
	<owl:ObjectProperty rdf:about="&auto-vc;widthExcludingDoorMirrors">
		<rdfs:subPropertyOf rdf:resource="&auto-vc;width"/>
		<rdfs:label xml:lang="en">width excluding door mirrors</rdfs:label>
		<rdfs:isDefinedBy rdf:resource="http://purl.org/vvo/ns#"/>
		<skos:definition xml:lang="en">The outer width of the vehicle, excluding door mirrors. Note that you can use gr:hasMinValueFloat and gr:hasMaxValueFloat to indicate ranges.
Typical unit code(s): CMT for centimeters, MTR for meters, INH for inches, FOT for foot/feet</skos:definition>
	</owl:ObjectProperty>
	
	<owl:ObjectProperty rdf:about="&auto-vc;widthWithDoorsOpen">
		<rdfs:subPropertyOf rdf:resource="&auto-vc;width"/>
		<rdfs:label xml:lang="en">width with doors open</rdfs:label>
		<rdfs:isDefinedBy rdf:resource="http://purl.org/vvo/ns#"/>
		<skos:definition xml:lang="en">The outer width of the vehicle with the doors open. Note that you can use gr:hasMinValueFloat and gr:hasMaxValueFloat to indicate ranges.
Typical unit code(s): CMT for centimeters, MTR for meters, INH for inches, FOT for foot/feet</skos:definition>
	</owl:ObjectProperty>
	
	<owl:AnnotationProperty rdf:about="&fibo-fnd-utl-av;abbreviation">
	</owl:AnnotationProperty>
	
	<owl:AnnotationProperty rdf:about="&fibo-fnd-utl-av;adaptedFrom">
	</owl:AnnotationProperty>
	
	<owl:AnnotationProperty rdf:about="&fibo-fnd-utl-av;hasMaturityLevel">
	</owl:AnnotationProperty>
	
	<owl:AnnotationProperty rdf:about="&fibo-fnd-utl-av;synonym">
	</owl:AnnotationProperty>
	
	<owl:Axiom>
		<rdfs:seeAlso>https://www.law.cornell.edu/cfr/text/49/390.5</rdfs:seeAlso>
		<owl:annotatedProperty rdf:resource="&skos;definition"/>
		<owl:annotatedSource rdf:resource="&auto-vc;CoveredFarmVehicle"/>
		<owl:annotatedTarget xml:lang="en">straight truck or articulated vehicle that is registered in a State with a license plate or other designation issued by the State of registration that allows law enforcement officials to identify it as a farm vehicle and used to transport agricultural commodities, livestock, machinery or supplies to or from a farm or ranch</owl:annotatedTarget>
		<fibo-fnd-utl-av:adaptedFrom>49 C.F.R. § 390.5</fibo-fnd-utl-av:adaptedFrom>
	</owl:Axiom>
	<owl:Axiom>
		<rdfs:seeAlso>https://www.law.cornell.edu/cfr/text/49/393.5</rdfs:seeAlso>
		<owl:annotatedProperty rdf:resource="&skos;definition"/>
		<owl:annotatedSource rdf:resource="&auto-vc;AgriculturalCommodityTrailer"/>
		<owl:annotatedTarget xml:lang="en">trailer that is designed to transport bulk agricultural commodities in off-road harvesting sites and to a processing plant or storage location, as evidenced by skeletal construction that accommodates harvest containers, a maximum length of 28 feet, and an arrangement of air control lines and reservoirs that minimizes damage in field operations</owl:annotatedTarget>
		<fibo-fnd-utl-av:adaptedFrom>49 C.F.R. § 393.5</fibo-fnd-utl-av:adaptedFrom>
	</owl:Axiom>
	<owl:Axiom>
		<rdfs:seeAlso>https://www.law.cornell.edu/cfr/text/49/393.5</rdfs:seeAlso>
		<owl:annotatedProperty rdf:resource="&skos;definition"/>
		<owl:annotatedSource rdf:resource="&auto-vc;BoatTrailer"/>
		<owl:annotatedTarget xml:lang="en">trailer designed with cradle-type mountings to transport a boat and configured to permit the launching of the boat from the rear of the trailer</owl:annotatedTarget>
		<fibo-fnd-utl-av:adaptedFrom>49 C.F.R. § 393.5</fibo-fnd-utl-av:adaptedFrom>
	</owl:Axiom>
	<owl:Axiom>
		<rdfs:seeAlso>https://www.law.cornell.edu/cfr/text/49/393.5</rdfs:seeAlso>
		<owl:annotatedProperty rdf:resource="&skos;definition"/>
		<owl:annotatedSource rdf:resource="&auto-vc;ContainerChassisTrailer"/>
		<owl:annotatedTarget xml:lang="en">semitrailer of skeleton construction limited to a bottom frame, one or more axles, specially built and fitted with locking devices for the transport of intermodal cargo containers so that when the chassis and container are assembled, the units serve the same function as an over the road trailer</owl:annotatedTarget>
		<fibo-fnd-utl-av:adaptedFrom>49 C.F.R. § 393.5</fibo-fnd-utl-av:adaptedFrom>
	</owl:Axiom>
	<owl:Axiom>
		<rdfs:seeAlso>https://www.law.cornell.edu/cfr/text/49/393.5</rdfs:seeAlso>
		<owl:annotatedProperty rdf:resource="&skos;definition"/>
		<owl:annotatedSource rdf:resource="&auto-vc;CribTypeLogTrailer"/>
		<owl:annotatedTarget xml:lang="en">trailer equipped with stakes, bunks, a front-end structure, and a rear structure to restrain logs</owl:annotatedTarget>
		<fibo-fnd-utl-av:adaptedFrom>49 C.F.R. § 393.5</fibo-fnd-utl-av:adaptedFrom>
	</owl:Axiom>
	<owl:Axiom>
		<rdfs:seeAlso>https://www.law.cornell.edu/cfr/text/49/393.5</rdfs:seeAlso>
		<owl:annotatedProperty rdf:resource="&skos;definition"/>
		<owl:annotatedSource rdf:resource="&auto-vc;HeavyHaulerTrailer"/>
		<owl:annotatedTarget xml:lang="en">trailer whose brakes lines are designed to adapt to separation or extension of the vehicle frame and/or which body consists only of a platform whose primary cargo-carrying surface is not more than 1,016 mm (40 inches) above the ground in an unloaded condition, except that it may include sides that are designed to be easily removable and a permanent “front-end structure”, but that is not a container chassis trailer</owl:annotatedTarget>
		<fibo-fnd-utl-av:adaptedFrom>49 C.F.R. § 393.5</fibo-fnd-utl-av:adaptedFrom>
	</owl:Axiom>
	<owl:Axiom>
		<rdfs:seeAlso>https://www.law.cornell.edu/cfr/text/49/393.5</rdfs:seeAlso>
		<owl:annotatedProperty rdf:resource="&skos;definition"/>
		<owl:annotatedSource rdf:resource="&auto-vc;HorizontalDischargeTrailer"/>
		<owl:annotatedTarget xml:lang="en">trailer or semitrailer that is equipped with a mechanical drive and a conveyor to deliver asphalt and other road building materials, in a controlled horizontal manner, into a lay down machine or paving equipment for road construction and paving operations</owl:annotatedTarget>
		<fibo-fnd-utl-av:adaptedFrom>49 C.F.R. § 393.5</fibo-fnd-utl-av:adaptedFrom>
	</owl:Axiom>
	<owl:Axiom>
		<rdfs:seeAlso>https://www.law.cornell.edu/cfr/text/49/393.5</rdfs:seeAlso>
		<owl:annotatedProperty rdf:resource="&skos;definition"/>
		<owl:annotatedSource rdf:resource="&auto-vc;PulpwoodTrailer"/>
		<owl:annotatedTarget xml:lang="en">trailer or semitrailer that is designed exclusively for harvesting logs or pulpwood and constructed with a skeletal frame with no means for attachment of a solid bed, body, or container</owl:annotatedTarget>
		<fibo-fnd-utl-av:adaptedFrom>49 C.F.R. § 393.5</fibo-fnd-utl-av:adaptedFrom>
	</owl:Axiom>
	<owl:Axiom>
		<rdfs:seeAlso>https://www.law.cornell.edu/cfr/text/49/393.5</rdfs:seeAlso>
		<owl:annotatedProperty rdf:resource="&skos;definition"/>
		<owl:annotatedSource rdf:resource="&auto-vc;StraddleTrailer"/>
		<owl:annotatedTarget xml:lang="en">trailer that is designed to transport bulk agricultural commodities from the harvesting location, as evidenced by a framework that is driven over the cargo and lifting arms that suspend the cargo for transit</owl:annotatedTarget>
		<fibo-fnd-utl-av:adaptedFrom>49 C.F.R. § 393.5</fibo-fnd-utl-av:adaptedFrom>
	</owl:Axiom>
	<owl:Axiom>
		<rdfs:seeAlso>https://www.law.cornell.edu/cfr/text/49/393.5</rdfs:seeAlso>
		<owl:annotatedProperty rdf:resource="&skos;definition"/>
		<owl:annotatedSource rdf:resource="&auto-vc;TractorPoleTrailer"/>
		<owl:annotatedTarget xml:lang="en">combination vehicle that carries logs lengthwise so that they form the body of the vehicle</owl:annotatedTarget>
		<fibo-fnd-utl-av:adaptedFrom>49 C.F.R. § 393.5</fibo-fnd-utl-av:adaptedFrom>
	</owl:Axiom>
	<owl:Axiom>
		<owl:annotatedProperty rdf:resource="&skos;definition"/>
		<owl:annotatedSource rdf:resource="&auto-vc;PriceSpecification"/>
		<owl:annotatedTarget xml:lang="en">indication of the unit price and delivery or payment charges</owl:annotatedTarget>
		<fibo-fnd-utl-av:adaptedFrom>https://schema.org/priceSpecification</fibo-fnd-utl-av:adaptedFrom>
	</owl:Axiom>
	<owl:Axiom>
		<owl:annotatedProperty rdf:resource="&skos;definition"/>
		<owl:annotatedSource rdf:resource="&auto-vc;RoadVehicle"/>
		<owl:annotatedTarget xml:lang="en">land vehicle other than a railway vehicle</owl:annotatedTarget>
		<fibo-fnd-utl-av:adaptedFrom>ANSI D.16-2017, section 2.2.6</fibo-fnd-utl-av:adaptedFrom>
	</owl:Axiom>
</rdf:RDF>